@prefix dcterms: <http://purl.org/dc/terms/> .
@prefix omop: <https://w3id.org/omop/ontology/> .
@prefix owl: <http://www.w3.org/2002/07/owl#> .
@prefix owlready: <http://www.lesfleursdunormal.fr/static/_downloads/owlready_ontology.owl#> .
@prefix rdf: <http://www.w3.org/1999/02/22-rdf-syntax-ns#> .
@prefix rdfs: <http://www.w3.org/2000/01/rdf-schema#> .
@prefix vann: <http://purl.org/vocab/vann/> .
@prefix xsd: <http://www.w3.org/2001/XMLSchema#> .

<https://w3id.org/omop/ontology> a owl:Ontology ;
    rdfs:label "OWL ontology for the Observational Medical Outcomes Partnership Common Data Model (OMOP CDM)"^^xsd:string ;
    dcterms:license <https://www.gnu.org/licenses/lgpl-3.0> ;
    vann:preferredNamespacePrefix "omop" ;
    vann:preferredNamespaceUri "https://w3id.org/omop/ontology/" ;
    rdfs:comment "OWL ontology for the Observational Medical Outcomes Partnership Common Data Model (OMOP CDM) version 6.0."^^xsd:string .

omop:omop_cdm_name a owl:AnnotationProperty ;
    rdfs:label "OMOP CDM name"^^xsd:string .

omop:abbreviation a owl:DatatypeProperty,
        owl:FunctionalProperty ;
    rdfs:label "Abbreviation"^^xsd:string ;
    rdfs:comment "For Cdm Source: The abbreviation of the CDM instance."@en ;
    rdfs:domain omop:CdmSource ;
    rdfs:range xsd:string ;
    omop:omop_cdm_name "cdm_source.cdm_source_abbreviation#353 AS str"^^xsd:string .

omop:address_1 a owl:DatatypeProperty,
        owl:FunctionalProperty ;
    rdfs:label "Address 1"^^xsd:string ;
    rdfs:comment "For Location: This is the first line of the address."@en ;
    rdfs:domain omop:Location ;
    rdfs:range xsd:string ;
    omop:omop_cdm_name "location.address_1#252 AS str"^^xsd:string .

omop:address_2 a owl:DatatypeProperty,
        owl:FunctionalProperty ;
    rdfs:label "Address 2"^^xsd:string ;
    rdfs:comment "For Location: This is the second line of the address"@en ;
    rdfs:domain omop:Location ;
    rdfs:range xsd:string ;
    omop:omop_cdm_name "location.address_2#253 AS str"^^xsd:string .

omop:amount_value a owl:DatatypeProperty,
        owl:FunctionalProperty ;
    rdfs:label "Amount value"^^xsd:string ;
    rdfs:comment "For Drug Strength: The numeric value or the amount of active ingredient contained within the drug product."@en ;
    rdfs:domain omop:DrugStrength ;
    rdfs:range xsd:decimal ;
    omop:omop_cdm_name "drug_strength.amount_value#413 AS float"^^xsd:string .

omop:anatomic_site_source_value a owl:DatatypeProperty,
        owl:FunctionalProperty ;
    rdfs:label "Anatomic site source value"^^xsd:string ;
    rdfs:comment "For Specimen: This is the site on the body where the specimen was taken from, as represented in the source."@en ;
    rdfs:domain omop:Specimen ;
    rdfs:range xsd:string ;
    omop:omop_cdm_name "specimen.anatomic_site_source_value#220 AS str"^^xsd:string .

omop:assisted_source_value a owl:DatatypeProperty,
        owl:FunctionalProperty ;
    rdfs:label "Assisted source value"^^xsd:string ;
    rdfs:comment "For Survey Conduct: Source value representing whether patient required assistance to complete the survey. Example: 'Completed without assistance', 'Completed with assistance'."@en ;
    rdfs:domain omop:SurveyConduct ;
    rdfs:range xsd:string ;
    omop:omop_cdm_name "survey_conduct.assisted_source_value#239 AS str"^^xsd:string .

omop:billed_date a owl:DatatypeProperty,
        owl:FunctionalProperty ;
    rdfs:label "Billed date"^^xsd:string ;
    rdfs:comment "For Cost: The date a bill was generated for a service or encounter"@en ;
    rdfs:domain omop:Cost ;
    rdfs:range xsd:date ;
    omop:omop_cdm_name "cost.billed_date#318 AS date"^^xsd:string .

omop:birth_datetime a owl:DatatypeProperty,
        owl:FunctionalProperty ;
    rdfs:label "Birth datetime"^^xsd:string ;
    rdfs:comment "For Person: This field is not required but highly encouraged. For data sources that provide the precise datetime of birth, that value should be stored in this field. If birth_datetime is not provided in the source, use the following logic to infer the date: If day_of_birth is null and month_of_birth is not null then use the first of the month in that year. If month_of_birth is null or if day_of_birth AND month_of_birth are both null and the person has records during their year of birth then use the date of the earliest record, otherwise use the 15th of June of that year. If time of birth is not given use midnight (00:00:0000)."@en ;
    rdfs:domain omop:Person ;
    rdfs:range xsd:dateTime ;
    omop:omop_cdm_name "person.birth_datetime#6 AS datetime"^^xsd:string .

omop:box_size a owl:DatatypeProperty,
        owl:FunctionalProperty ;
    rdfs:label "Box size"^^xsd:string ;
    rdfs:comment "For Drug Strength: The number of units of Clinical Branded Drug or Quantified Clinical or Branded Drug contained in a box as dispensed to the patient."@en ;
    rdfs:domain omop:DrugStrength ;
    rdfs:range xsd:integer ;
    omop:omop_cdm_name "drug_strength.box_size#419 AS int"^^xsd:string .

omop:cause_source_value a owl:DatatypeProperty,
        owl:FunctionalProperty ;
    rdfs:label "Cause source value"^^xsd:string ;
    rdfs:domain omop:Death ;
    rdfs:range xsd:string ;
    omop:omop_cdm_name "death.cause_source_value#175 AS str"^^xsd:string .

omop:cdm_etl_reference a owl:DatatypeProperty,
        owl:FunctionalProperty ;
    rdfs:label "Cdm etl reference"^^xsd:string ;
    rdfs:comment "For Cdm Source: Put the link to the CDM version used."@en ;
    rdfs:domain omop:CdmSource ;
    rdfs:range xsd:string ;
    omop:omop_cdm_name "cdm_source.cdm_etl_reference#357 AS str"^^xsd:string .

omop:cdm_holder a owl:DatatypeProperty,
        owl:FunctionalProperty ;
    rdfs:label "Cdm holder"^^xsd:string ;
    rdfs:comment "For Cdm Source: The holder of the CDM instance."@en ;
    rdfs:domain omop:CdmSource ;
    rdfs:range xsd:string ;
    omop:omop_cdm_name "cdm_source.cdm_holder#354 AS str"^^xsd:string .

omop:cdm_release_date a owl:DatatypeProperty,
        owl:FunctionalProperty ;
    rdfs:label "Cdm release date"^^xsd:string ;
    rdfs:comment "For Cdm Source: The release data of the CDM instance."@en ;
    rdfs:domain omop:CdmSource ;
    rdfs:range xsd:date ;
    omop:omop_cdm_name "cdm_source.cdm_release_date#359 AS date"^^xsd:string .

omop:cdm_version a owl:DatatypeProperty,
        owl:FunctionalProperty ;
    rdfs:label "Cdm version"^^xsd:string ;
    rdfs:domain omop:CdmSource ;
    rdfs:range xsd:string ;
    omop:omop_cdm_name "cdm_source.cdm_version#360 AS str"^^xsd:string .

omop:city a owl:DatatypeProperty,
        owl:FunctionalProperty ;
    rdfs:label "City"^^xsd:string ;
    rdfs:domain omop:Location ;
    rdfs:range xsd:string ;
    omop:omop_cdm_name "location.city#254 AS str"^^xsd:string .

omop:cohort_initiation_date a owl:DatatypeProperty,
        owl:FunctionalProperty ;
    rdfs:label "Cohort initiation date"^^xsd:string ;
    rdfs:comment "For Cohort Definition: A date to indicate when the Cohort was initiated in the COHORT table."@en ;
    rdfs:domain omop:CohortDefinition ;
    rdfs:range xsd:date ;
    omop:omop_cdm_name "cohort_definition.cohort_initiation_date#433 AS date"^^xsd:string .

omop:collection_method_source_value a owl:DatatypeProperty,
        owl:FunctionalProperty ;
    rdfs:label "Collection method source value"^^xsd:string ;
    rdfs:comment "For Survey Conduct: The collection method as it appears in the source data."@en ;
    rdfs:domain omop:SurveyConduct ;
    rdfs:range xsd:string ;
    omop:omop_cdm_name "survey_conduct.collection_method_source_value#242 AS str"^^xsd:string .

omop:cost a owl:DatatypeProperty,
        owl:FunctionalProperty ;
    rdfs:label "Cost"^^xsd:string ;
    rdfs:comment "For Cost: The actual financial cost amount"@en ;
    rdfs:domain omop:Cost ;
    rdfs:range xsd:decimal ;
    omop:omop_cdm_name "cost.cost#316 AS float"^^xsd:string .

omop:county a owl:DatatypeProperty,
        owl:FunctionalProperty ;
    rdfs:label "County"^^xsd:string ;
    rdfs:domain omop:Location ;
    rdfs:range xsd:string ;
    omop:omop_cdm_name "location.county#257 AS str"^^xsd:string .

omop:date a owl:DatatypeProperty,
        owl:FunctionalProperty ;
    rdfs:label "Date"^^xsd:string ;
    rdfs:comment """For Measurement: Use this date to determine the date of the measurement.
If there are multiple dates in the source data associated with a record such as order_date, draw_date, and result_date, choose the one that is closest to the date the sample was drawn from the patient."""@en,
        "For Note Nlp: The date of the note processing."@en,
        "For Note: The date the note was recorded."@en,
        """For Observation: The date of the Observation. Depending on what the Observation represents this could be the date of a lab test, the date of a survey, or the date a patient's family history was taken.
For some observations the ETL may need to make a choice as to which date to choose."""@en,
        """For Procedure Occurrence: Use this date to determine the date the procedure occurred.
If a procedure lasts more than a day, then it should be recorded as a separate record for each day the procedure occurred, this logic is in lieu of the procedure_end_date, which will be added in a future version of the CDM."""@en,
        "For Specimen: The date the specimen was collected."@en ;
    rdfs:domain omop:Event ;
    rdfs:range xsd:date ;
    omop:omop_cdm_name "death.death_date#171 AS date"^^xsd:string,
        "measurement.measurement_date#132 AS date"^^xsd:string,
        "metadata.metadata_date#350 AS date"^^xsd:string,
        "note.note_date#181 AS date"^^xsd:string,
        "note_nlp.nlp_date#202 AS date"^^xsd:string,
        "observation.observation_date#152 AS date"^^xsd:string,
        "procedure_occurrence.procedure_date#103 AS date"^^xsd:string,
        "specimen.specimen_date#211 AS date"^^xsd:string .

omop:datetime a owl:DatatypeProperty,
        owl:FunctionalProperty ;
    rdfs:label "Datetime"^^xsd:string ;
    rdfs:comment "For Measurement: This is not required, though it is in v6. If a source does not specify datetime the convention is to set the time to midnight (00:00:0000)"@en,
        "For Note Nlp: The date and time of the note processing."@en,
        "For Note: If time is not given set the time to midnight."@en,
        "For Observation: If no time is given set to midnight (00:00:00)."@en,
        "For Procedure Occurrence: This is not required, though it is in v6. If a source does not specify datetime the convention is to set the time to midnight (00:00:0000)"@en ;
    rdfs:domain omop:Event ;
    rdfs:range xsd:dateTime ;
    omop:omop_cdm_name "death.death_datetime#172 AS datetime"^^xsd:string,
        "measurement.measurement_datetime#133 AS datetime"^^xsd:string,
        "metadata.metadata_datetime#351 AS datetime"^^xsd:string,
        "note.note_datetime#182 AS datetime"^^xsd:string,
        "note_nlp.nlp_datetime#203 AS datetime"^^xsd:string,
        "observation.observation_datetime#153 AS datetime"^^xsd:string,
        "procedure_occurrence.procedure_datetime#104 AS datetime"^^xsd:string,
        "specimen.specimen_datetime#212 AS datetime"^^xsd:string .

omop:day_of_birth a owl:DatatypeProperty,
        owl:FunctionalProperty ;
    rdfs:label "Day of birth"^^xsd:string ;
    rdfs:comment "For Person: For data sources that provide the precise date of birth, the day should be extracted and stored in this field."@en ;
    rdfs:domain omop:Person ;
    rdfs:range xsd:integer ;
    omop:omop_cdm_name "person.day_of_birth#5 AS int"^^xsd:string .

omop:days_supply a owl:DatatypeProperty,
        owl:FunctionalProperty ;
    rdfs:label "Days supply"^^xsd:string ;
    rdfs:comment "For Drug Exposure: Days supply of the drug. This should be the verbatim days_supply as given on the prescription. If the drug is physician administered use duration end date if given or set to 1 as default if duration is not available."@en ;
    rdfs:domain omop:DrugExposure ;
    rdfs:range xsd:integer ;
    omop:omop_cdm_name "drug_exposure.days_supply#89 AS int"^^xsd:string .

omop:dea a owl:DatatypeProperty,
        owl:FunctionalProperty ;
    rdfs:label "Dea"^^xsd:string ;
    rdfs:comment "For Provider: This is the identifier issued by the DEA, a US federal agency, that allows a provider to write prescriptions for controlled substances."@en ;
    rdfs:domain omop:Provider ;
    rdfs:range xsd:string ;
    omop:omop_cdm_name "provider.dea#276 AS str"^^xsd:string .

omop:death_datetime a owl:DatatypeProperty,
        owl:FunctionalProperty ;
    rdfs:label "Death datetime"^^xsd:string ;
    rdfs:comment """For Person: This field is the death date to be used in analysis, as determined by the ETL logic. Any additional information about a Person's death is stored in the [OBSERVATION](https://ohdsi.github.io/CommonDataModel/cdm60.html#observation) table with the concept_id [4306655](https://athena.ohdsi.org/search-terms/terms/4306655) or in the CONDITION_OCCURRENCE .
If there are multiple dates of death given for a Person, choose the one that is deemed most reliable. This may be a discharge from the hospital where the Person is listed as deceased or it could be latest death date provided. If a patient has clinical activity more than 60 days after the death date given in the source, it is a viable option to drop the death record as it may have been falsely reported. Similarly, if the death record is from a reputable source (e.g. government provided information) it is also a viable option to remove event records that occur in the data > 60 days after death."""@en ;
    rdfs:domain omop:Person ;
    rdfs:range xsd:dateTime ;
    omop:omop_cdm_name "person.death_datetime#7 AS datetime"^^xsd:string .

omop:denominator_value a owl:DatatypeProperty,
        owl:FunctionalProperty ;
    rdfs:label "Denominator value"^^xsd:string ;
    rdfs:comment "For Drug Strength: The amount of total liquid (or other divisible product, such as ointment, gel, spray, etc.)."@en ;
    rdfs:domain omop:DrugStrength ;
    rdfs:range xsd:decimal ;
    omop:omop_cdm_name "drug_strength.denominator_value#417 AS float"^^xsd:string .

omop:description a owl:DatatypeProperty,
        owl:FunctionalProperty ;
    rdfs:label "Description"^^xsd:string ;
    rdfs:comment "For Cohort Definition: A complete description of the cohort."@en ;
    rdfs:domain omop:CohortDefinition ;
    rdfs:range xsd:string ;
    omop:omop_cdm_name "cohort_definition.cohort_definition_description#429 AS str"^^xsd:string .

omop:discharge_to_source_value a owl:DatatypeProperty,
        owl:FunctionalProperty ;
    rdfs:label "Discharge to source value"^^xsd:string ;
    rdfs:comment "For Visit Detail: This information may be called something different in the source data but the field is meant to contain a value indicating where a person was discharged to after a visit, as in they went home or were moved to long-term care. Typically this applies only to visits that have a length of stay of a day or more."@en,
        "For Visit Occurrence: This information may be called something different in the source data but the field is meant to contain a value indicating where a person was discharged to after a visit, as in they went home or were moved to long-term care. Typically this applies only to visits that have a length of stay of a day or more."@en ;
    rdfs:domain omop:BaseVisit ;
    rdfs:range xsd:string ;
    omop:omop_cdm_name "visit_detail.discharge_to_source_value#56 AS str"^^xsd:string,
        "visit_occurrence.discharge_to_source_value#40 AS str"^^xsd:string .

omop:disease_status_source_value a owl:DatatypeProperty,
        owl:FunctionalProperty ;
    rdfs:label "Disease status source value"^^xsd:string ;
    rdfs:domain omop:Specimen ;
    rdfs:range xsd:string ;
    omop:omop_cdm_name "specimen.disease_status_source_value#221 AS str"^^xsd:string .

omop:dose_unit_source_value a owl:DatatypeProperty,
        owl:FunctionalProperty ;
    rdfs:label "Dose unit source value"^^xsd:string ;
    rdfs:comment """For Drug Exposure: This field houses the verbatim value from the source data representing the dose unit of the drug given.
This information may be called something different in the source data but the field is meant to contain a value indicating the unit of dosage of drug given to the patient. This is an older column and will be deprecated in an upcoming version."""@en ;
    rdfs:domain omop:DrugExposure ;
    rdfs:range xsd:string ;
    omop:omop_cdm_name "drug_exposure.dose_unit_source_value#99 AS str"^^xsd:string .

omop:drg_source_value a owl:DatatypeProperty,
        owl:FunctionalProperty ;
    rdfs:label "Drg source value"^^xsd:string ;
    rdfs:comment "For Cost: The source value for the 3-digit DRG source code as it appears in the source data, stored here for reference."@en ;
    rdfs:domain omop:Cost ;
    rdfs:range xsd:string ;
    omop:omop_cdm_name "cost.drg_source_value#323 AS str"^^xsd:string .

omop:end_date a owl:DatatypeProperty,
        owl:FunctionalProperty ;
    rdfs:label "End date"^^xsd:string ;
    rdfs:comment """For Condition Occurrence: Use this date to determine the end date of the condition
Most often data sources do not have the idea of a start date for a condition. Rather, if a source only has one date associated with a condition record it is acceptable to use that date for both the CONDITION_START_DATE and the CONDITION_END_DATE."""@en,
        """For Device Exposure: The DEVICE_EXPOSURE_END_DATE denotes the day the device exposure ended for the patient, if given.
Put the end date or discontinuation date as it appears from the source data or leave blank if unavailable."""@en,
        """For Drug Exposure: The DRUG_EXPOSURE_END_DATE denotes the day the drug exposure ended for the patient.
If this information is not explicitly available in the data, infer the end date using the following methods:/n/n 1. Start first with duration or days supply using the calculation drug start date + days supply -1 day. 2. Use quantity divided by daily dose that you may obtain from the sig or a source field (or assumed daily dose of 1) for solid, indivisibile, drug products. If quantity represents ingredient amount, quantity divided by daily dose * concentration (from drug_strength) drug concept id tells you the dose form. 3. If it is an administration record, set drug end date equal to drug start date. If the record is a written prescription then set end date to start date + 29. If the record is a mail-order prescription set end date to start date + 89. The end date must be equal to or greater than the start date. Ibuprofen 20mg/mL oral solution concept tells us this is oral solution. Calculate duration as quantity (200 example) * daily dose (5mL) /concentration (20mg/mL) 200*5/20 = 50 days. [Examples by dose form](https://ohdsi.github.io/CommonDataModel/drug_dose.html)"""@en,
        "For Location History: The date the relationship ended"@en,
        """For Observation Period: Use this date to determine the end date of the period for which we can assume that all events for a Person are recorded.
It is often the case that the idea of Observation Periods does not exist in source data. In those cases, the observation_period_end_date can be inferred as the last Event date available for the Person. In insurance claim data, the Observation Period can be considered as the time period the Person is enrolled with a payer."""@en,
        "For Payer Plan Period: End date of Plan coverage."@en,
        """For Visit Detail: This the end date of the patient-provider interaction.
Visit Detail end dates are mandatory. If end dates are not provided in the source there are three ways in which to derive them:<br>
- Outpatient Visit Detail: visit_detail_end_datetime = visit_detail_start_datetime
- Emergency Room Visit Detail: visit_detail_end_datetime = visit_detail_start_datetime
- Inpatient Visit Detail: Usually there is information about discharge. If not, you should be able to derive the end date from the sudden decline of activity or from the absence of inpatient procedures/drugs.
- Non-hospital institution Visit Details: Particularly for claims data, if end dates are not provided assume the visit is for the duration of month that it occurs.<br>
For Inpatient Visit Details ongoing at the date of ETL, put date of processing the data into visit_detai_end_datetime and visit_detail_type_concept_id with 32220 "Still patient" to identify the visit as incomplete.
All other Visits Details: visit_detail_end_datetime = visit_detail_start_datetime."""@en,
        """For Visit Occurrence: For inpatient visits the end date is typically the discharge date.
Visit end dates are mandatory. If end dates are not provided in the source there are three ways in which to derive them:
Outpatient Visit: visit_end_datetime = visit_start_datetime
Emergency Room Visit: visit_end_datetime = visit_start_datetime
Inpatient Visit: Usually there is information about discharge. If not, you should be able to derive the end date from the sudden decline of activity or from the absence of inpatient procedures/drugs.
Non-hospital institution Visits: Particularly for claims data, if end dates are not provided assume the visit is for the duration of month that it occurs.
For Inpatient Visits ongoing at the date of ETL, put date of processing the data into visit_end_datetime and visit_type_concept_id with 32220 "Still patient" to identify the visit as incomplete.
All other Visits: visit_end_datetime = visit_start_datetime. If this is a one-day visit the end date should match the start date."""@en ;
    rdfs:domain omop:DateDuration ;
    rdfs:range xsd:date ;
    omop:omop_cdm_name "cohort.cohort_end_date#426 AS date"^^xsd:string,
        "condition_occurrence.condition_end_date#66 AS date"^^xsd:string,
        "device_exposure.device_exposure_end_date#119 AS date"^^xsd:string,
        "drug_exposure.drug_exposure_end_date#82 AS date"^^xsd:string,
        "location_history.end_date#266 AS date"^^xsd:string,
        "observation_period.observation_period_end_date#23 AS date"^^xsd:string,
        "payer_plan_period.payer_plan_period_end_date#290 AS date"^^xsd:string,
        "visit_detail.visit_detail_end_date#47 AS date"^^xsd:string,
        "visit_occurrence.visit_end_date#30 AS date"^^xsd:string .

omop:end_datetime a owl:DatatypeProperty,
        owl:FunctionalProperty ;
    rdfs:label "End datetime"^^xsd:string ;
    rdfs:comment """For Condition Era: The end date for the Condition Era
constructed from the individual
instances of Condition Occurrences.
It is the end date of the final
continuously recorded instance of the
Condition."""@en,
        "For Condition Occurrence: If a source does not specify datetime the convention is to set the time to midnight (00:00:0000)"@en,
        "For Device Exposure: If a source does not specify datetime the convention is to set the time to midnight (00:00:0000)"@en,
        "For Dose Era: The date the Person was no longer exposed to the dosage of the specific drug ingredient. An era is ended if there are 31 days or more between dosage records."@en,
        """For Drug Era: The Drug Era End Date is the end date of the last Drug Exposure. The End Date of each Drug Exposure is either taken from the field drug_exposure_end_date or, as it is typically not available, inferred using the following rules:
For pharmacy prescription data, the date when the drug was dispensed plus the number of days of supply are used to extrapolate the End Date for the Drug Exposure. Depending on the country-specific healthcare system, this supply information is either explicitly provided in the day_supply field or inferred from package size or similar information.
For Procedure Drugs, usually the drug is administered on a single date (i.e., the administration date).
A standard Persistence Window of 30 days (gap, slack) is permitted between two subsequent such extrapolated DRUG_EXPOSURE records to be considered to be merged into a single Drug Era."""@en,
        "For Drug Exposure: This is not required, though it is in v6. If a source does not specify datetime the convention is to set the time to midnight (00:00:0000)"@en,
        "For Visit Detail: If no time is given for the end date of a visit, set it to midnight (00:00:0000)."@en,
        "For Visit Occurrence: If no time is given for the end date of a visit, set it to midnight (00:00:0000)."@en ;
    rdfs:domain omop:DatetimeDuration ;
    rdfs:range xsd:dateTime ;
    omop:omop_cdm_name "condition_era.condition_era_end_datetime#343 AS datetime"^^xsd:string,
        "condition_occurrence.condition_end_datetime#67 AS datetime"^^xsd:string,
        "device_exposure.device_exposure_end_datetime#120 AS datetime"^^xsd:string,
        "dose_era.dose_era_end_datetime#338 AS datetime"^^xsd:string,
        "drug_era.drug_era_end_datetime#329 AS datetime"^^xsd:string,
        "drug_exposure.drug_exposure_end_datetime#83 AS datetime"^^xsd:string,
        "visit_detail.visit_detail_end_datetime#48 AS datetime"^^xsd:string,
        "visit_occurrence.visit_end_datetime#31 AS datetime"^^xsd:string .

omop:ethnicity_source_value a owl:DatatypeProperty,
        owl:FunctionalProperty ;
    rdfs:label "Ethnicity source value"^^xsd:string ;
    rdfs:comment """For Person: This field is used to store the ethnicity of the person from the source data. It is not intended for use in standard analytics but for reference only.
If the person has an ethnicity other than the OMB standard of "Hispanic" or "Not Hispanic" store that value from the source data here."""@en ;
    rdfs:domain omop:Person ;
    rdfs:range xsd:string ;
    omop:omop_cdm_name "person.ethnicity_source_value#18 AS str"^^xsd:string .

omop:exposure_count a owl:DatatypeProperty,
        owl:FunctionalProperty ;
    rdfs:label "Exposure count"^^xsd:string ;
    rdfs:domain omop:DrugEra ;
    rdfs:range xsd:integer ;
    omop:omop_cdm_name "drug_era.drug_exposure_count#330 AS int"^^xsd:string .

omop:family_source_value a owl:DatatypeProperty,
        owl:FunctionalProperty ;
    rdfs:label "Family source value"^^xsd:string ;
    rdfs:comment """For Payer Plan Period: The common identifier for all people (often a family) that covered by the same policy.
Often these are the common digits of the enrollment id of the policy members."""@en ;
    rdfs:domain omop:PayerPlanPeriod ;
    rdfs:range xsd:string ;
    omop:omop_cdm_name "payer_plan_period.family_source_value#303 AS str"^^xsd:string .

omop:gap_days a owl:DatatypeProperty,
        owl:FunctionalProperty ;
    rdfs:label "Gap days"^^xsd:string ;
    rdfs:comment "For Drug Era: The Gap Days determine how many total drug-free days are observed between all Drug Exposure events that contribute to a DRUG_ERA record. It is assumed that the drugs are \"not stockpiled\" by the patient, i.e. that if a new drug prescription or refill is observed (a new DRUG_EXPOSURE record is written), the remaining supply from the previous events is abandoned.   The difference between Persistence Window and Gap Days is that the former is the maximum drug-free time allowed between two subsequent DRUG_EXPOSURE records, while the latter is the sum of actual drug-free days for the given Drug Era under the above assumption of non-stockpiling."@en ;
    rdfs:domain omop:DrugEra ;
    rdfs:range xsd:integer ;
    omop:omop_cdm_name "drug_era.gap_days#331 AS int"^^xsd:string .

omop:gender_source_value a owl:DatatypeProperty,
        owl:FunctionalProperty ;
    rdfs:label "Gender source value"^^xsd:string ;
    rdfs:comment """For Person: This field is used to store the biological sex of the person from the source data. It is not intended for use in standard analytics but for reference only.
Put the biological sex of the person as it appears in the source data."""@en,
        """For Provider: This is provider's gender as it appears in the source data.
Put the provider's gender as it appears in the source data. This field is up to the discretion of the ETL-er as to whether this should be the coded value from the source or the text description of the lookup value."""@en ;
    rdfs:domain omop:BasePerson ;
    rdfs:range xsd:string ;
    omop:omop_cdm_name "person.gender_source_value#14 AS str"^^xsd:string,
        "provider.gender_source_value#284 AS str"^^xsd:string .

omop:has_amount_unit a owl:FunctionalProperty,
        owl:ObjectProperty ;
    rdfs:label "Has amount unit"^^xsd:string ;
    owlready:python_name "amount_unit"^^xsd:string ;
    rdfs:comment "For Drug Strength: The Concept representing the Unit of measure for the amount of active ingredient contained within the drug product."@en ;
    rdfs:domain omop:DrugStrength ;
    rdfs:range omop:Concept ;
    omop:omop_cdm_name "drug_strength.amount_unit_concept_id#414 AS Concept"^^xsd:string .

omop:has_anatomic_site a owl:FunctionalProperty,
        owl:ObjectProperty ;
    rdfs:label "Has anatomic site"^^xsd:string ;
    owlready:python_name "anatomic_site"^^xsd:string ;
    rdfs:comment """For Specimen: This is the site on the body where the specimen is from.
Map the ANATOMIC_SITE_SOURCE_VALUE to a Standard Concept in the Spec Anatomic Site domain. This should be coded at the lowest level of granularity [Accepted Concepts](https://athena.ohdsi.org/search-terms/terms?standardConcept=Standard&domain=Spec+Anatomic+Site&conceptClass=Body+Structure&page=4&pageSize=15&query=)"""@en ;
    rdfs:domain omop:Specimen ;
    rdfs:range omop:Concept ;
    omop:omop_cdm_name "specimen.anatomic_site_concept_id#215 AS Concept"^^xsd:string .

omop:has_cause a owl:FunctionalProperty,
        owl:ObjectProperty ;
    rdfs:label "Has cause"^^xsd:string ;
    owlready:python_name "cause"^^xsd:string ;
    rdfs:domain omop:Death ;
    rdfs:range omop:Concept ;
    omop:omop_cdm_name "death.cause_concept_id#174 AS Concept"^^xsd:string .

omop:has_cause_source a owl:FunctionalProperty,
        owl:ObjectProperty ;
    rdfs:label "Has cause source"^^xsd:string ;
    owlready:python_name "cause_source"^^xsd:string ;
    rdfs:domain omop:Death ;
    rdfs:range omop:Concept ;
    omop:omop_cdm_name "death.cause_source_concept_id#176 AS Concept"^^xsd:string .

omop:has_contract_person a owl:FunctionalProperty,
        owl:ObjectProperty ;
    rdfs:label "Has contract person"^^xsd:string ;
    owlready:python_name "contract_person"^^xsd:string ;
    rdfs:comment """For Payer Plan Period: The Person who is the primary subscriber/contract owner for Plan.
This may or may not be the same as the PERSON_ID. For example, if a mother has her son on her plan and the PAYER_PLAN_PERIOD record is the for son, the sons's PERSON_ID would go in PAYER_PLAN_PERIOD.PERSON_ID and the mother's PERSON_ID would go in PAYER_PLAN_PERIOD.CONTRACT_PERSON_ID."""@en ;
    rdfs:domain omop:PayerPlanPeriod ;
    rdfs:range omop:Person ;
    omop:omop_cdm_name "payer_plan_period.contract_person_id#288 AS Person"^^xsd:string .

omop:has_currency a owl:FunctionalProperty,
        owl:ObjectProperty ;
    rdfs:label "Has currency"^^xsd:string ;
    owlready:python_name "currency"^^xsd:string ;
    rdfs:comment "For Cost: A foreign key identifier to the concept representing the 3-letter code used to delineate international currencies, such as USD for US Dollar. These belong to the 'Currency' vocabulary"@en ;
    rdfs:domain omop:Cost ;
    rdfs:range omop:Concept ;
    omop:omop_cdm_name "cost.currency_concept_id#315 AS Concept"^^xsd:string .

omop:has_death a owl:ObjectProperty ;
    rdfs:label "Has death"^^xsd:string ;
    owlready:python_name "deaths"^^xsd:string ;
    rdfs:domain omop:Person ;
    rdfs:range omop:Death ;
    omop:omop_cdm_name "death.person_id#170 AS Person"^^xsd:string .

omop:has_denominator_unit a owl:FunctionalProperty,
        owl:ObjectProperty ;
    rdfs:label "Has denominator unit"^^xsd:string ;
    owlready:python_name "denominator_unit"^^xsd:string ;
    rdfs:comment "For Drug Strength: The Concept representing the denominator unit for the concentration of active ingredient."@en ;
    rdfs:domain omop:DrugStrength ;
    rdfs:range omop:Concept ;
    omop:omop_cdm_name "drug_strength.denominator_unit_concept_id#418 AS Concept"^^xsd:string .

omop:has_disease_status a owl:FunctionalProperty,
        owl:ObjectProperty ;
    rdfs:label "Has disease status"^^xsd:string ;
    owlready:python_name "disease_status"^^xsd:string ;
    rdfs:domain omop:Specimen ;
    rdfs:range omop:Concept ;
    omop:omop_cdm_name "specimen.disease_status_concept_id#216 AS Concept"^^xsd:string .

omop:has_drg a owl:FunctionalProperty,
        owl:ObjectProperty ;
    rdfs:label "Has drg"^^xsd:string ;
    owlready:python_name "drg"^^xsd:string ;
    rdfs:comment "For Cost: A foreign key referring to a Standard Concept ID in the Standardized Vocabularies for DRG codes belonging to the 'DRG' vocabulary."@en ;
    rdfs:domain omop:Cost ;
    rdfs:range omop:Concept ;
    omop:omop_cdm_name "cost.drg_concept_id#321 AS Concept"^^xsd:string .

omop:has_modifier a owl:FunctionalProperty,
        owl:ObjectProperty ;
    rdfs:label "Has modifier"^^xsd:string ;
    owlready:python_name "modifier"^^xsd:string ;
    rdfs:comment """For Procedure Occurrence: The modifiers are intended to give additional information about the procedure but as of now the vocabulary is under review.
It is up to the ETL to choose how to map modifiers if they exist in source data. These concepts are typically distinguished by 'Modifier' concept classes (e.g., 'CPT4 Modifier' as part of the 'CPT4' vocabulary). If there is more than one modifier on a record, one should be chosen that pertains to the procedure rather than provider. If not available, set to 0. [Accepted Concepts](https://athena.ohdsi.org/search-terms/terms?conceptClass=CPT4+Modifier&conceptClass=HCPCS+Modifier&vocabulary=CPT4&vocabulary=HCPCS&standardConcept=Standard&page=1&pageSize=15&query=)."""@en ;
    rdfs:domain omop:ProcedureOccurrence ;
    rdfs:range omop:Concept ;
    omop:omop_cdm_name "procedure_occurrence.modifier_concept_id#106 AS Concept"^^xsd:string .

omop:has_numerator_unit a owl:FunctionalProperty,
        owl:ObjectProperty ;
    rdfs:label "Has numerator unit"^^xsd:string ;
    owlready:python_name "numerator_unit"^^xsd:string ;
    rdfs:comment "For Drug Strength: The Concept representing the Unit of measure for the concentration of active ingredient."@en ;
    rdfs:domain omop:DrugStrength ;
    rdfs:range omop:Concept ;
    omop:omop_cdm_name "drug_strength.numerator_unit_concept_id#416 AS Concept"^^xsd:string .

omop:has_obs_event_field a owl:FunctionalProperty,
        owl:ObjectProperty ;
    rdfs:label "Has obs event field"^^xsd:string ;
    owlready:python_name "obs_event_field"^^xsd:string ;
    rdfs:comment """For Observation: If the Observation record is related to another record in the database, this field is the CONCEPT_ID that identifies which table the primary key of the linked record came from.
Put the CONCEPT_ID that identifies which table and field the OBSERVATION_EVENT_ID came from."""@en ;
    rdfs:domain omop:Observation ;
    rdfs:range omop:Concept ;
    omop:omop_cdm_name "observation.obs_event_field_concept_id#168 AS Concept"^^xsd:string .

omop:has_operator a owl:FunctionalProperty,
        owl:ObjectProperty ;
    rdfs:label "Has operator"^^xsd:string ;
    owlready:python_name "operator"^^xsd:string ;
    rdfs:comment """For Measurement: The meaning of Concept [4172703](https://athena.ohdsi.org/search-terms/terms/4172703) for '=' is identical to omission of a OPERATOR_CONCEPT_ID value. Since the use of this field is rare, it's important when devising analyses to not to forget testing for the content of this field for values different from =.
Operators are <, <=, =, >=, > and these concepts belong to the 'Meas Value Operator' domain. [Accepted Concepts](https://athena.ohdsi.org/search-terms/terms?domain=Meas+Value+Operator&standardConcept=Standard&page=1&pageSize=15&query=)."""@en ;
    rdfs:domain omop:Measurement ;
    rdfs:range omop:Concept ;
    omop:omop_cdm_name "measurement.operator_concept_id#136 AS Concept"^^xsd:string .

omop:has_parent a owl:FunctionalProperty,
        owl:ObjectProperty ;
    rdfs:label "Has parent"^^xsd:string ;
    owlready:python_name "parent"^^xsd:string ;
    rdfs:comment """For Visit Detail: Use this field to find the visit detail that subsumes the given visit detail record. This is used in the case that a visit detail record needs to be nested beyond the VISIT_OCCURRENCE/VISIT_DETAIL relationship.
If there are multiple nested levels to how Visits are represented in the source, the VISIT_DETAIL_PARENT_ID can be used to record this relationship."""@en ;
    rdfs:domain omop:VisitDetail ;
    rdfs:range omop:VisitDetail ;
    omop:omop_cdm_name "visit_detail.visit_detail_parent_id#59 AS VisitDetail"^^xsd:string .

omop:has_preceding_visit_detail a owl:FunctionalProperty,
        owl:ObjectProperty ;
    rdfs:label "Has preceding visit detail"^^xsd:string ;
    owlready:python_name "preceding_visit_detail"^^xsd:string ;
    rdfs:comment """For Visit Detail: Use this field to find the visit detail that occurred for the person prior to the given visit detail record. There could be a few days or a few years in between.
The PRECEDING_VISIT_DETAIL_ID can be used to link a visit immediately preceding the current Visit Detail. Note this is not symmetrical, and there is no such thing as a "following_visit_id"."""@en ;
    rdfs:domain omop:VisitDetail ;
    rdfs:range omop:VisitDetail ;
    omop:omop_cdm_name "visit_detail.preceding_visit_detail_id#58 AS VisitDetail"^^xsd:string .

omop:has_preceding_visit_occurrence a owl:FunctionalProperty,
        owl:ObjectProperty ;
    rdfs:label "Has preceding visit occurrence"^^xsd:string ;
    owlready:python_name "preceding_visit_occurrence"^^xsd:string ;
    rdfs:comment """For Visit Occurrence: Use this field to find the visit that occurred for the person prior to the given visit. There could be a few days or a few years in between.
The preceding_visit_id can be used to link a visit immediately preceding the current visit. Note this is not symmetrical, and there is no such thing as a "following_visit_id"."""@en ;
    rdfs:domain omop:VisitOccurrence ;
    rdfs:range omop:VisitOccurrence ;
    omop:omop_cdm_name "visit_occurrence.preceding_visit_occurrence_id#41 AS VisitOccurrence"^^xsd:string .

omop:has_qualifier a owl:FunctionalProperty,
        owl:ObjectProperty ;
    rdfs:label "Has qualifier"^^xsd:string ;
    owlready:python_name "qualifier"^^xsd:string ;
    rdfs:comment """For Observation: This field contains all attributes specifying the clinical fact further, such as as degrees, severities, drug-drug interaction alerts etc.
Use your best judgement as to what Concepts to use here and if they are necessary to accurately represent the clinical record. There is no restriction on the domain of these Concepts, they just need to be Standard."""@en ;
    rdfs:domain omop:Observation ;
    rdfs:range omop:Concept ;
    omop:omop_cdm_name "observation.qualifier_concept_id#158 AS Concept"^^xsd:string .

omop:has_response_visit_occurrence a owl:FunctionalProperty,
        owl:ObjectProperty ;
    rdfs:label "Has response visit occurrence"^^xsd:string ;
    owlready:python_name "response_visit_occurrence"^^xsd:string ;
    rdfs:comment "For Survey Conduct: The Visit during which any treatment related to the Survey was carried out."@en ;
    rdfs:domain omop:SurveyConduct ;
    rdfs:range omop:VisitOccurrence ;
    omop:omop_cdm_name "survey_conduct.response_visit_occurrence_id#250 AS VisitOccurrence"^^xsd:string .

omop:has_revenue_code a owl:FunctionalProperty,
        owl:ObjectProperty ;
    rdfs:label "Has revenue code"^^xsd:string ;
    owlready:python_name "revenue_code"^^xsd:string ;
    rdfs:comment "For Cost: A foreign key referring to a Standard Concept ID in the Standardized Vocabularies for Revenue codes belonging to the 'Revenue Code' vocabulary."@en ;
    rdfs:domain omop:Cost ;
    rdfs:range omop:Concept ;
    omop:omop_cdm_name "cost.revenue_code_concept_id#320 AS Concept"^^xsd:string .

omop:has_route a owl:FunctionalProperty,
        owl:ObjectProperty ;
    rdfs:label "Has route"^^xsd:string ;
    owlready:python_name "route"^^xsd:string ;
    rdfs:comment "For Drug Exposure: The standard CONCEPT_ID that the ROUTE_SOURCE_VALUE maps to in the route domain."@en ;
    rdfs:domain omop:DrugExposure ;
    rdfs:range omop:Concept ;
    omop:omop_cdm_name "drug_exposure.route_concept_id#91 AS Concept"^^xsd:string .

omop:has_section a owl:FunctionalProperty,
        owl:ObjectProperty ;
    rdfs:label "Has section"^^xsd:string ;
    owlready:python_name "section"^^xsd:string ;
    rdfs:comment "For Note Nlp: The SECTION_CONCEPT_ID should be used to represent the note section contained in the NOTE_NLP record. These concepts can be found as parts of document panels and are based on the type of note written, i.e. a discharge summary. These panels can be found as concepts with the relationship 'Subsumes' to CONCEPT_ID [45875957](https://athena.ohdsi.org/search-terms/terms/45875957)."@en ;
    rdfs:domain omop:NoteNlp ;
    rdfs:range omop:Concept ;
    omop:omop_cdm_name "note_nlp.section_concept_id#195 AS Concept"^^xsd:string .

omop:has_sponsor_source a owl:FunctionalProperty,
        owl:ObjectProperty ;
    rdfs:label "Has sponsor source"^^xsd:string ;
    owlready:python_name "sponsor_source"^^xsd:string ;
    rdfs:comment "For Payer Plan Period: If the source data codes the sponsor in an OMOP supported vocabulary store the concept_id here."@en ;
    rdfs:domain omop:PayerPlanPeriod ;
    rdfs:range omop:Concept ;
    omop:omop_cdm_name "payer_plan_period.sponsor_source_concept_id#302 AS Concept"^^xsd:string .

omop:has_stop_reason_concept a owl:FunctionalProperty,
        owl:ObjectProperty ;
    rdfs:label "Has stop reason concept"^^xsd:string ;
    owlready:python_name "stop_reason_concept"^^xsd:string ;
    rdfs:comment """For Payer Plan Period: This field represents the reason the Person left the Plan, if known.
Map the stop reason directly to a standard CONCEPT_ID. If one does not exists please contact the vocabulary team. There is no global controlled vocabulary available for this information. [Accepted Concepts](http://athena.ohdsi.org/search-terms/terms?domain=Plan+Stop+Reason&standardConcept=Standard&page=1&pageSize=15&query=)."""@en ;
    rdfs:domain omop:PayerPlanPeriod ;
    rdfs:range omop:Concept ;
    omop:omop_cdm_name "payer_plan_period.stop_reason_concept_id#304 AS Concept"^^xsd:string .

omop:has_stop_reason_source a owl:FunctionalProperty,
        owl:ObjectProperty ;
    rdfs:label "Has stop reason source"^^xsd:string ;
    owlready:python_name "stop_reason_source"^^xsd:string ;
    rdfs:comment "For Payer Plan Period: If the source data codes the stop reason in an OMOP supported vocabulary store the concept_id here."@en ;
    rdfs:domain omop:PayerPlanPeriod ;
    rdfs:range omop:Concept ;
    omop:omop_cdm_name "payer_plan_period.stop_reason_source_concept_id#306 AS Concept"^^xsd:string .

omop:has_unique_device a owl:FunctionalProperty,
        owl:ObjectProperty ;
    rdfs:label "Has unique device"^^xsd:string ;
    owlready:python_name "unique_device"^^xsd:string ;
    rdfs:comment """For Device Exposure: This is the Unique Device Identification number for devices regulated by the FDA, if given.
For medical devices that are regulated by the FDA, a Unique Device Identification (UDI) is provided if available in the data source and is recorded in the UNIQUE_DEVICE_ID field."""@en ;
    rdfs:domain omop:DeviceExposure ;
    omop:omop_cdm_name "device_exposure.unique_device_id#122 AS Thing"^^xsd:string .

omop:incurred_date a owl:DatatypeProperty,
        owl:FunctionalProperty ;
    rdfs:label "Incurred date"^^xsd:string ;
    rdfs:comment "For Cost: The first date of service of the clinical event corresponding to the cost as in table capturing the information (e.g. date of visit, date of procedure, date of condition, date of drug etc)."@en ;
    rdfs:domain omop:Cost ;
    rdfs:range xsd:date ;
    omop:omop_cdm_name "cost.incurred_date#317 AS date"^^xsd:string .

omop:latitude a owl:DatatypeProperty,
        owl:FunctionalProperty ;
    rdfs:label "Latitude"^^xsd:string ;
    rdfs:comment "For Location: The geocoded latitude."@en ;
    rdfs:domain omop:Location ;
    rdfs:range xsd:decimal ;
    omop:omop_cdm_name "location.latitude#259 AS float"^^xsd:string .

omop:longitude a owl:DatatypeProperty,
        owl:FunctionalProperty ;
    rdfs:label "Longitude"^^xsd:string ;
    rdfs:comment "For Location: The geocoded longitude."@en ;
    rdfs:domain omop:Location ;
    rdfs:range xsd:decimal ;
    omop:omop_cdm_name "location.longitude#260 AS float"^^xsd:string .

omop:lot_number a owl:DatatypeProperty,
        owl:FunctionalProperty ;
    rdfs:label "Lot number"^^xsd:string ;
    rdfs:domain omop:DrugExposure ;
    rdfs:range xsd:string ;
    omop:omop_cdm_name "drug_exposure.lot_number#92 AS str"^^xsd:string .

omop:modifier_source_value a owl:DatatypeProperty,
        owl:FunctionalProperty ;
    rdfs:label "Modifier source value"^^xsd:string ;
    rdfs:comment "For Procedure Occurrence: The original modifier code from the source is stored here for reference."@en ;
    rdfs:domain omop:ProcedureOccurrence ;
    rdfs:range xsd:string ;
    omop:omop_cdm_name "procedure_occurrence.modifier_source_value#113 AS str"^^xsd:string .

omop:month_of_birth a owl:DatatypeProperty,
        owl:FunctionalProperty ;
    rdfs:label "Month of birth"^^xsd:string ;
    rdfs:comment "For Person: For data sources that provide the precise date of birth, the month should be extracted and stored in this field."@en ;
    rdfs:domain omop:Person ;
    rdfs:range xsd:integer ;
    omop:omop_cdm_name "person.month_of_birth#4 AS int"^^xsd:string .

omop:npi a owl:DatatypeProperty,
        owl:FunctionalProperty ;
    rdfs:label "Npi"^^xsd:string ;
    rdfs:comment "For Provider: This is the National Provider Number issued to health care providers in the US by the Centers for Medicare and Medicaid Services (CMS)."@en ;
    rdfs:domain omop:Provider ;
    rdfs:range xsd:string ;
    omop:omop_cdm_name "provider.npi#275 AS str"^^xsd:string .

omop:numerator_value a owl:DatatypeProperty,
        owl:FunctionalProperty ;
    rdfs:label "Numerator value"^^xsd:string ;
    rdfs:comment "For Drug Strength: The concentration of the active ingredient contained within the drug product."@en ;
    rdfs:domain omop:DrugStrength ;
    rdfs:range xsd:decimal ;
    omop:omop_cdm_name "drug_strength.numerator_value#415 AS float"^^xsd:string .

omop:occurrence_count a owl:DatatypeProperty,
        owl:FunctionalProperty ;
    rdfs:label "Occurrence count"^^xsd:string ;
    rdfs:comment """For Condition Era: The number of individual Condition
Occurrences used to construct the
condition era."""@en ;
    rdfs:domain omop:ConditionEra ;
    rdfs:range xsd:integer ;
    omop:omop_cdm_name "condition_era.condition_occurrence_count#344 AS int"^^xsd:string .

omop:offset a owl:DatatypeProperty,
        owl:FunctionalProperty ;
    rdfs:label "Offset"^^xsd:string ;
    rdfs:comment "For Note Nlp: Character offset of the extracted term in the input note"@en ;
    rdfs:domain omop:NoteNlp ;
    rdfs:range xsd:string ;
    omop:omop_cdm_name "note_nlp.offset#197 AS str"^^xsd:string .

omop:paid_date a owl:DatatypeProperty,
        owl:FunctionalProperty ;
    rdfs:label "Paid date"^^xsd:string ;
    rdfs:comment "For Cost: The date payment was received for a service or encounter"@en ;
    rdfs:domain omop:Cost ;
    rdfs:range xsd:date ;
    omop:omop_cdm_name "cost.paid_date#319 AS date"^^xsd:string .

omop:payer_source_value a owl:DatatypeProperty,
        owl:FunctionalProperty ;
    rdfs:label "Payer source value"^^xsd:string ;
    rdfs:comment "For Payer Plan Period: This is the Payer as it appears in the source data."@en ;
    rdfs:domain omop:PayerPlanPeriod ;
    rdfs:range xsd:string ;
    omop:omop_cdm_name "payer_plan_period.payer_source_value#292 AS str"^^xsd:string .

omop:place_of_service_source_value a owl:DatatypeProperty,
        owl:FunctionalProperty ;
    rdfs:label "Place of service source value"^^xsd:string ;
    rdfs:comment "For Care Site: Put the place of service of the care_site as it appears in the source data."@en ;
    rdfs:domain omop:CareSite ;
    rdfs:range xsd:string ;
    omop:omop_cdm_name "care_site.place_of_service_source_value#272 AS str"^^xsd:string .

omop:plan_source_value a owl:DatatypeProperty,
        owl:FunctionalProperty ;
    rdfs:label "Plan source value"^^xsd:string ;
    rdfs:comment "For Payer Plan Period: This is the health benefit Plan of the Person as it appears in the source data."@en ;
    rdfs:domain omop:PayerPlanPeriod ;
    rdfs:range xsd:string ;
    omop:omop_cdm_name "payer_plan_period.plan_source_value#295 AS str"^^xsd:string .

omop:qualifier_source_value a owl:DatatypeProperty,
        owl:FunctionalProperty ;
    rdfs:label "Qualifier source value"^^xsd:string ;
    rdfs:comment """For Observation: This field houses the verbatim value from the source data representing the qualifier of the Observation that occurred.
This code is mapped to a Standard Condition Concept in the Standardized Vocabularies and the original code is stored here for reference."""@en ;
    rdfs:domain omop:Observation ;
    rdfs:range xsd:string ;
    omop:omop_cdm_name "observation.qualifier_source_value#166 AS str"^^xsd:string .

omop:race_source_value a owl:DatatypeProperty,
        owl:FunctionalProperty ;
    rdfs:label "Race source value"^^xsd:string ;
    rdfs:comment """For Person: This field is used to store the race of the person from the source data. It is not intended for use in standard analytics but for reference only.
Put the race of the person as it appears in the source data."""@en ;
    rdfs:domain omop:Person ;
    rdfs:range xsd:string ;
    omop:omop_cdm_name "person.race_source_value#16 AS str"^^xsd:string .

omop:range_high a owl:DatatypeProperty,
        owl:FunctionalProperty ;
    rdfs:label "Range high"^^xsd:string ;
    rdfs:comment """For Measurement: Ranges have the same unit as the VALUE_AS_NUMBER. These ranges are provided by the source and should remain NULL if not given.
If reference ranges for upper and lower limit of normal as provided (typically by a laboratory) these are stored in the RANGE_HIGH and RANGE_LOW fields. This should be set to NULL if not provided."""@en ;
    rdfs:domain omop:Measurement ;
    rdfs:range xsd:decimal ;
    omop:omop_cdm_name "measurement.range_high#141 AS float"^^xsd:string .

omop:range_low a owl:DatatypeProperty,
        owl:FunctionalProperty ;
    rdfs:label "Range low"^^xsd:string ;
    rdfs:comment """For Measurement: Ranges have the same unit as the VALUE_AS_NUMBER. These ranges are provided by the source and should remain NULL if not given.
If reference ranges for upper and lower limit of normal as provided (typically by a laboratory) these are stored in the RANGE_HIGH and RANGE_LOW fields. This should be set to NULL if not provided."""@en ;
    rdfs:domain omop:Measurement ;
    rdfs:range xsd:decimal ;
    omop:omop_cdm_name "measurement.range_low#140 AS float"^^xsd:string .

omop:refills a owl:DatatypeProperty,
        owl:FunctionalProperty ;
    rdfs:label "Refills"^^xsd:string ;
    rdfs:comment "For Drug Exposure: This is only filled in when the record is coming from a prescription written this field is meant to represent intended refills at time of the prescription."@en ;
    rdfs:domain omop:DrugExposure ;
    rdfs:range xsd:integer ;
    omop:omop_cdm_name "drug_exposure.refills#87 AS int"^^xsd:string .

omop:respondent_type_source_value a owl:DatatypeProperty,
        owl:FunctionalProperty ;
    rdfs:label "Respondent type source value"^^xsd:string ;
    rdfs:comment "For Survey Conduct: Source code representing role of person who completed the survey."@en ;
    rdfs:domain omop:SurveyConduct ;
    rdfs:range xsd:string ;
    omop:omop_cdm_name "survey_conduct.respondent_type_source_value#240 AS str"^^xsd:string .

omop:revenue_code_source_value a owl:DatatypeProperty,
        owl:FunctionalProperty ;
    rdfs:label "Revenue code source value"^^xsd:string ;
    rdfs:comment "For Cost: The source value for the Revenue code as it appears in the source data, stored here for reference."@en ;
    rdfs:domain omop:Cost ;
    rdfs:range xsd:string ;
    omop:omop_cdm_name "cost.revenue_code_source_value#322 AS str"^^xsd:string .

omop:route_source_value a owl:DatatypeProperty,
        owl:FunctionalProperty ;
    rdfs:label "Route source value"^^xsd:string ;
    rdfs:comment """For Drug Exposure: This field houses the verbatim value from the source data representing the drug route.
This information may be called something different in the source data but the field is meant to contain a value indicating when and how a drug was given to a patient. This source value is mapped to a standard concept which is stored in the ROUTE_CONCEPT_ID field."""@en ;
    rdfs:domain omop:DrugExposure ;
    rdfs:range xsd:string ;
    omop:omop_cdm_name "drug_exposure.route_source_value#98 AS str"^^xsd:string .

omop:sig a owl:DatatypeProperty,
        owl:FunctionalProperty ;
    rdfs:label "Sig"^^xsd:string ;
    rdfs:comment """For Drug Exposure: This is the verbatim instruction for the drug as written by the provider.
Put the written out instructions for the drug as it is verbatim in the source, if available."""@en ;
    rdfs:domain omop:DrugExposure ;
    rdfs:range xsd:string ;
    omop:omop_cdm_name "drug_exposure.sig#90 AS str"^^xsd:string .

omop:snippet a owl:DatatypeProperty,
        owl:FunctionalProperty ;
    rdfs:label "Snippet"^^xsd:string ;
    rdfs:comment "For Note Nlp: A small window of text surrounding the term"@en ;
    rdfs:domain omop:NoteNlp ;
    rdfs:range xsd:string ;
    omop:omop_cdm_name "note_nlp.snippet#196 AS str"^^xsd:string .

omop:source_code_description a owl:DatatypeProperty,
        owl:FunctionalProperty ;
    rdfs:label "Source code description"^^xsd:string ;
    rdfs:comment """For Source To Concept Map: An optional description for the
source code. This is included as a
convenience to compare the
description of the source code to
the name of the concept."""@en ;
    rdfs:domain omop:SourceToConceptMap ;
    rdfs:range xsd:string ;
    omop:omop_cdm_name "source_to_concept_map.source_code_description#405 AS str"^^xsd:string .

omop:source_description a owl:DatatypeProperty,
        owl:FunctionalProperty ;
    rdfs:label "Source description"^^xsd:string ;
    rdfs:comment "For Cdm Source: The description of the CDM instance."@en ;
    rdfs:domain omop:CdmSource ;
    rdfs:range xsd:string ;
    omop:omop_cdm_name "cdm_source.source_description#355 AS str"^^xsd:string .

omop:source_documentation_reference a owl:DatatypeProperty,
        owl:FunctionalProperty ;
    rdfs:label "Source documentation reference"^^xsd:string ;
    rdfs:domain omop:CdmSource ;
    rdfs:range xsd:string ;
    omop:omop_cdm_name "cdm_source.source_documentation_reference#356 AS str"^^xsd:string .

omop:source_release_date a owl:DatatypeProperty,
        owl:FunctionalProperty ;
    rdfs:label "Source release date"^^xsd:string ;
    rdfs:comment "For Cdm Source: The release date of the source data."@en ;
    rdfs:domain omop:CdmSource ;
    rdfs:range xsd:date ;
    omop:omop_cdm_name "cdm_source.source_release_date#358 AS date"^^xsd:string .

omop:specialty_source_value a owl:DatatypeProperty,
        owl:FunctionalProperty ;
    rdfs:label "Specialty source value"^^xsd:string ;
    rdfs:comment """For Provider: This is the kind of provider or specialty as it appears in the source data. This includes physician specialties such as internal medicine, emergency medicine, etc. and allied health professionals such as nurses, midwives, and pharmacists.
Put the kind of provider as it appears in the source data. This field is up to the discretion of the ETL-er as to whether this should be the coded value from the source or the text description of the lookup value."""@en ;
    rdfs:domain omop:Provider ;
    rdfs:range xsd:string ;
    omop:omop_cdm_name "provider.specialty_source_value#282 AS str"^^xsd:string .

omop:sponsor_source_value a owl:DatatypeProperty,
        owl:FunctionalProperty ;
    rdfs:label "Sponsor source value"^^xsd:string ;
    rdfs:comment "For Payer Plan Period: The Plan sponsor as it appears in the source data."@en ;
    rdfs:domain omop:PayerPlanPeriod ;
    rdfs:range xsd:string ;
    omop:omop_cdm_name "payer_plan_period.sponsor_source_value#301 AS str"^^xsd:string .

omop:standard a owl:DatatypeProperty,
        owl:FunctionalProperty ;
    rdfs:label "Standard"^^xsd:string ;
    rdfs:comment """For Concept: This flag determines where a Concept is
a Standard Concept, i.e. is used in the
data, a Classification Concept, or a
non-standard Source Concept. The
allowable values are 'S' (Standard
Concept) and 'C' (Classification
Concept), otherwise the content is NULL."""@en ;
    rdfs:domain omop:Concept ;
    rdfs:range xsd:string ;
    omop:omop_cdm_name "concept.standard_concept#367 AS str"^^xsd:string .

omop:start_date a owl:DatatypeProperty,
        owl:FunctionalProperty ;
    rdfs:label "Start date"^^xsd:string ;
    rdfs:comment """For Condition Occurrence: Use this date to determine the start date of the condition
Most often data sources do not have the idea of a start date for a condition. Rather, if a source only has one date associated with a condition record it is acceptable to use that date for both the CONDITION_START_DATE and the CONDITION_END_DATE."""@en,
        """For Device Exposure: Use this date to determine the start date of the device record.
Valid entries include a start date of a procedure to implant a device, the date of a prescription for a device, or the date of device administration."""@en,
        """For Drug Exposure: Use this date to determine the start date of the drug record.
Valid entries include a start date of a prescription, the date a prescription was filled, or the date on which a Drug administration was recorded. It is a valid ETL choice to use the date the drug was ordered as the DRUG_EXPOSURE_START_DATE."""@en,
        "For Location History: The date the relationship started"@en,
        """For Observation Period: Use this date to determine the start date of the Observation Period
It is often the case that the idea of Observation Periods does not exist in source data. In those cases, the observation_period_start_date can be inferred as the earliest Event date available for the Person. In insurance claim data, the Observation Period can be considered as the time period the Person is enrolled with a payer. If a Person switches plans but stays with the same payer, and therefore capturing of data continues, that change would be captured in [PAYER_PLAN_PERIOD](https://ohdsi.github.io/CommonDataModel/cdm60.html#payer_plan_period)."""@en,
        "For Payer Plan Period: Start date of Plan coverage."@en,
        """For Visit Detail: This is the date of the start of the encounter. This may or may not be equal to the date of the Visit the Visit Detail is associated with.
When populating visit_start_date, you should think about the patient experience to make decisions on how to define visits. Most likely this should be the date of the patient-provider interaction."""@en,
        """For Visit Occurrence: For inpatient visits, the start date is typically the admission date. For outpatient visits the start date and end date will be the same.
When populating visit_start_date, you should think about the patient experience to make decisions on how to define visits. In the case of an inpatient visit this should be the date the patient was admitted to the hospital or institution. In all other cases this should be the date of the patient-provider interaction."""@en ;
    rdfs:domain omop:DateDuration ;
    rdfs:range xsd:date ;
    omop:omop_cdm_name "cohort.cohort_start_date#425 AS date"^^xsd:string,
        "condition_occurrence.condition_start_date#64 AS date"^^xsd:string,
        "device_exposure.device_exposure_start_date#117 AS date"^^xsd:string,
        "drug_exposure.drug_exposure_start_date#80 AS date"^^xsd:string,
        "location_history.start_date#265 AS date"^^xsd:string,
        "observation_period.observation_period_start_date#22 AS date"^^xsd:string,
        "payer_plan_period.payer_plan_period_start_date#289 AS date"^^xsd:string,
        "visit_detail.visit_detail_start_date#45 AS date"^^xsd:string,
        "visit_occurrence.visit_start_date#28 AS date"^^xsd:string .

omop:start_datetime a owl:DatatypeProperty,
        owl:FunctionalProperty ;
    rdfs:label "Start datetime"^^xsd:string ;
    rdfs:comment """For Condition Era: The start date for the Condition Era
constructed from the individual
instances of Condition Occurrences.
It is the start date of the very first
chronologically recorded instance of
the condition with at least 31 days since any prior record of the same Condition."""@en,
        "For Condition Occurrence: If a source does not specify datetime the convention is to set the time to midnight (00:00:0000)"@en,
        "For Device Exposure: This is not required, though it is in v6. If a source does not specify datetime the convention is to set the time to midnight (00:00:0000)"@en,
        "For Dose Era: The date the Person started on the specific dosage, with at least 31 days since any prior exposure."@en,
        "For Drug Era: The Drug Era Start Date is the start date of the first Drug Exposure for a given ingredient, with at least 31 days since the previous exposure."@en,
        "For Drug Exposure: This is not required, though it is in v6. If a source does not specify datetime the convention is to set the time to midnight (00:00:0000)"@en,
        "For Visit Detail: If no time is given for the start date of a visit, set it to midnight (00:00:0000)."@en,
        "For Visit Occurrence: If no time is given for the start date of a visit, set it to midnight (00:00:0000)."@en ;
    rdfs:domain omop:DatetimeDuration ;
    rdfs:range xsd:dateTime ;
    omop:omop_cdm_name "condition_era.condition_era_start_datetime#342 AS datetime"^^xsd:string,
        "condition_occurrence.condition_start_datetime#65 AS datetime"^^xsd:string,
        "device_exposure.device_exposure_start_datetime#118 AS datetime"^^xsd:string,
        "dose_era.dose_era_start_datetime#337 AS datetime"^^xsd:string,
        "drug_era.drug_era_start_datetime#328 AS datetime"^^xsd:string,
        "drug_exposure.drug_exposure_start_datetime#81 AS datetime"^^xsd:string,
        "visit_detail.visit_detail_start_datetime#46 AS datetime"^^xsd:string,
        "visit_occurrence.visit_start_datetime#29 AS datetime"^^xsd:string .

omop:state a owl:DatatypeProperty,
        owl:FunctionalProperty ;
    rdfs:label "State"^^xsd:string ;
    rdfs:domain omop:Location ;
    rdfs:range xsd:string ;
    omop:omop_cdm_name "location.state#255 AS str"^^xsd:string .

omop:status_source_value a owl:DatatypeProperty,
        owl:FunctionalProperty ;
    rdfs:label "Status source value"^^xsd:string ;
    rdfs:comment """For Condition Occurrence: This field houses the verbatim value from the source data representing the condition status.
This information may be called something different in the source data but the field is meant to contain a value indicating when and how a diagnosis was given to a patient. This source value is mapped to a standard concept which is stored in the CONDITION_STATUS_CONCEPT_ID field."""@en ;
    rdfs:domain omop:ConditionOccurrence ;
    rdfs:range xsd:string ;
    omop:omop_cdm_name "condition_occurrence.condition_status_source_value#76 AS str"^^xsd:string .

omop:stop_reason_source_value a owl:DatatypeProperty,
        owl:FunctionalProperty ;
    rdfs:label "Stop reason source value"^^xsd:string ;
    rdfs:comment "For Payer Plan Period: The Plan stop reason as it appears in the source data."@en ;
    rdfs:domain omop:PayerPlanPeriod ;
    rdfs:range xsd:string ;
    omop:omop_cdm_name "payer_plan_period.stop_reason_source_value#305 AS str"^^xsd:string .

omop:survey_end_date a owl:DatatypeProperty,
        owl:FunctionalProperty ;
    rdfs:label "Survey end date"^^xsd:string ;
    rdfs:comment "For Survey Conduct: Date on which the survey was completed."@en ;
    rdfs:domain omop:SurveyConduct ;
    rdfs:range xsd:date ;
    omop:omop_cdm_name "survey_conduct.survey_end_date#232 AS date"^^xsd:string .

omop:survey_source_identifier a owl:DatatypeProperty,
        owl:FunctionalProperty ;
    rdfs:label "Survey source identifier"^^xsd:string ;
    rdfs:comment "For Survey Conduct: Unique identifier for each completed survey in source system."@en ;
    rdfs:domain omop:SurveyConduct ;
    rdfs:range xsd:string ;
    omop:omop_cdm_name "survey_conduct.survey_source_identifier#245 AS str"^^xsd:string .

omop:survey_source_value a owl:DatatypeProperty,
        owl:FunctionalProperty ;
    rdfs:label "Survey source value"^^xsd:string ;
    rdfs:comment "For Survey Conduct: The survey name as it appears in the source data."@en ;
    rdfs:domain omop:SurveyConduct ;
    rdfs:range xsd:string ;
    omop:omop_cdm_name "survey_conduct.survey_source_value#243 AS str"^^xsd:string .

omop:survey_start_date a owl:DatatypeProperty,
        owl:FunctionalProperty ;
    rdfs:label "Survey start date"^^xsd:string ;
    rdfs:comment "For Survey Conduct: Date on which the survey was started."@en ;
    rdfs:domain omop:SurveyConduct ;
    rdfs:range xsd:date ;
    omop:omop_cdm_name "survey_conduct.survey_start_date#230 AS date"^^xsd:string .

omop:survey_start_datetime a owl:DatatypeProperty,
        owl:FunctionalProperty ;
    rdfs:label "Survey start datetime"^^xsd:string ;
    rdfs:comment "For Survey Conduct: If no time given, set to midnight."@en ;
    rdfs:domain omop:SurveyConduct ;
    rdfs:range xsd:dateTime ;
    omop:omop_cdm_name "survey_conduct.survey_start_datetime#231 AS datetime"^^xsd:string .

omop:survey_version_number a owl:DatatypeProperty,
        owl:FunctionalProperty ;
    rdfs:label "Survey version number"^^xsd:string ;
    rdfs:comment "For Survey Conduct: Version number of the questionnaire or survey used."@en ;
    rdfs:domain omop:SurveyConduct ;
    rdfs:range xsd:string ;
    omop:omop_cdm_name "survey_conduct.survey_version_number#248 AS str"^^xsd:string .

omop:syntax a owl:DatatypeProperty,
        owl:FunctionalProperty ;
    rdfs:label "Syntax"^^xsd:string ;
    rdfs:comment "For Cohort Definition: Syntax or code to operationalize the Cohort Definition."@en ;
    rdfs:domain omop:CohortDefinition ;
    rdfs:range xsd:string ;
    omop:omop_cdm_name "cohort_definition.cohort_definition_syntax#431 AS str"^^xsd:string .

omop:system a owl:DatatypeProperty,
        owl:FunctionalProperty ;
    rdfs:label "System"^^xsd:string ;
    rdfs:comment "For Note Nlp: Name and version of the NLP system that extracted the term. Useful for data provenance."@en ;
    rdfs:domain omop:NoteNlp ;
    rdfs:range xsd:string ;
    omop:omop_cdm_name "note_nlp.nlp_system#201 AS str"^^xsd:string .

omop:term_exists a owl:DatatypeProperty,
        owl:FunctionalProperty ;
    rdfs:label "Term exists"^^xsd:string ;
    rdfs:comment """For Note Nlp: Term_exists is defined as a flag that indicates if the patient actually has or had the condition. Any of the following modifiers would make Term_exists false:
Negation = true
Subject = [anything other than the patient]
Conditional = true/li>
Rule_out = true
Uncertain = very low certainty or any lower certainties
A complete lack of modifiers would make Term_exists true.
"""@en ;
    rdfs:domain omop:NoteNlp ;
    rdfs:range xsd:string ;
    omop:omop_cdm_name "note_nlp.term_exists#204 AS str"^^xsd:string .

omop:term_modifiers a owl:DatatypeProperty,
        owl:FunctionalProperty ;
    rdfs:label "Term modifiers"^^xsd:string ;
    rdfs:comment """For Note Nlp: For the modifiers that are there, they would have to have these values:<br><br>
- Negation = false
- Subject = patient
- Conditional = false
- Rule_out = false
- Uncertain = true or high or moderate or even low (could argue about low). Term_modifiers will concatenate all modifiers for different types of entities (conditions, drugs, labs etc) into one string. Lab values will be saved as one of the modifiers."""@en ;
    rdfs:domain omop:NoteNlp ;
    rdfs:range xsd:string ;
    omop:omop_cdm_name "note_nlp.term_modifiers#206 AS str"^^xsd:string .

omop:term_temporal a owl:DatatypeProperty,
        owl:FunctionalProperty ;
    rdfs:label "Term temporal"^^xsd:string ;
    rdfs:comment """For Note Nlp: Term_temporal is to indicate if a condition is present or just in the past. The following would be past:<br><br>
- History = true
- Concept_date = anything before the time of the report"""@en ;
    rdfs:domain omop:NoteNlp ;
    rdfs:range xsd:string ;
    omop:omop_cdm_name "note_nlp.term_temporal#205 AS str"^^xsd:string .

omop:time a owl:DatatypeProperty,
        owl:FunctionalProperty ;
    rdfs:label "Time"^^xsd:string ;
    rdfs:comment "For Measurement: This is present for backwards compatibility and will be deprecated in an upcoming version."@en ;
    rdfs:domain omop:Measurement ;
    rdfs:range xsd:string ;
    omop:omop_cdm_name "measurement.measurement_time#134 AS str"^^xsd:string .

omop:timing_source_value a owl:DatatypeProperty,
        owl:FunctionalProperty ;
    rdfs:label "Timing source value"^^xsd:string ;
    rdfs:comment "For Survey Conduct: Text string representing the timing of the survey. Example: Baseline, 6-month follow-up."@en ;
    rdfs:domain omop:SurveyConduct ;
    rdfs:range xsd:string ;
    omop:omop_cdm_name "survey_conduct.timing_source_value#241 AS str"^^xsd:string .

omop:title a owl:DatatypeProperty,
        owl:FunctionalProperty ;
    rdfs:label "Title"^^xsd:string ;
    rdfs:comment "For Note: The title of the note."@en ;
    rdfs:domain omop:Note ;
    rdfs:range xsd:string ;
    omop:omop_cdm_name "note.note_title#185 AS str"^^xsd:string .

omop:validated_survey_source_value a owl:DatatypeProperty,
        owl:FunctionalProperty ;
    rdfs:label "Validated survey source value"^^xsd:string ;
    rdfs:comment "For Survey Conduct: Source value representing the validation status of the survey."@en ;
    rdfs:domain omop:SurveyConduct ;
    rdfs:range xsd:integer ;
    omop:omop_cdm_name "survey_conduct.validated_survey_source_value#247 AS int"^^xsd:string .

omop:value_as_datetime a owl:DatatypeProperty,
        owl:FunctionalProperty ;
    rdfs:label "Value as datetime"^^xsd:string ;
    rdfs:comment "For Observation: It is possible that some Observation records might store a result as a date value."@en ;
    rdfs:domain omop:Observation ;
    rdfs:range xsd:dateTime ;
    omop:omop_cdm_name "observation.value_as_datetime#169 AS datetime"^^xsd:string .

omop:value_source_value a owl:DatatypeProperty,
        owl:FunctionalProperty ;
    rdfs:label "Value source value"^^xsd:string ;
    rdfs:comment """For Measurement: This field houses the verbatim result value of the Measurement from the source data .
If both a continuous and categorical result are given in the source data such that both VALUE_AS_NUMBER and VALUE_AS_CONCEPT_ID are both included, store the verbatim value that was mapped to VALUE_AS_CONCEPT_ID here."""@en ;
    rdfs:domain omop:Measurement ;
    rdfs:range xsd:string ;
    omop:omop_cdm_name "measurement.value_source_value#148 AS str"^^xsd:string .

omop:verbatim_end_date a owl:DatatypeProperty,
        owl:FunctionalProperty ;
    rdfs:label "Verbatim end date"^^xsd:string ;
    rdfs:comment """For Drug Exposure: This is the end date of the drug exposure as it appears in the source data, if it is given
Put the end date or discontinuation date as it appears from the source data or leave blank if unavailable."""@en ;
    rdfs:domain omop:DrugExposure ;
    rdfs:range xsd:date ;
    omop:omop_cdm_name "drug_exposure.verbatim_end_date#84 AS date"^^xsd:string .

omop:version a owl:DatatypeProperty,
        owl:FunctionalProperty ;
    rdfs:label "Version"^^xsd:string ;
    rdfs:comment """For Vocabulary: Version of the Vocabulary as indicated in
the source."""@en ;
    rdfs:domain omop:Vocabulary ;
    rdfs:range xsd:string ;
    omop:omop_cdm_name "vocabulary.vocabulary_version#375 AS str"^^xsd:string .

omop:vocabulary_version a owl:DatatypeProperty,
        owl:FunctionalProperty ;
    rdfs:label "Vocabulary version"^^xsd:string ;
    rdfs:domain omop:CdmSource ;
    rdfs:range xsd:string ;
    omop:omop_cdm_name "cdm_source.vocabulary_version#361 AS str"^^xsd:string .

omop:zip a owl:DatatypeProperty,
        owl:FunctionalProperty ;
    rdfs:label "Zip"^^xsd:string ;
    rdfs:comment "For Location: Zip codes are handled as strings of up to 9 characters length. For US addresses, these represent either a 3-digit abbreviated Zip code as provided by many sources for patient protection reasons, the full 5-digit Zip or the 9-digit (ZIP + 4) codes. Unless for specific reasons analytical methods should expect and utilize only the first 3 digits. For international addresses, different rules apply."@en ;
    rdfs:domain omop:Location ;
    rdfs:range xsd:string ;
    omop:omop_cdm_name "location.zip#256 AS str"^^xsd:string .

omop:Cohort a owl:Class ;
    rdfs:label "Cohort"^^xsd:string ;
    rdfs:comment "The COHORT table contains records of subjects that satisfy a given set of criteria for a duration of time. The definition of the cohort is contained within the COHORT_DEFINITION table. It is listed as part of the RESULTS schema because it is a table that users of the database as well as tools such as ATLAS need to be able to write to. The CDM and Vocabulary tables are all read-only so it is suggested that the COHORT and COHORT_DEFINTION tables are kept in a separate schema to alleviate confusion."@en ;
    rdfs:subClassOf [ a owl:Restriction ;
            owl:allValuesFrom omop:CohortDefinition ;
            owl:onProperty omop:has_definition ],
        [ a owl:Restriction ;
            owl:onProperty omop:has_definition ;
            owl:someValuesFrom omop:CohortDefinition ],
        [ a owl:Restriction ;
            owl:allValuesFrom owl:Thing ;
            owl:onProperty omop:has_subject ],
        [ a owl:Restriction ;
            owl:onProperty omop:has_subject ;
            owl:someValuesFrom owl:Thing ],
        omop:DateDuration ;
    omop:omop_cdm_name "cohort"^^xsd:string .

omop:Duration a owl:Class ;
    rdfs:label "Duration"^^xsd:string ;
    rdfs:subClassOf omop:OmopCDMThing .

omop:code a owl:DatatypeProperty,
        owl:FunctionalProperty ;
    rdfs:label "Code"^^xsd:string ;
    rdfs:comment """For Concept: The concept code represents the identifier
of the Concept in the source vocabulary,
such as SNOMED-CT concept IDs,
RxNorm RXCUIs etc. Note that concept
codes are not unique across vocabularies."""@en ;
    rdfs:domain omop:Concept ;
    rdfs:range xsd:string ;
    omop:omop_cdm_name "concept.concept_code#368 AS str"^^xsd:string .

omop:concept_id_1 a owl:DatatypeProperty,
        owl:FunctionalProperty ;
    rdfs:label "Concept id 1"^^xsd:string ;
    rdfs:domain omop:ConceptRelationship ;
    rdfs:range xsd:integer ;
    omop:omop_cdm_name "concept_relationship.concept_id_1#383 AS int"^^xsd:string .

omop:concept_id_2 a owl:DatatypeProperty,
        owl:FunctionalProperty ;
    rdfs:label "Concept id 2"^^xsd:string ;
    rdfs:domain omop:ConceptRelationship ;
    rdfs:range xsd:integer ;
    omop:omop_cdm_name "concept_relationship.concept_id_2#384 AS int"^^xsd:string .

omop:contract_source_value a owl:DatatypeProperty,
        owl:FunctionalProperty ;
    rdfs:label "Contract source value"^^xsd:string ;
    rdfs:comment "For Payer Plan Period: This is the relationship of the PERSON_ID to CONTRACT_PERSON_ID as it appears in the source data."@en ;
    rdfs:domain omop:PayerPlanPeriod ;
    rdfs:range xsd:string ;
    omop:omop_cdm_name "payer_plan_period.contract_source_value#298 AS str"^^xsd:string .

omop:defines_ancestry a owl:DatatypeProperty,
        owl:FunctionalProperty ;
    rdfs:label "Defines ancestry"^^xsd:string ;
    rdfs:domain omop:Relationship ;
    rdfs:range xsd:string ;
    omop:omop_cdm_name "relationship.defines_ancestry#392 AS str"^^xsd:string .

omop:domain_concept_id_1 a owl:DatatypeProperty,
        owl:FunctionalProperty ;
    rdfs:label "Domain concept id 1"^^xsd:string ;
    rdfs:domain omop:FactRelationship ;
    rdfs:range xsd:integer ;
    omop:omop_cdm_name "fact_relationship.domain_concept_id_1#222 AS int"^^xsd:string .

omop:domain_concept_id_2 a owl:DatatypeProperty,
        owl:FunctionalProperty ;
    rdfs:label "Domain concept id 2"^^xsd:string ;
    rdfs:domain omop:FactRelationship ;
    rdfs:range xsd:integer ;
    omop:omop_cdm_name "fact_relationship.domain_concept_id_2#224 AS int"^^xsd:string .

omop:fact_id_1 a owl:DatatypeProperty,
        owl:FunctionalProperty ;
    rdfs:label "Fact id 1"^^xsd:string ;
    rdfs:domain omop:FactRelationship ;
    rdfs:range xsd:integer ;
    omop:omop_cdm_name "fact_relationship.fact_id_1#223 AS int"^^xsd:string .

omop:fact_id_2 a owl:DatatypeProperty,
        owl:FunctionalProperty ;
    rdfs:label "Fact id 2"^^xsd:string ;
    rdfs:domain omop:FactRelationship ;
    rdfs:range xsd:integer ;
    omop:omop_cdm_name "fact_relationship.fact_id_2#225 AS int"^^xsd:string .

omop:has_ancestor a owl:FunctionalProperty,
        owl:ObjectProperty ;
    rdfs:label "Has ancestor"^^xsd:string ;
    owlready:python_name "ancestor"^^xsd:string ;
    rdfs:comment """For Concept Ancestor: The Concept Id for the higher-level concept
that forms the ancestor in the relationship."""@en ;
    rdfs:domain omop:ConceptAncestor ;
    rdfs:range omop:Concept ;
    omop:omop_cdm_name "concept_ancestor.ancestor_concept_id#398 AS Concept"^^xsd:string .

omop:has_assisted a owl:FunctionalProperty,
        owl:ObjectProperty ;
    rdfs:label "Has assisted"^^xsd:string ;
    owlready:python_name "assisted"^^xsd:string ;
    rdfs:comment """For Survey Conduct: This is a Concept that represents whether the survey was completed with assistance or independently.
There is no specific domain or class for this field, just choose the one that best represents the value given in the source."""@en ;
    rdfs:domain omop:SurveyConduct ;
    rdfs:range omop:Concept ;
    omop:omop_cdm_name "survey_conduct.assisted_concept_id#235 AS Concept"^^xsd:string .

omop:has_care_site a owl:FunctionalProperty,
        owl:ObjectProperty ;
    rdfs:label "Has care site"^^xsd:string ;
    owlready:python_name "care_site"^^xsd:string ;
    rdfs:comment "For Person: The Care Site refers to where the Provider typically provides the primary care."@en,
        """For Provider: This is the CARE_SITE_ID for the location that the provider primarily practices in.
If a Provider has more than one Care Site, the main or most often exerted CARE_SITE_ID should be recorded."""@en,
        """For Visit Detail: This field provides information about the Care Site where the Visit Detail took place.
There should only be one Care Site associated with a Visit Detail."""@en,
        """For Visit Occurrence: This field provides information about the care site where the visit took place.
There should only be one care site associated with a visit."""@en ;
    rdfs:domain [ a owl:Class ;
            owl:unionOf ( omop:BaseVisit omop:BasePerson ) ] ;
    rdfs:range omop:CareSite ;
    omop:omop_cdm_name "person.care_site_id#12 AS CareSite"^^xsd:string,
        "provider.care_site_id#278 AS CareSite"^^xsd:string,
        "visit_detail.care_site_id#51 AS CareSite"^^xsd:string,
        "visit_occurrence.care_site_id#34 AS CareSite"^^xsd:string .

omop:has_collection_method a owl:FunctionalProperty,
        owl:ObjectProperty ;
    rdfs:label "Has collection method"^^xsd:string ;
    owlready:python_name "collection_method"^^xsd:string ;
    rdfs:comment """For Survey Conduct: This Concept represents how the responses were collected.
Use the concepts that have the relationship 'Has Answer' with the CONCEPT_ID [42529316](https://athena.ohdsi.org/search-terms/terms/42529316)."""@en ;
    rdfs:domain omop:SurveyConduct ;
    rdfs:range omop:Concept ;
    omop:omop_cdm_name "survey_conduct.collection_method_concept_id#238 AS Concept"^^xsd:string .

omop:has_condition_era a owl:ObjectProperty ;
    rdfs:label "Has condition era"^^xsd:string ;
    owlready:python_name "condition_eras"^^xsd:string ;
    rdfs:domain omop:Person ;
    rdfs:range omop:ConditionEra ;
    omop:omop_cdm_name "condition_era.person_id#340 AS Person"^^xsd:string .

omop:has_contract a owl:FunctionalProperty,
        owl:ObjectProperty ;
    rdfs:label "Has contract"^^xsd:string ;
    owlready:python_name "contract"^^xsd:string ;
    rdfs:comment """For Payer Plan Period: This field represents the relationship between the PERSON_ID and CONTRACT_PERSON_ID. It should be read as PERSON_ID is the *CONTRACT_CONCEPT_ID* of the CONTRACT_PERSON_ID. So if CONTRACT_CONCEPT_ID represents the relationship 'Stepdaughter' then the Person for whom PAYER_PLAN_PERIOD record was recorded is the stepdaughter of the CONTRACT_PERSON_ID.
If available, use this field to represent the relationship between the PERSON_ID and the CONTRACT_PERSON_ID. If the Person for whom the PAYER_PLAN_PERIOD record was recorded is the stepdaughter of the CONTRACT_PERSON_ID then CONTRACT_CONCEPT_ID would be [4330864](https://athena.ohdsi.org/search-terms/terms/4330864). If not available, set to 0. [Accepted Concepts](https://athena.ohdsi.org/search-terms/terms?standardConcept=Standard&domain=Relationship&page=12&pageSize=15&query=)."""@en ;
    rdfs:domain omop:PayerPlanPeriod ;
    rdfs:range omop:Concept ;
    omop:omop_cdm_name "payer_plan_period.contract_concept_id#297 AS Concept"^^xsd:string .

omop:has_contract_source a owl:FunctionalProperty,
        owl:ObjectProperty ;
    rdfs:label "Has contract source"^^xsd:string ;
    owlready:python_name "contract_source"^^xsd:string ;
    rdfs:comment "For Payer Plan Period: If the source data codes the relationship between the PERSON_ID and CONTRACT_PERSON_ID in an OMOP supported vocabulary store the concept_id here. If not available, set to 0."@en ;
    rdfs:domain omop:PayerPlanPeriod ;
    rdfs:range omop:Concept ;
    omop:omop_cdm_name "payer_plan_period.contract_source_concept_id#299 AS Concept"^^xsd:string .

omop:has_cost a owl:ObjectProperty ;
    rdfs:label "Has cost"^^xsd:string ;
    owlready:python_name "costs"^^xsd:string ;
    rdfs:domain omop:Person ;
    rdfs:range omop:Cost ;
    omop:omop_cdm_name "cost.person_id#308 AS Person"^^xsd:string .

omop:has_definition a owl:FunctionalProperty,
        owl:ObjectProperty ;
    rdfs:label "Has definition"^^xsd:string ;
    owlready:python_name "definition"^^xsd:string ;
    rdfs:domain omop:Cohort ;
    rdfs:range omop:CohortDefinition ;
    omop:omop_cdm_name "cohort.cohort_definition_id#423 AS CohortDefinition"^^xsd:string .

omop:has_definition_type a owl:FunctionalProperty,
        owl:ObjectProperty ;
    rdfs:label "Has definition type"^^xsd:string ;
    owlready:python_name "definition_type"^^xsd:string ;
    rdfs:comment "For Cohort Definition: Type defining what kind of Cohort Definition the record represents and how the syntax may be executed."@en ;
    rdfs:domain omop:CohortDefinition ;
    rdfs:range omop:Concept ;
    omop:omop_cdm_name "cohort_definition.definition_type_concept_id#430 AS Concept"^^xsd:string .

omop:has_descendant a owl:FunctionalProperty,
        owl:ObjectProperty ;
    rdfs:label "Has descendant"^^xsd:string ;
    owlready:python_name "descendant"^^xsd:string ;
    rdfs:comment """For Concept Ancestor: The Concept Id for the lower-level concept
that forms the descendant in the
relationship."""@en ;
    rdfs:domain omop:ConceptAncestor ;
    rdfs:range omop:Concept ;
    omop:omop_cdm_name "concept_ancestor.descendant_concept_id#399 AS Concept"^^xsd:string .

omop:has_discharge_to a owl:FunctionalProperty,
        owl:ObjectProperty ;
    rdfs:label "Has discharge to"^^xsd:string ;
    owlready:python_name "discharge_to"^^xsd:string ;
    rdfs:comment """For Visit Detail: Use this field to determine where the patient was discharged to after a visit detail record. This concept is part of the visit domain and can indicate if a patient was discharged to home or sent to a long-term care facility, for example.
If available, map the DISCHARGE_TO_SOURCE_VALUE to a Standard Concept in the Visit domain. If not available, set to 0. [Accepted Concepts](https://athena.ohdsi.org/search-terms/terms?domain=Visit&standardConcept=Standard&page=1&pageSize=15&query=)."""@en,
        """For Visit Occurrence: Use this field to determine where the patient was discharged to after a visit. This concept is part of the visit domain and can indicate if a patient was discharged to home or sent to a long-term care facility, for example.
If available, map the discharge_to_source_value to a standard concept in the visit domain. If not available set to 0."""@en ;
    rdfs:domain omop:BaseVisit ;
    rdfs:range omop:Concept ;
    omop:omop_cdm_name "visit_detail.discharge_to_concept_id#57 AS Concept"^^xsd:string,
        "visit_occurrence.discharge_to_concept_id#39 AS Concept"^^xsd:string .

omop:has_dose_era a owl:ObjectProperty ;
    rdfs:label "Has dose era"^^xsd:string ;
    owlready:python_name "dose_eras"^^xsd:string ;
    rdfs:domain omop:Person ;
    rdfs:range omop:DoseEra ;
    omop:omop_cdm_name "dose_era.person_id#333 AS Person"^^xsd:string .

omop:has_drug_era a owl:ObjectProperty ;
    rdfs:label "Has drug era"^^xsd:string ;
    owlready:python_name "drug_eras"^^xsd:string ;
    rdfs:domain omop:Person ;
    rdfs:range omop:DrugEra ;
    omop:omop_cdm_name "drug_era.person_id#326 AS Person"^^xsd:string .

omop:has_encoding a owl:FunctionalProperty,
        owl:ObjectProperty ;
    rdfs:label "Has encoding"^^xsd:string ;
    owlready:python_name "encoding"^^xsd:string ;
    rdfs:comment """For Note: This is the Concept representing the character encoding type.
Put the Concept Id that represents the encoding character type here. Currently the only option is UTF-8 ([32678](https://athena.ohdsi.org/search-terms/terms/32678)). It the note is encoded in any other type, like ASCII then put 0."""@en ;
    rdfs:domain omop:Note ;
    rdfs:range omop:Concept ;
    omop:omop_cdm_name "note.encoding_concept_id#187 AS Concept"^^xsd:string .

omop:has_entity a owl:FunctionalProperty,
        owl:ObjectProperty ;
    rdfs:label "Has entity"^^xsd:string ;
    owlready:python_name "entity"^^xsd:string ;
    rdfs:comment "For Location History: The unique identifier for the entity. References either person_id, provider_id, or care_site_id, depending on domain_id."@en ;
    rdfs:domain omop:LocationHistory ;
    omop:omop_cdm_name "location_history.entity_id#264 AS Thing"^^xsd:string .

omop:has_ethnicity a owl:FunctionalProperty,
        owl:ObjectProperty ;
    rdfs:label "Has ethnicity"^^xsd:string ;
    owlready:python_name "ethnicity"^^xsd:string ;
    rdfs:comment """For Person: This field captures Ethnicity as defined by the Office of Management and Budget (OMB) of the US Government: it distinguishes only between "Hispanic" and "Not Hispanic". Races and ethnic backgrounds are not stored here.
Only use this field if you have US-based data and a source of this information. Do not attempt to infer Ethnicity from the race or ethnic background of the Person. [Accepted ethnicity concepts](http://athena.ohdsi.org/search-terms/terms?domain=Ethnicity&standardConcept=Standard&page=1&pageSize=15&query=)"""@en ;
    rdfs:domain omop:Person ;
    rdfs:range omop:Concept ;
    omop:omop_cdm_name "person.ethnicity_concept_id#9 AS Concept"^^xsd:string .

omop:has_ethnicity_source a owl:FunctionalProperty,
        owl:ObjectProperty ;
    rdfs:label "Has ethnicity source"^^xsd:string ;
    owlready:python_name "ethnicity_source"^^xsd:string ;
    rdfs:comment """For Person: Due to the small number of options, this tends to be zero.
If the source data codes ethnicity in an OMOP supported vocabulary, store the concept_id here, otherwise set to 0."""@en ;
    rdfs:domain omop:Person ;
    rdfs:range omop:Concept ;
    omop:omop_cdm_name "person.ethnicity_source_concept_id#19 AS Concept"^^xsd:string .

omop:has_gender a owl:FunctionalProperty,
        owl:ObjectProperty ;
    rdfs:label "Has gender"^^xsd:string ;
    owlready:python_name "gender"^^xsd:string ;
    rdfs:comment """For Person: This field is meant to capture the biological sex at birth of the Person. This field should not be used to study gender identity issues.
Use the gender or sex value present in the data under the assumption that it is the biological sex at birth. If the source data captures gender identity it should be stored in the [OBSERVATION](https://ohdsi.github.io/CommonDataModel/cdm60.html#observation) table. [Accepted gender concepts](http://athena.ohdsi.org/search-terms/terms?domain=Gender&standardConcept=Standard&page=1&pageSize=15&query=)"""@en,
        """For Provider: This field represents the recorded gender of the provider in the source data.
If given, put a concept from the gender domain representing the recorded gender of the provider. If not available, set to 0. [Accepted Concepts](http://athena.ohdsi.org/search-terms/terms?domain=Gender&standardConcept=Standard&page=1&pageSize=15&query=)."""@en ;
    rdfs:domain omop:BasePerson ;
    rdfs:range omop:Concept ;
    omop:omop_cdm_name "person.gender_concept_id#2 AS Concept"^^xsd:string,
        "provider.gender_concept_id#280 AS Concept"^^xsd:string .

omop:has_gender_source a owl:FunctionalProperty,
        owl:ObjectProperty ;
    rdfs:label "Has gender source"^^xsd:string ;
    owlready:python_name "gender_source"^^xsd:string ;
    rdfs:comment """For Person: Due to the small number of options, this tends to be zero.
If the source data codes biological sex in a non-standard vocabulary, store the concept_id here, otherwise set to 0."""@en,
        """For Provider: This is often zero as many sites use proprietary codes to store provider gender.
If the source data codes provider gender in an OMOP supported vocabulary store the concept_id here. If not available, set to 0."""@en ;
    rdfs:domain omop:BasePerson ;
    rdfs:range omop:Concept ;
    omop:omop_cdm_name "person.gender_source_concept_id#15 AS Concept"^^xsd:string,
        "provider.gender_source_concept_id#285 AS Concept"^^xsd:string .

omop:has_ingredient a owl:FunctionalProperty,
        owl:ObjectProperty ;
    rdfs:label "Has ingredient"^^xsd:string ;
    owlready:python_name "ingredient"^^xsd:string ;
    rdfs:comment """For Drug Strength: The Concept representing the active ingredient contained within the drug product.
Combination Drugs will have more than one record in this table, one for each active Ingredient."""@en ;
    rdfs:domain omop:DrugStrength ;
    rdfs:range omop:Concept ;
    omop:omop_cdm_name "drug_strength.ingredient_concept_id#412 AS Concept"^^xsd:string .

omop:has_note_nlp a owl:ObjectProperty ;
    rdfs:label "Has note nlp"^^xsd:string ;
    owlready:python_name "note_nlps"^^xsd:string ;
    rdfs:comment "reversed relation, For Note Nlp: This is the NOTE_ID for the NOTE record the NLP record is associated to."@en ;
    rdfs:domain omop:Note ;
    rdfs:range omop:NoteNlp ;
    omop:omop_cdm_name "note_nlp.note_id#194 AS Note"^^xsd:string .

omop:has_observation_period a owl:ObjectProperty ;
    rdfs:label "Has observation period"^^xsd:string ;
    owlready:python_name "observation_periods"^^xsd:string ;
    rdfs:comment "reversed relation, For Observation Period: The Person ID of the PERSON record for which the Observation Period is recorded."@en ;
    rdfs:domain omop:Person ;
    rdfs:range omop:ObservationPeriod ;
    omop:omop_cdm_name "observation_period.person_id#21 AS Person"^^xsd:string .

omop:has_payer a owl:FunctionalProperty,
        owl:ObjectProperty ;
    rdfs:label "Has payer"^^xsd:string ;
    owlready:python_name "payer"^^xsd:string ;
    rdfs:comment """For Payer Plan Period: This field represents the organization who reimburses the provider which administers care to the Person.
Map the Payer directly to a standard CONCEPT_ID. If one does not exists please contact the vocabulary team. There is no global controlled vocabulary available for this information. The point is to stratify on this information and identify if Persons have the same payer, though the name of the Payer is not necessary. If not available, set to 0. [Accepted Concepts](http://athena.ohdsi.org/search-terms/terms?domain=Payer&standardConcept=Standard&page=1&pageSize=15&query=)."""@en ;
    rdfs:domain omop:PayerPlanPeriod ;
    rdfs:range omop:Concept ;
    omop:omop_cdm_name "payer_plan_period.payer_concept_id#291 AS Concept"^^xsd:string .

omop:has_payer_source a owl:FunctionalProperty,
        owl:ObjectProperty ;
    rdfs:label "Has payer source"^^xsd:string ;
    owlready:python_name "payer_source"^^xsd:string ;
    rdfs:comment "For Payer Plan Period: If the source data codes the Payer in an OMOP supported vocabulary store the concept_id here. If not available, set to 0."@en ;
    rdfs:domain omop:PayerPlanPeriod ;
    rdfs:range omop:Concept ;
    omop:omop_cdm_name "payer_plan_period.payer_source_concept_id#293 AS Concept"^^xsd:string .

omop:has_period_type a owl:FunctionalProperty,
        owl:ObjectProperty ;
    rdfs:label "Has period type"^^xsd:string ;
    owlready:python_name "period_type"^^xsd:string ;
    rdfs:comment """For Observation Period: This field can be used to determine the provenance of the Observation Period as in whether the period was determined from an insurance enrollment file, EHR healthcare encounters, or other sources.
Choose the observation_period_type_concept_id that best represents how the period was determined. [Accepted Concepts](https://athena.ohdsi.org/search-terms/terms?domain=Type+Concept&standardConcept=Standard&page=1&pageSize=15&query=)."""@en ;
    rdfs:domain omop:ObservationPeriod ;
    rdfs:range omop:Concept ;
    omop:omop_cdm_name "observation_period.period_type_concept_id#24 AS Concept"^^xsd:string .

omop:has_place_of_service a owl:FunctionalProperty,
        owl:ObjectProperty ;
    rdfs:label "Has place of service"^^xsd:string ;
    owlready:python_name "place_of_service"^^xsd:string ;
    rdfs:comment """For Care Site: This is a high-level way of characterizing a Care Site. Typically, however, Care Sites can provide care in multiple settings (inpatient, outpatient, etc.) and this granularity should be reflected in the visit.
Choose the concept in the visit domain that best represents the setting in which healthcare is provided in the Care Site. If most visits in a Care Site are Inpatient, then the place_of_service_concept_id should represent Inpatient. If information is present about a unique Care Site (e.g. Pharmacy) then a Care Site record should be created. If this information is not available then set to 0. [Accepted Concepts](https://athena.ohdsi.org/search-terms/terms?domain=Visit&standardConcept=Standard&page=2&pageSize=15&query=)."""@en ;
    rdfs:domain omop:CareSite ;
    rdfs:range omop:Concept ;
    omop:omop_cdm_name "care_site.place_of_service_concept_id#269 AS Concept"^^xsd:string .

omop:has_plan a owl:FunctionalProperty,
        owl:ObjectProperty ;
    rdfs:label "Has plan"^^xsd:string ;
    owlready:python_name "plan"^^xsd:string ;
    rdfs:comment """For Payer Plan Period: This field represents the specific health benefit Plan the Person is enrolled in.
Map the Plan directly to a standard CONCEPT_ID. If one does not exists please contact the vocabulary team. There is no global controlled vocabulary available for this information. The point is to stratify on this information and identify if Persons have the same health benefit Plan though the name of the Plan is not necessary. If not available, set to 0. [Accepted Concepts](http://athena.ohdsi.org/search-terms/terms?domain=Plan&standardConcept=Standard&page=1&pageSize=15&query=)."""@en ;
    rdfs:domain omop:PayerPlanPeriod ;
    rdfs:range omop:Concept ;
    omop:omop_cdm_name "payer_plan_period.plan_concept_id#294 AS Concept"^^xsd:string .

omop:has_plan_source a owl:FunctionalProperty,
        owl:ObjectProperty ;
    rdfs:label "Has plan source"^^xsd:string ;
    owlready:python_name "plan_source"^^xsd:string ;
    rdfs:comment "For Payer Plan Period: If the source data codes the Plan in an OMOP supported vocabulary store the concept_id here. If not available, set to 0."@en ;
    rdfs:domain omop:PayerPlanPeriod ;
    rdfs:range omop:Concept ;
    omop:omop_cdm_name "payer_plan_period.plan_source_concept_id#296 AS Concept"^^xsd:string .

omop:has_race a owl:FunctionalProperty,
        owl:ObjectProperty ;
    rdfs:label "Has race"^^xsd:string ;
    owlready:python_name "race"^^xsd:string ;
    rdfs:comment """For Person: This field captures race or ethnic background of the person.
Only use this field if you have information about race or ethnic background. The Vocabulary contains Concepts about the main races and ethnic backgrounds in a hierarchical system. Due to the imprecise nature of human races and ethnic backgrounds, this is not a perfect system. Mixed races are not supported. If a clear race or ethnic background cannot be established, use Concept_Id 0. [Accepted Race Concepts](http://athena.ohdsi.org/search-terms/terms?domain=Race&standardConcept=Standard&page=1&pageSize=15&query=)."""@en ;
    rdfs:domain omop:Person ;
    rdfs:range omop:Concept ;
    omop:omop_cdm_name "person.race_concept_id#8 AS Concept"^^xsd:string .

omop:has_race_source a owl:FunctionalProperty,
        owl:ObjectProperty ;
    rdfs:label "Has race source"^^xsd:string ;
    owlready:python_name "race_source"^^xsd:string ;
    rdfs:comment """For Person: Due to the small number of options, this tends to be zero.
If the source data codes race in an OMOP supported vocabulary store the concept_id here, otherwise set to 0."""@en ;
    rdfs:domain omop:Person ;
    rdfs:range omop:Concept ;
    omop:omop_cdm_name "person.race_source_concept_id#17 AS Concept"^^xsd:string .

omop:has_relationship_type a owl:FunctionalProperty,
        owl:ObjectProperty ;
    rdfs:label "Has relationship type"^^xsd:string ;
    owlready:python_name "relationship_type"^^xsd:string ;
    rdfs:comment """For Location History: This is the relationship between the location and the entity (PERSON, PROVIDER, or CARE_SITE)
Concepts in this field must be in the Location class. [Accepted Concepts](https://athena.ohdsi.org/search-terms/terms?standardConcept=Standard&conceptClass=Location&page=1&pageSize=15&query=&boosts). If the DOMAIN_ID is CARE_SITE this should be 0 and when the domain is PROVIDER the value is [Office](https://athena.ohdsi.org/search-terms/terms/4121722)."""@en ;
    rdfs:domain omop:LocationHistory ;
    rdfs:range omop:Concept ;
    omop:omop_cdm_name "location_history.relationship_type_concept_id#262 AS Concept"^^xsd:string .

omop:has_respondent_type a owl:FunctionalProperty,
        owl:ObjectProperty ;
    rdfs:label "Has respondent type"^^xsd:string ;
    owlready:python_name "respondent_type"^^xsd:string ;
    rdfs:comment """For Survey Conduct: This is a Concept that represents who actually recorded the answers to the survey. For example, this could be the patient or a research associate.
There is no specific domain or class for this field, just choose the one that best represents the value given in the source."""@en ;
    rdfs:domain omop:SurveyConduct ;
    rdfs:range omop:Concept ;
    omop:omop_cdm_name "survey_conduct.respondent_type_concept_id#236 AS Concept"^^xsd:string .

omop:has_reverse_relationship a owl:FunctionalProperty,
        owl:ObjectProperty ;
    rdfs:label "Has reverse relationship"^^xsd:string ;
    owlready:python_name "reverse_relationship"^^xsd:string ;
    rdfs:domain omop:Relationship ;
    omop:omop_cdm_name "relationship.reverse_relationship_id#393 AS Thing"^^xsd:string .

omop:has_source_vocabulary a owl:FunctionalProperty,
        owl:ObjectProperty ;
    rdfs:label "Has source vocabulary"^^xsd:string ;
    owlready:python_name "source_vocabulary"^^xsd:string ;
    rdfs:comment """For Source To Concept Map: A foreign key to the
VOCABULARY table defining the
vocabulary of the source code that
is being translated to a Standard
Concept."""@en ;
    rdfs:domain omop:SourceToConceptMap ;
    rdfs:range omop:Vocabulary ;
    omop:omop_cdm_name "source_to_concept_map.source_vocabulary_id#404 AS Vocabulary"^^xsd:string .

omop:has_specialty a owl:FunctionalProperty,
        owl:ObjectProperty ;
    rdfs:label "Has specialty"^^xsd:string ;
    owlready:python_name "specialty"^^xsd:string ;
    rdfs:comment """For Provider: This field either represents the most common specialty that occurs in the data or the most specific concept that represents all specialties listed, should the provider have more than one. This includes physician specialties such as internal medicine, emergency medicine, etc. and allied health professionals such as nurses, midwives, and pharmacists.
If a Provider has more than one Specialty, there are two options: 1. Choose a concept_id which is a common ancestor to the multiple specialties, or, 2. Choose the specialty that occurs most often for the provider. Concepts in this field should be Standard with a domain of Provider. If not available, set to 0. [Accepted Concepts](http://athena.ohdsi.org/search-terms/terms?domain=Provider&standardConcept=Standard&page=1&pageSize=15&query=)."""@en ;
    rdfs:domain omop:Provider ;
    rdfs:range omop:Concept ;
    omop:omop_cdm_name "provider.specialty_concept_id#277 AS Concept"^^xsd:string .

omop:has_specialty_source a owl:FunctionalProperty,
        owl:ObjectProperty ;
    rdfs:label "Has specialty source"^^xsd:string ;
    owlready:python_name "specialty_source"^^xsd:string ;
    rdfs:comment """For Provider: This is often zero as many sites use proprietary codes to store physician speciality.
If the source data codes provider specialty in an OMOP supported vocabulary store the concept_id here. If not available, set to 0."""@en ;
    rdfs:domain omop:Provider ;
    rdfs:range omop:Concept ;
    omop:omop_cdm_name "provider.specialty_source_concept_id#283 AS Concept"^^xsd:string .

omop:has_specimen a owl:ObjectProperty ;
    rdfs:label "Has specimen"^^xsd:string ;
    owlready:python_name "specimens"^^xsd:string ;
    rdfs:comment "reversed relation, For Specimen: The person from whom the specimen is collected."@en ;
    rdfs:domain omop:Person ;
    rdfs:range omop:Specimen ;
    omop:omop_cdm_name "specimen.person_id#208 AS Person"^^xsd:string .

omop:has_sponsor a owl:FunctionalProperty,
        owl:ObjectProperty ;
    rdfs:label "Has sponsor"^^xsd:string ;
    owlready:python_name "sponsor"^^xsd:string ;
    rdfs:comment """For Payer Plan Period: This field represents the sponsor of the Plan who finances the Plan. This includes self-insured, small group health plan and large group health plan.
Map the sponsor directly to a standard CONCEPT_ID. If one does not exists please contact the vocabulary team. There is no global controlled vocabulary available for this information. The point is to stratify on this information and identify if Persons have the same sponsor though the name of the sponsor is not necessary. If not available, set to 0. [Accepted Concepts](http://athena.ohdsi.org/search-terms/terms?domain=Sponsor&standardConcept=Standard&page=1&pageSize=15&query=)."""@en ;
    rdfs:domain omop:PayerPlanPeriod ;
    rdfs:range omop:Concept ;
    omop:omop_cdm_name "payer_plan_period.sponsor_concept_id#300 AS Concept"^^xsd:string .

omop:has_status a owl:FunctionalProperty,
        owl:ObjectProperty ;
    rdfs:label "Has status"^^xsd:string ;
    owlready:python_name "status"^^xsd:string ;
    rdfs:comment """For Condition Occurrence: This concept represents the point during the visit the diagnosis was given (admitting diagnosis, final diagnosis), whether the diagnosis was determined due to laboratory findings, if the diagnosis was exclusionary, or if it was a preliminary diagnosis, among others.
Choose the Concept in the Condition Status domain that best represents the point during the visit when the diagnosis was given. These can include admitting diagnosis, principal diagnosis, and secondary diagnosis. If not available, set to 0. [Accepted Concepts](https://athena.ohdsi.org/search-terms/terms?domain=Condition+Status&standardConcept=Standard&page=1&pageSize=15&query=)."""@en ;
    rdfs:domain omop:ConditionOccurrence ;
    rdfs:range omop:Concept ;
    omop:omop_cdm_name "condition_occurrence.condition_status_concept_id#69 AS Concept"^^xsd:string .

omop:has_survey a owl:FunctionalProperty,
        owl:ObjectProperty ;
    rdfs:label "Has survey"^^xsd:string ;
    owlready:python_name "survey"^^xsd:string ;
    rdfs:comment """For Survey Conduct: This is the Concept that represents the survey that was completed.
Put the CONCEPT_ID that identifies the survey that the Person completed. There is no specified domain for this table but the concept class 'staging/scales' contains many common surveys. [Accepted Concepts](https://athena.ohdsi.org/search-terms/terms?standardConcept=Standard&conceptClass=Staging+%2F+Scales&page=5&pageSize=15&query=)."""@en ;
    rdfs:domain omop:SurveyConduct ;
    rdfs:range omop:Concept ;
    omop:omop_cdm_name "survey_conduct.survey_concept_id#229 AS Concept"^^xsd:string .

omop:has_survey_source a owl:FunctionalProperty,
        owl:ObjectProperty ;
    rdfs:label "Has survey source"^^xsd:string ;
    owlready:python_name "survey_source"^^xsd:string ;
    rdfs:comment "For Survey Conduct: If unavailable, set to 0."@en ;
    rdfs:domain omop:SurveyConduct ;
    rdfs:range omop:Concept ;
    omop:omop_cdm_name "survey_conduct.survey_source_concept_id#244 AS Concept"^^xsd:string .

omop:has_target a owl:FunctionalProperty,
        owl:ObjectProperty ;
    rdfs:label "Has target"^^xsd:string ;
    owlready:python_name "target"^^xsd:string ;
    rdfs:comment """For Source To Concept Map: The target Concept
to which the source code is being
mapped."""@en ;
    rdfs:domain omop:SourceToConceptMap ;
    rdfs:range omop:Concept ;
    omop:omop_cdm_name "source_to_concept_map.target_concept_id#406 AS Concept"^^xsd:string .

omop:has_target_vocabulary a owl:FunctionalProperty,
        owl:ObjectProperty ;
    rdfs:label "Has target vocabulary"^^xsd:string ;
    owlready:python_name "target_vocabulary"^^xsd:string ;
    rdfs:comment "For Source To Concept Map: The Vocabulary of the target Concept."@en ;
    rdfs:domain omop:SourceToConceptMap ;
    rdfs:range omop:Vocabulary ;
    omop:omop_cdm_name "source_to_concept_map.target_vocabulary_id#407 AS Vocabulary"^^xsd:string .

omop:has_timing a owl:FunctionalProperty,
        owl:ObjectProperty ;
    rdfs:label "Has timing"^^xsd:string ;
    owlready:python_name "timing"^^xsd:string ;
    rdfs:comment """For Survey Conduct: This is a Concept that represents the timing of the survey. For example this could be the 3-month follow-up appointment.
There is no specific domain or class for this field, just choose the one that best represents the value given in the source."""@en ;
    rdfs:domain omop:SurveyConduct ;
    rdfs:range omop:Concept ;
    omop:omop_cdm_name "survey_conduct.timing_concept_id#237 AS Concept"^^xsd:string .

omop:has_validated_survey a owl:FunctionalProperty,
        owl:ObjectProperty ;
    rdfs:label "Has validated survey"^^xsd:string ;
    owlready:python_name "validated_survey"^^xsd:string ;
    rdfs:comment "For Survey Conduct: If unavailable, set to 0."@en ;
    rdfs:domain omop:SurveyConduct ;
    rdfs:range omop:Concept ;
    omop:omop_cdm_name "survey_conduct.validated_survey_concept_id#246 AS Concept"^^xsd:string .

omop:has_visit_occurrence a owl:ObjectProperty ;
    rdfs:label "Has visit occurrence"^^xsd:string ;
    owlready:python_name "visit_occurrences"^^xsd:string ;
    rdfs:domain omop:Person ;
    rdfs:range omop:VisitOccurrence ;
    omop:omop_cdm_name "visit_occurrence.person_id#26 AS Person"^^xsd:string .

omop:has_vocabulary a owl:FunctionalProperty,
        owl:ObjectProperty ;
    rdfs:label "Has vocabulary"^^xsd:string ;
    owlready:python_name "vocabulary"^^xsd:string ;
    rdfs:comment """For Concept: A foreign key to the [VOCABULARY](https://ohdsi.github.io/CommonDataModel/cdm531.html#vocabulary)
table indicating from which source the
Concept has been adapted."""@en ;
    rdfs:domain omop:Concept ;
    rdfs:range omop:Vocabulary ;
    omop:omop_cdm_name "concept.vocabulary_id#365 AS Vocabulary"^^xsd:string .

omop:id a owl:DatatypeProperty,
        owl:FunctionalProperty ;
    rdfs:label "Id"^^xsd:string ;
    rdfs:comment "For Care Site: Assign an id to each unique combination of location_id and place_of_service_source_value."@en,
        "For Cohort Definition: This is the identifier given to the cohort, usually by the ATLAS application"@en,
        "For Concept Class: A unique key for each class."@en,
        "For Concept: A unique identifier for each Concept across all domains."@en,
        """For Condition Occurrence: The unique key given to a condition record for a person. Refer to the ETL for how duplicate conditions during the same visit were handled.
Each instance of a condition present in the source data should be assigned this unique key. In some cases, a person can have multiple records of the same condition within the same visit. It is valid to keep these duplicates and assign them individual, unique, CONDITION_OCCURRENCE_IDs, though it is up to the ETL how they should be handled."""@en,
        "For Cost: A unique identifier for each COST record."@en,
        """For Device Exposure: The unique key given to records a person's exposure to a foreign physical object or instrument.
Each instance of an exposure to a foreign object or device present in the source data should be assigned this unique key."""@en,
        "For Domain: A unique key for each domain."@en,
        """For Drug Exposure: The unique key given to records of drug dispensings or administrations for a person. Refer to the ETL for how duplicate drugs during the same visit were handled.
Each instance of a drug dispensing or administration present in the source data should be assigned this unique key. In some cases, a person can have multiple records of the same drug within the same visit. It is valid to keep these duplicates and assign them individual, unique, DRUG_EXPOSURE_IDs, though it is up to the ETL how they should be handled."""@en,
        """For Location: The unique key given to a unique Location.
Each instance of a Location in the source data should be assigned this unique key."""@en,
        """For Measurement: The unique key given to a Measurement record for a Person. Refer to the ETL for how duplicate Measurements during the same Visit were handled.
Each instance of a measurement present in the source data should be assigned this unique key. In some cases, a person can have multiple records of the same measurement within the same visit. It is valid to keep these duplicates and assign them individual, unique, MEASUREMENT_IDs, though it is up to the ETL how they should be handled."""@en,
        "For Note Nlp: A unique identifier for the NLP record."@en,
        "For Note: A unique identifier for each note."@en,
        """For Observation Period: A Person can have multiple discrete Observation Periods which are identified by the Observation_Period_Id.
Assign a unique observation_period_id to each discrete Observation Period for a Person."""@en,
        """For Observation: The unique key given to an Observation record for a Person. Refer to the ETL for how duplicate Observations during the same Visit were handled.
Each instance of an observation present in the source data should be assigned this unique key."""@en,
        "For Payer Plan Period: A unique identifier for each unique combination of a Person, Payer, Plan, and Period of time."@en,
        """For Person: It is assumed that every person with a different unique identifier is in fact a different person and should be treated independently.
Any person linkage that needs to occur to uniquely identify Persons ought to be done prior to writing this table. This identifier can be the original id from the source data provided if it is an integer, otherwise it can be an autogenerated number."""@en,
        """For Procedure Occurrence: The unique key given to a procedure record for a person. Refer to the ETL for how duplicate procedures during the same visit were handled.
Each instance of a procedure occurrence in the source data should be assigned this unique key. In some cases, a person can have multiple records of the same procedure within the same visit. It is valid to keep these duplicates and assign them individual, unique, PROCEDURE_OCCURRENCE_IDs, though it is up to the ETL how they should be handled."""@en,
        """For Provider: It is assumed that every provider with a different unique identifier is in fact a different person and should be treated independently.
This identifier can be the original id from the source data provided it is an integer, otherwise it can be an autogenerated number."""@en,
        "For Specimen: Unique identifier for each specimen."@en,
        """For Survey Conduct: Unique identifier for each completed survey.
For each instance of a survey completion create a unique identifier."""@en,
        """For Visit Detail: Use this to identify unique interactions between a person and the health care system. This identifier links across the other CDM event tables to associate events with a visit detail.
This should be populated by creating a unique identifier for each unique interaction between a person and the healthcare system where the person receives a medical good or service over a span of time."""@en,
        """For Visit Occurrence: Use this to identify unique interactions between a person and the health care system. This identifier links across the other CDM event tables to associate events with a visit.
This should be populated by creating a unique identifier for each unique interaction between a person and the healthcare system where the person receives a medical good or service over a span of time."""@en,
        """For Vocabulary: A unique identifier for each Vocabulary, such
as ICD9CM, SNOMED, Visit."""@en ;
    rdfs:domain omop:OmopCDMThing ;
    rdfs:range [ a rdfs:Datatype ;
            owl:unionOf ( xsd:integer xsd:string ) ] ;
    omop:omop_cdm_name "care_site.care_site_id#267 AS int|str"^^xsd:string,
        "cohort_definition.cohort_definition_id#427 AS int|str"^^xsd:string,
        "concept.concept_id#362 AS int|str"^^xsd:string,
        "concept_class.concept_class_id#380 AS int|str"^^xsd:string,
        "condition_era.condition_era_id#339 AS int|str"^^xsd:string,
        "condition_occurrence.condition_occurrence_id#61 AS int|str"^^xsd:string,
        "cost.cost_id#307 AS int|str"^^xsd:string,
        "device_exposure.device_exposure_id#114 AS int|str"^^xsd:string,
        "domain.domain_id#377 AS int|str"^^xsd:string,
        "dose_era.dose_era_id#332 AS int|str"^^xsd:string,
        "drug_era.drug_era_id#325 AS int|str"^^xsd:string,
        "drug_exposure.drug_exposure_id#77 AS int|str"^^xsd:string,
        "location.location_id#251 AS int|str"^^xsd:string,
        "measurement.measurement_id#129 AS int|str"^^xsd:string,
        "note.note_id#177 AS int|str"^^xsd:string,
        "note_nlp.note_nlp_id#193 AS int|str"^^xsd:string,
        "observation.observation_id#149 AS int|str"^^xsd:string,
        "observation_period.observation_period_id#20 AS int|str"^^xsd:string,
        "payer_plan_period.payer_plan_period_id#286 AS int|str"^^xsd:string,
        "person.person_id#1 AS int|str"^^xsd:string,
        "procedure_occurrence.procedure_occurrence_id#100 AS int|str"^^xsd:string,
        "provider.provider_id#273 AS int|str"^^xsd:string,
        "relationship.relationship_id#389 AS int|str"^^xsd:string,
        "specimen.specimen_id#207 AS int|str"^^xsd:string,
        "survey_conduct.survey_conduct_id#227 AS int|str"^^xsd:string,
        "visit_detail.visit_detail_id#42 AS int|str"^^xsd:string,
        "visit_occurrence.visit_occurrence_id#25 AS int|str"^^xsd:string,
        "vocabulary.vocabulary_id#372 AS int|str"^^xsd:string .

omop:is_hierarchical a owl:DatatypeProperty,
        owl:FunctionalProperty ;
    rdfs:label "Is hierarchical"^^xsd:string ;
    rdfs:domain omop:Relationship ;
    rdfs:range xsd:string ;
    omop:omop_cdm_name "relationship.is_hierarchical#391 AS str"^^xsd:string .

omop:lexical_variant a owl:DatatypeProperty,
        owl:FunctionalProperty ;
    rdfs:label "Lexical variant"^^xsd:string ;
    rdfs:comment "For Note Nlp: Raw text extracted from the NLP tool."@en ;
    rdfs:domain omop:NoteNlp ;
    rdfs:range xsd:string ;
    omop:omop_cdm_name "note_nlp.lexical_variant#198 AS str"^^xsd:string .

omop:max_levels_of_separation a owl:DatatypeProperty,
        owl:FunctionalProperty ;
    rdfs:label "Max levels of separation"^^xsd:string ;
    rdfs:comment """For Concept Ancestor: The maximum separation in number of
levels of hierarchy between ancestor and
descendant concepts. This is an attribute
that is used to simplify hierarchic analysis."""@en ;
    rdfs:domain omop:ConceptAncestor ;
    rdfs:range xsd:integer ;
    omop:omop_cdm_name "concept_ancestor.max_levels_of_separation#401 AS int"^^xsd:string .

omop:min_levels_of_separation a owl:DatatypeProperty,
        owl:FunctionalProperty ;
    rdfs:label "Min levels of separation"^^xsd:string ;
    rdfs:comment """For Concept Ancestor: The minimum separation in number of
levels of hierarchy between ancestor and
descendant concepts. This is an attribute
that is used to simplify hierarchic analysis."""@en ;
    rdfs:domain omop:ConceptAncestor ;
    rdfs:range xsd:integer ;
    omop:omop_cdm_name "concept_ancestor.min_levels_of_separation#400 AS int"^^xsd:string .

omop:reference a owl:DatatypeProperty,
        owl:FunctionalProperty ;
    rdfs:label "Reference"^^xsd:string ;
    rdfs:comment """For Vocabulary: External reference to documentation or
available download of the about the
vocabulary."""@en ;
    rdfs:domain omop:Vocabulary ;
    rdfs:range xsd:string ;
    omop:omop_cdm_name "vocabulary.vocabulary_reference#374 AS str"^^xsd:string .

omop:source_code a owl:DatatypeProperty,
        owl:FunctionalProperty ;
    rdfs:label "Source code"^^xsd:string ;
    rdfs:comment """For Source To Concept Map: The source code being translated
into a Standard Concept."""@en ;
    rdfs:domain omop:SourceToConceptMap ;
    rdfs:range xsd:string ;
    omop:omop_cdm_name "source_to_concept_map.source_code#402 AS str"^^xsd:string .

omop:stop_reason a owl:DatatypeProperty,
        owl:FunctionalProperty ;
    rdfs:label "Stop reason"^^xsd:string ;
    rdfs:comment """For Condition Occurrence: The Stop Reason indicates why a Condition is no longer valid with respect to the purpose within the source data. Note that a Stop Reason does not necessarily imply that the condition is no longer occurring.
This information is often not populated in source data and it is a valid etl choice to leave it blank if the information does not exist."""@en,
        """For Drug Exposure: The reason a person stopped a medication as it is represented in the source. Reasons include regimen completed, changed, removed, etc. This field will be retired in v6.0.
This information is often not populated in source data and it is a valid etl choice to leave it blank if the information does not exist."""@en ;
    rdfs:domain [ a owl:Class ;
            owl:unionOf ( omop:ConditionOccurrence omop:DrugExposure ) ] ;
    rdfs:range xsd:string ;
    omop:omop_cdm_name "condition_occurrence.stop_reason#70 AS str"^^xsd:string,
        "drug_exposure.stop_reason#86 AS str"^^xsd:string .

omop:survey_end_datetime a owl:DatatypeProperty,
        owl:FunctionalProperty ;
    rdfs:label "Survey end datetime"^^xsd:string ;
    rdfs:comment "For Survey Conduct: If no time given, set to midnight."@en ;
    rdfs:domain omop:SurveyConduct ;
    rdfs:range xsd:dateTime ;
    omop:omop_cdm_name "survey_conduct.survey_end_datetime#233 AS datetime"^^xsd:string .

omop:text a owl:DatatypeProperty,
        owl:FunctionalProperty ;
    rdfs:label "Text"^^xsd:string ;
    rdfs:comment "For Note: The content of the note."@en ;
    rdfs:domain omop:Note ;
    rdfs:range xsd:string ;
    omop:omop_cdm_name "note.note_text#186 AS str"^^xsd:string .

omop:value a owl:DatatypeProperty,
        owl:FunctionalProperty ;
    rdfs:label "Value"^^xsd:string ;
    rdfs:comment "For Dose Era: The numeric value of the dosage of the drug_ingredient."@en ;
    rdfs:domain omop:DoseEra ;
    rdfs:range xsd:decimal ;
    omop:omop_cdm_name "dose_era.dose_value#336 AS float"^^xsd:string .

omop:value_as_number a owl:DatatypeProperty,
        owl:FunctionalProperty ;
    rdfs:label "Value as number"^^xsd:string ;
    rdfs:comment """For Measurement: This is the numerical value of the Result of the Measurement, if available. Note that measurements such as blood pressures will be split into their component parts i.e. one record for systolic, one record for diastolic.
If there is a negative value coming from the source, set the VALUE_AS_NUMBER to NULL, with the exception of the following Measurements (listed as LOINC codes):<br>-  [1925-7](https://athena.ohdsi.org/search-terms/terms/3003396) Base excess in Arterial blood by calculation - [1927-3](https://athena.ohdsi.org/search-terms/terms/3002032) Base excess in Venous blood by calculation - [8632-2](https://athena.ohdsi.org/search-terms/terms/3006277) QRS-Axis - [11555-0](https://athena.ohdsi.org/search-terms/terms/3012501) Base excess in Blood by calculation - [1926-5](https://athena.ohdsi.org/search-terms/terms/3003129) Base excess in Capillary blood by calculation - [28638-5](https://athena.ohdsi.org/search-terms/terms/3004959) Base excess in Arterial cord blood by calculation [28639-3](https://athena.ohdsi.org/search-terms/terms/3007435) Base excess in Venous cord blood by calculation"""@en,
        "For Observation: This is the numerical value of the Result of the Observation, if applicable and available. It is not expected that all Observations will have numeric results, rather, this field is here to house values should they exist."@en ;
    rdfs:domain [ a owl:Class ;
            owl:unionOf ( omop:Observation omop:Measurement ) ] ;
    rdfs:range xsd:decimal ;
    omop:omop_cdm_name "measurement.value_as_number#137 AS float"^^xsd:string,
        "observation.value_as_number#155 AS float"^^xsd:string .

omop:value_as_string a owl:DatatypeProperty,
        owl:FunctionalProperty ;
    rdfs:label "Value as string"^^xsd:string ;
    rdfs:comment "For Observation: This is the categorical value of the Result of the Observation, if applicable and available."@en ;
    rdfs:domain [ a owl:Class ;
            owl:unionOf ( omop:Observation omop:Metadata ) ] ;
    rdfs:range xsd:string ;
    omop:omop_cdm_name "metadata.value_as_string#348 AS str"^^xsd:string,
        "observation.value_as_string#156 AS str"^^xsd:string .

omop:ConceptSynonym a owl:Class ;
    rdfs:label "Concept synonym"^^xsd:string ;
    rdfs:comment "The CONCEPT_SYNONYM table is used to store alternate names and descriptions for Concepts."@en ;
    rdfs:subClassOf [ a owl:Restriction ;
            owl:allValuesFrom omop:Concept ;
            owl:onProperty omop:has_concept ],
        [ a owl:Restriction ;
            owl:onProperty omop:has_concept ;
            owl:someValuesFrom omop:Concept ],
        [ a owl:Restriction ;
            owl:allValuesFrom omop:Concept ;
            owl:onProperty omop:has_language ],
        [ a owl:Restriction ;
            owl:onProperty omop:has_language ;
            owl:someValuesFrom omop:Concept ],
        [ a owl:Restriction ;
            owl:allValuesFrom xsd:string ;
            owl:onProperty omop:name ],
        [ a owl:Restriction ;
            owl:onProperty omop:name ;
            owl:someValuesFrom xsd:string ],
        omop:OmopCDMThing ;
    omop:omop_cdm_name "concept_synonym"^^xsd:string .

omop:ConditionEra a owl:Class ;
    rdfs:label "Condition era"^^xsd:string ;
    rdfs:comment """A Condition Era is defined as a span of time when the Person is assumed to have a given condition. Similar to Drug Eras, Condition Eras are chronological periods of Condition Occurrence. Combining individual Condition Occurrences into a single Condition Era serves two purposes:

- It allows aggregation of chronic conditions that require frequent ongoing care, instead of treating each Condition Occurrence as an independent event.
- It allows aggregation of multiple, closely timed doctor visits for the same Condition to avoid double-counting the Condition Occurrences.
For example, consider a Person who visits her Primary Care Physician (PCP) and who is referred to a specialist. At a later time, the Person visits the specialist, who confirms the PCP's original diagnosis and provides the appropriate treatment to resolve the condition. These two independent doctor visits should be aggregated into one Condition Era."""@en ;
    rdfs:subClassOf [ a owl:Restriction ;
            owl:onProperty [ owl:inverseOf omop:has_condition_era ] ;
            owl:someValuesFrom omop:Person ],
        [ a owl:Restriction ;
            owl:allValuesFrom xsd:integer ;
            owl:onProperty omop:occurrence_count ],
        omop:Era ;
    omop:omop_cdm_name "condition_era"^^xsd:string .

omop:ObservationPeriod a owl:Class ;
    rdfs:label "Observation period"^^xsd:string ;
    rdfs:comment "This table contains records which define spans of time during which two conditions are expected to hold: (i) Clinical Events that happened to the Person are recorded in the Event tables, and (ii) absense of records indicate such Events did not occur during this span of time."@en ;
    rdfs:subClassOf [ a owl:Restriction ;
            owl:onProperty omop:has_period_type ;
            owl:someValuesFrom omop:Concept ],
        [ a owl:Restriction ;
            owl:onProperty [ owl:inverseOf omop:has_observation_period ] ;
            owl:someValuesFrom omop:Person ],
        [ a owl:Restriction ;
            owl:allValuesFrom omop:Concept ;
            owl:onProperty omop:has_period_type ],
        omop:ClinicalElement,
        omop:DateDuration ;
    omop:omop_cdm_name "observation_period"^^xsd:string .

omop:admitted_from_source_value a owl:DatatypeProperty,
        owl:FunctionalProperty ;
    rdfs:label "Admitted from source value"^^xsd:string ;
    rdfs:comment """For Visit Detail: Use this field to determine where the patient was admitted from. This concept is part of the visit domain and can indicate if a patient was admitted to the hospital from a long-term care facility, for example.
If available, map the admitted_from_source_value to a standard concept in the visit domain. If not available, map to 0. [Accepted Concepts](https://athena.ohdsi.org/search-terms/terms?domain=Visit&standardConcept=Standard&page=1&pageSize=15&query=)."""@en,
        "For Visit Occurrence: This information may be called something different in the source data but the field is meant to contain a value indicating where a person was admitted from. Typically this applies only to visits that have a length of stay, like inpatient visits or long-term care visits."@en ;
    rdfs:domain [ a owl:Class ;
            owl:unionOf ( omop:VisitDetail omop:VisitOccurrence ) ] ;
    omop:omop_cdm_name "visit_detail.admitted_from_source_value#55 AS int"^^xsd:string,
        "visit_occurrence.admitted_from_source_value#38 AS str"^^xsd:string .

omop:has_admitted_from a owl:FunctionalProperty,
        owl:ObjectProperty ;
    rdfs:label "Has admitted from"^^xsd:string ;
    owlready:python_name "admitted_from"^^xsd:string ;
    rdfs:comment "For Visit Detail: This information may be called something different in the source data but the field is meant to contain a value indicating where a person was admitted from. Typically this applies only to visits that have a length of stay, like inpatient visits or long-term care visits."@en,
        """For Visit Occurrence: Use this field to determine where the patient was admitted from. This concept is part of the visit domain and can indicate if a patient was admitted to the hospital from a long-term care facility, for example.
If available, map the admitted_from_source_value to a standard concept in the visit domain. If not available set to 0."""@en ;
    rdfs:domain [ a owl:Class ;
            owl:unionOf ( omop:VisitDetail omop:VisitOccurrence ) ] ;
    rdfs:range omop:Concept ;
    omop:omop_cdm_name "visit_detail.admitted_from_concept_id#54 AS Concept"^^xsd:string,
        "visit_occurrence.admitted_from_concept_id#37 AS Concept"^^xsd:string .

omop:has_condition_occurrence a owl:ObjectProperty ;
    rdfs:label "Has condition occurrence"^^xsd:string ;
    owlready:python_name "condition_occurrences"^^xsd:string ;
    rdfs:comment "reversed relation, For Condition Occurrence: The PERSON_ID of the PERSON for whom the condition is recorded."@en,
        """reversed relation, For Condition Occurrence: The VISIT_DETAIL record during which the condition occurred. For example, if the person was in the ICU at the time of the diagnosis the VISIT_OCCURRENCE record would reflect the overall hospital stay and the VISIT_DETAIL record would reflect the ICU stay during the hospital visit.
Same rules apply as for the VISIT_OCCURRENCE_ID."""@en,
        """reversed relation, For Condition Occurrence: The visit during which the condition occurred.
Depending on the structure of the source data, this may have to be determined based on dates. If a CONDITION_START_DATE occurs within the start and end date of a Visit it is a valid ETL choice to choose the VISIT_OCCURRENCE_ID from the Visit that subsumes it, even if not explicitly stated in the data. While not required, an attempt should be made to locate the VISIT_OCCURRENCE_ID of the CONDITION_OCCURRENCE record."""@en ;
    rdfs:domain [ a owl:Class ;
            owl:unionOf ( omop:BaseVisit omop:Person ) ] ;
    rdfs:range omop:ConditionOccurrence ;
    omop:omop_cdm_name "condition_occurrence.person_id#62 AS Person"^^xsd:string,
        "condition_occurrence.visit_detail_id#73 AS VisitDetail"^^xsd:string,
        "condition_occurrence.visit_occurrence_id#72 AS VisitOccurrence"^^xsd:string .

omop:has_device_exposure a owl:ObjectProperty ;
    rdfs:label "Has device exposure"^^xsd:string ;
    owlready:python_name "device_exposures"^^xsd:string ;
    rdfs:comment """reversed relation, For Device Exposure: The Visit Detail during which the device was prescribed or given.
To populate this field device exposures must be explicitly initiated in the visit detail record."""@en,
        """reversed relation, For Device Exposure: The Visit during which the device was prescribed or given.
To populate this field device exposures must be explicitly initiated in the visit."""@en ;
    rdfs:domain [ a owl:Class ;
            owl:unionOf ( omop:BaseVisit omop:Person ) ] ;
    rdfs:range omop:DeviceExposure ;
    omop:omop_cdm_name "device_exposure.person_id#115 AS Person"^^xsd:string,
        "device_exposure.visit_detail_id#126 AS VisitDetail"^^xsd:string,
        "device_exposure.visit_occurrence_id#125 AS VisitOccurrence"^^xsd:string .

omop:has_drug_exposure a owl:ObjectProperty ;
    rdfs:label "Has drug exposure"^^xsd:string ;
    owlready:python_name "drug_exposures"^^xsd:string ;
    rdfs:comment "reversed relation, For Drug Exposure: The PERSON_ID of the PERSON for whom the drug dispensing or administration is recorded. This may be a system generated code."@en,
        """reversed relation, For Drug Exposure: The VISIT_DETAIL record during which the drug exposure occurred. For example, if the person was in the ICU at the time of the drug administration the VISIT_OCCURRENCE record would reflect the overall hospital stay and the VISIT_DETAIL record would reflect the ICU stay during the hospital visit.
Same rules apply as for the VISIT_OCCURRENCE_ID."""@en,
        """reversed relation, For Drug Exposure: The Visit during which the drug was prescribed, administered or dispensed.
To populate this field drug exposures must be explicitly initiated in the visit."""@en ;
    rdfs:domain [ a owl:Class ;
            owl:unionOf ( omop:BaseVisit omop:Person ) ] ;
    rdfs:range omop:DrugExposure ;
    omop:omop_cdm_name "drug_exposure.person_id#78 AS Person"^^xsd:string,
        "drug_exposure.visit_detail_id#95 AS VisitDetail"^^xsd:string,
        "drug_exposure.visit_occurrence_id#94 AS VisitOccurrence"^^xsd:string .

omop:has_event_field a owl:FunctionalProperty,
        owl:ObjectProperty ;
    rdfs:label "Has event field"^^xsd:string ;
    owlready:python_name "event_field"^^xsd:string ;
    rdfs:comment """For Cost: If the Cost record is related to another record in the database, this field is the CONCEPT_ID that identifies which table the primary key of the linked record came from.
Put the CONCEPT_ID that identifies which table and field the COST_EVENT_ID came from."""@en ;
    rdfs:domain [ a owl:Class ;
            owl:unionOf ( omop:Cost omop:Note ) ] ;
    rdfs:range omop:Concept ;
    omop:omop_cdm_name "cost.cost_event_field_concept_id#310 AS Concept"^^xsd:string,
        "note.note_event_field_concept_id#180 AS Concept"^^xsd:string .

omop:has_measurement a owl:ObjectProperty ;
    rdfs:label "Has measurement"^^xsd:string ;
    owlready:python_name "measurements"^^xsd:string ;
    rdfs:comment "reversed relation, For Measurement: The PERSON_ID of the PERSON for whom the measurement is recorded. This may be a system generated code."@en,
        """reversed relation, For Measurement: The VISIT_DETAIL record during which the Measurement occurred. For example, if the Person was in the ICU at the time the VISIT_OCCURRENCE record would reflect the overall hospital stay and the VISIT_DETAIL record would reflect the ICU stay during the hospital visit.
Same rules apply as for the VISIT_OCCURRENCE_ID."""@en,
        """reversed relation, For Measurement: The visit during which the Measurement occurred.
Depending on the structure of the source data, this may have to be determined based on dates. If a MEASUREMENT_DATE occurs within the start and end date of a Visit it is a valid ETL choice to choose the VISIT_OCCURRENCE_ID from the visit that subsumes it, even if not explicitly stated in the data. While not required, an attempt should be made to locate the VISIT_OCCURRENCE_ID of the measurement record. If a measurement is related to a visit explicitly in the source data, it is possible that the result date of the Measurement falls outside of the bounds of the Visit dates."""@en ;
    rdfs:domain [ a owl:Class ;
            owl:unionOf ( omop:BaseVisit omop:Person ) ] ;
    rdfs:range omop:Measurement ;
    omop:omop_cdm_name "measurement.person_id#130 AS Person"^^xsd:string,
        "measurement.visit_detail_id#144 AS VisitDetail"^^xsd:string,
        "measurement.visit_occurrence_id#143 AS VisitOccurrence"^^xsd:string .

omop:has_note a owl:ObjectProperty ;
    rdfs:label "Has note"^^xsd:string ;
    owlready:python_name "notes"^^xsd:string ;
    rdfs:comment "reversed relation, For Note: The Visit Detail during which the note was written."@en,
        "reversed relation, For Note: The Visit during which the note was written."@en ;
    rdfs:domain [ a owl:Class ;
            owl:unionOf ( omop:BaseVisit omop:Person ) ] ;
    rdfs:range omop:Note ;
    omop:omop_cdm_name "note.person_id#178 AS Person"^^xsd:string,
        "note.visit_detail_id#191 AS VisitDetail"^^xsd:string,
        "note.visit_occurrence_id#190 AS VisitOccurrence"^^xsd:string .

omop:has_observation a owl:ObjectProperty ;
    rdfs:label "Has observation"^^xsd:string ;
    owlready:python_name "observations"^^xsd:string ;
    rdfs:comment "reversed relation, For Observation: The PERSON_ID of the Person for whom the Observation is recorded. This may be a system generated code."@en,
        """reversed relation, For Observation: The VISIT_DETAIL record during which the Observation occurred. For example, if the Person was in the ICU at the time the VISIT_OCCURRENCE record would reflect the overall hospital stay and the VISIT_DETAIL record would reflect the ICU stay during the hospital visit.
Same rules apply as for the VISIT_OCCURRENCE_ID."""@en,
        """reversed relation, For Observation: The visit during which the Observation occurred.
Depending on the structure of the source data, this may have to be determined based on dates. If an OBSERVATION_DATE occurs within the start and end date of a Visit it is a valid ETL choice to choose the VISIT_OCCURRENCE_ID from the visit that subsumes it, even if not explicitly stated in the data. While not required, an attempt should be made to locate the VISIT_OCCURRENCE_ID of the observation record. If an observation is related to a visit explicitly in the source data, it is possible that the result date of the Observation falls outside of the bounds of the Visit dates."""@en ;
    rdfs:domain [ a owl:Class ;
            owl:unionOf ( omop:BaseVisit omop:Person ) ] ;
    rdfs:range omop:Observation ;
    omop:omop_cdm_name "observation.person_id#150 AS Person"^^xsd:string,
        "observation.visit_detail_id#162 AS VisitDetail"^^xsd:string,
        "observation.visit_occurrence_id#161 AS VisitOccurrence"^^xsd:string .

omop:has_payer_plan_period a owl:FunctionalProperty,
        owl:ObjectProperty ;
    rdfs:label "Has payer plan period"^^xsd:string ;
    owlready:python_name "payer_plan_period"^^xsd:string ;
    rdfs:comment "For Cost: A foreign key to the PAYER_PLAN_PERIOD table, where the details of the Payer, Plan and Family are stored. Record the payer_plan_id that relates to the payer who contributed to the paid_by_payer field."@en,
        """reversed relation, For Payer Plan Period: The Person covered by the Plan.
A single Person can have multiple, overlapping, PAYER_PLAN_PERIOD records"""@en ;
    rdfs:domain [ a owl:Class ;
            owl:unionOf ( omop:Cost omop:Person ) ] ;
    rdfs:range omop:PayerPlanPeriod ;
    omop:omop_cdm_name "cost.payer_plan_period_id#324 AS PayerPlanPeriod"^^xsd:string,
        "payer_plan_period.person_id#287 AS Person"^^xsd:string .

omop:has_procedure_occurrence a owl:ObjectProperty ;
    rdfs:label "Has procedure occurrence"^^xsd:string ;
    owlready:python_name "procedure_occurrences"^^xsd:string ;
    rdfs:comment "reversed relation, For Procedure Occurrence: The PERSON_ID of the PERSON for whom the procedure is recorded. This may be a system generated code."@en,
        """reversed relation, For Procedure Occurrence: The VISIT_DETAIL record during which the Procedure occurred. For example, if the Person was in the ICU at the time of the Procedure the VISIT_OCCURRENCE record would reflect the overall hospital stay and the VISIT_DETAIL record would reflect the ICU stay during the hospital visit.
Same rules apply as for the VISIT_OCCURRENCE_ID."""@en,
        """reversed relation, For Procedure Occurrence: The visit during which the procedure occurred.
Depending on the structure of the source data, this may have to be determined based on dates. If a PROCEDURE_DATE occurs within the start and end date of a Visit it is a valid ETL choice to choose the VISIT_OCCURRENCE_ID from the Visit that subsumes it, even if not explicitly stated in the data. While not required, an attempt should be made to locate the VISIT_OCCURRENCE_ID of the PROCEDURE_OCCURRENCE record."""@en ;
    rdfs:domain [ a owl:Class ;
            owl:unionOf ( omop:BaseVisit omop:Person ) ] ;
    rdfs:range omop:ProcedureOccurrence ;
    omop:omop_cdm_name "procedure_occurrence.person_id#101 AS Person"^^xsd:string,
        "procedure_occurrence.visit_detail_id#110 AS VisitDetail"^^xsd:string,
        "procedure_occurrence.visit_occurrence_id#109 AS VisitOccurrence"^^xsd:string .

omop:has_survey_conduct a owl:ObjectProperty ;
    rdfs:label "Has survey conduct"^^xsd:string ;
    owlready:python_name "survey_conducts"^^xsd:string ;
    rdfs:comment "reversed relation, For Survey Conduct: The Visit during which the Survey occurred."@en ;
    rdfs:domain [ a owl:Class ;
            owl:unionOf ( omop:Person omop:VisitOccurrence ) ] ;
    rdfs:range omop:SurveyConduct ;
    omop:omop_cdm_name "survey_conduct.person_id#228 AS Person"^^xsd:string,
        "survey_conduct.visit_occurrence_id#249 AS VisitOccurrence"^^xsd:string .

omop:has_value_as_concept a owl:FunctionalProperty,
        owl:ObjectProperty ;
    rdfs:label "Has value as concept"^^xsd:string ;
    owlready:python_name "value_as_concept"^^xsd:string ;
    rdfs:comment """For Measurement: If the raw data gives a categorial result for measurements those values are captured and mapped to standard concepts in the 'Meas Value' domain.
If the raw data provides categorial results as well as continuous results for measurements, it is a valid ETL choice to preserve both values. The continuous value should go in the VALUE_AS_NUMBER field and the categorical value should be mapped to a standard concept in the 'Meas Value' domain and put in the VALUE_AS_CONCEPT_ID field. This is also the destination for the 'Maps to value' relationship."""@en,
        """For Observation: It is possible that some records destined for the Observation table have two clinical ideas represented in one source code. This is common with ICD10 codes that describe a family history of some Condition, for example. In OMOP the Vocabulary breaks these two clinical ideas into two codes; one becomes the OBSERVATION_CONCEPT_ID and the other becomes the VALUE_AS_CONCEPT_ID. It is important when using the Observation table to keep this possibility in mind and to examine the VALUE_AS_CONCEPT_ID field for relevant information.
Note that the value of VALUE_AS_CONCEPT_ID may be provided through mapping from a source Concept which contains the content of the Observation. In those situations, the CONCEPT_RELATIONSHIP table in addition to the 'Maps to' record contains a second record with the relationship_id set to 'Maps to value'. For example, ICD10 [Z82.4](https://athena.ohdsi.org/search-terms/terms/45581076) 'Family history of ischaemic heart disease and other diseases of the circulatory system' has a 'Maps to' relationship to [4167217](https://athena.ohdsi.org/search-terms/terms/4167217) 'Family history of clinical finding' as well as a 'Maps to value' record to [134057](https://athena.ohdsi.org/search-terms/terms/134057) 'Disorder of cardiovascular system'."""@en ;
    rdfs:domain [ a owl:Class ;
            owl:unionOf ( omop:Observation omop:Metadata omop:Measurement ) ] ;
    rdfs:range omop:Concept ;
    omop:omop_cdm_name "measurement.value_as_concept_id#138 AS Concept"^^xsd:string,
        "metadata.value_as_concept_id#349 AS Concept"^^xsd:string,
        "observation.value_as_concept_id#157 AS Concept"^^xsd:string .

omop:unit_source_value a owl:DatatypeProperty,
        owl:FunctionalProperty ;
    rdfs:label "Unit source value"^^xsd:string ;
    rdfs:comment """For Measurement: This field houses the verbatim value from the source data representing the unit of the Measurement that occurred.
This code is mapped to a Standard Condition Concept in the Standardized Vocabularies and the original code is stored here for reference."""@en,
        """For Observation: This field houses the verbatim value from the source data representing the unit of the Observation that occurred.
This code is mapped to a Standard Condition Concept in the Standardized Vocabularies and the original code is stored here for reference."""@en,
        "For Specimen: This unit for the quantity of the specimen, as represented in the source."@en ;
    rdfs:domain [ a owl:Class ;
            owl:unionOf ( omop:Observation omop:Measurement omop:Specimen ) ] ;
    rdfs:range xsd:string ;
    omop:omop_cdm_name "measurement.unit_source_value#147 AS str"^^xsd:string,
        "observation.unit_source_value#165 AS str"^^xsd:string,
        "specimen.unit_source_value#219 AS str"^^xsd:string .

omop:year_of_birth a owl:DatatypeProperty,
        owl:FunctionalProperty ;
    rdfs:label "Year of birth"^^xsd:string ;
    rdfs:comment """For Person: Compute age using year_of_birth.
For data sources with date of birth, the year should be extracted. For data sources where the year of birth is not available, the approximate year of birth could be derived based on age group categorization, if available."""@en ;
    rdfs:domain [ a owl:Class ;
            owl:unionOf ( omop:Provider omop:Person ) ] ;
    rdfs:range xsd:integer ;
    omop:omop_cdm_name "person.year_of_birth#3 AS int"^^xsd:string,
        "provider.year_of_birth#279 AS int"^^xsd:string .

omop:ConceptAncestor a owl:Class ;
    rdfs:label "Concept ancestor"^^xsd:string ;
    rdfs:comment """The CONCEPT_ANCESTOR table is designed to simplify observational analysis by providing the complete hierarchical relationships between Concepts. Only direct parent-child relationships between Concepts are stored in the CONCEPT_RELATIONSHIP table. To determine higher level ancestry connections, all individual direct relationships would have to be navigated at analysis time. The CONCEPT_ANCESTOR table includes records for all parent-child relationships, as well as grandparent-grandchild relationships and those of any other level of lineage. Using the CONCEPT_ANCESTOR table allows for querying for all descendants of a hierarchical concept. For example, drug ingredients and drug products are all descendants of a drug class ancestor.

This table is entirely derived from the CONCEPT, CONCEPT_RELATIONSHIP and RELATIONSHIP tables."""@en ;
    rdfs:subClassOf [ a owl:Restriction ;
            owl:allValuesFrom omop:Concept ;
            owl:onProperty omop:has_ancestor ],
        [ a owl:Restriction ;
            owl:onProperty omop:has_ancestor ;
            owl:someValuesFrom omop:Concept ],
        [ a owl:Restriction ;
            owl:allValuesFrom omop:Concept ;
            owl:onProperty omop:has_descendant ],
        [ a owl:Restriction ;
            owl:onProperty omop:has_descendant ;
            owl:someValuesFrom omop:Concept ],
        [ a owl:Restriction ;
            owl:allValuesFrom xsd:integer ;
            owl:onProperty omop:min_levels_of_separation ],
        [ a owl:Restriction ;
            owl:onProperty omop:min_levels_of_separation ;
            owl:someValuesFrom xsd:integer ],
        [ a owl:Restriction ;
            owl:allValuesFrom xsd:integer ;
            owl:onProperty omop:max_levels_of_separation ],
        [ a owl:Restriction ;
            owl:onProperty omop:max_levels_of_separation ;
            owl:someValuesFrom xsd:integer ],
        omop:OmopCDMThing ;
    omop:omop_cdm_name "concept_ancestor"^^xsd:string .

omop:ConceptClass a owl:Class ;
    rdfs:label "Concept class"^^xsd:string ;
    rdfs:comment "The CONCEPT_CLASS table is a reference table, which includes a list of the classifications used to differentiate Concepts within a given Vocabulary. This reference table is populated with a single record for each Concept Class."@en ;
    rdfs:subClassOf [ a owl:Restriction ;
            owl:allValuesFrom omop:Concept ;
            owl:onProperty omop:has_concept ],
        [ a owl:Restriction ;
            owl:onProperty omop:has_concept ;
            owl:someValuesFrom omop:Concept ],
        [ a owl:Restriction ;
            owl:allValuesFrom xsd:string ;
            owl:onProperty omop:name ],
        [ a owl:Restriction ;
            owl:onProperty omop:name ;
            owl:someValuesFrom xsd:string ],
        omop:OmopCDMThing ;
    omop:omop_cdm_name "concept_class"^^xsd:string .

omop:DoseEra a owl:Class ;
    rdfs:label "Dose era"^^xsd:string ;
    rdfs:comment "A Dose Era is defined as a span of time when the Person is assumed to be exposed to a constant dose of a specific active ingredient."@en ;
    rdfs:subClassOf [ a owl:Restriction ;
            owl:allValuesFrom omop:Concept ;
            owl:onProperty omop:has_unit ],
        [ a owl:Restriction ;
            owl:onProperty omop:has_unit ;
            owl:someValuesFrom omop:Concept ],
        [ a owl:Restriction ;
            owl:onProperty [ owl:inverseOf omop:has_dose_era ] ;
            owl:someValuesFrom omop:Person ],
        [ a owl:Restriction ;
            owl:allValuesFrom xsd:decimal ;
            owl:onProperty omop:value ],
        [ a owl:Restriction ;
            owl:onProperty omop:value ;
            owl:someValuesFrom xsd:decimal ],
        omop:Era ;
    omop:omop_cdm_name "dose_era"^^xsd:string .

omop:DrugEra a owl:Class ;
    rdfs:label "Drug era"^^xsd:string ;
    rdfs:comment "A Drug Era is defined as a span of time when the Person is assumed to be exposed to a particular active ingredient. A Drug Era is not the same as a Drug Exposure: Exposures are individual records corresponding to the source when Drug was delivered to the Person, while successive periods of Drug Exposures are combined under certain rules to produce continuous Drug Eras."@en ;
    rdfs:subClassOf [ a owl:Restriction ;
            owl:onProperty [ owl:inverseOf omop:has_drug_era ] ;
            owl:someValuesFrom omop:Person ],
        [ a owl:Restriction ;
            owl:allValuesFrom xsd:integer ;
            owl:onProperty omop:exposure_count ],
        [ a owl:Restriction ;
            owl:allValuesFrom xsd:integer ;
            owl:onProperty omop:gap_days ],
        omop:Era ;
    omop:omop_cdm_name "drug_era"^^xsd:string .

omop:Era a owl:Class ;
    rdfs:label "Era"^^xsd:string ;
    rdfs:subClassOf [ a owl:Restriction ;
            owl:allValuesFrom omop:Concept ;
            owl:onProperty omop:has_concept ],
        [ a owl:Restriction ;
            owl:onProperty omop:has_concept ;
            owl:someValuesFrom omop:Concept ],
        omop:ClinicalElement,
        omop:DatetimeDuration .

omop:LocationHistory a owl:Class ;
    rdfs:label "Location history"^^xsd:string ;
    rdfs:comment "The LOCATION HISTORY table stores relationships between Persons or Care Sites and geographic locations over time. **This table is new to CDM v6.0**"@en ;
    rdfs:subClassOf [ a owl:Restriction ;
            owl:allValuesFrom omop:Location ;
            owl:onProperty omop:has_location ],
        [ a owl:Restriction ;
            owl:onProperty omop:has_location ;
            owl:someValuesFrom omop:Location ],
        [ a owl:Restriction ;
            owl:allValuesFrom omop:Concept ;
            owl:onProperty omop:has_relationship_type ],
        [ a owl:Restriction ;
            owl:onProperty omop:has_relationship_type ;
            owl:someValuesFrom omop:Concept ],
        [ a owl:Restriction ;
            owl:allValuesFrom omop:Domain ;
            owl:onProperty omop:has_domain ],
        [ a owl:Restriction ;
            owl:onProperty omop:has_domain ;
            owl:someValuesFrom omop:Domain ],
        [ a owl:Restriction ;
            owl:allValuesFrom owl:Thing ;
            owl:onProperty omop:has_entity ],
        [ a owl:Restriction ;
            owl:onProperty omop:has_entity ;
            owl:someValuesFrom owl:Thing ],
        omop:DateDuration ;
    omop:omop_cdm_name "location_history"^^xsd:string .

omop:Occurrence a owl:Class ;
    rdfs:label "Occurrence"^^xsd:string ;
    rdfs:subClassOf omop:ClinicalElement .

omop:has_class a owl:FunctionalProperty,
        owl:ObjectProperty ;
    rdfs:label "Has class"^^xsd:string ;
    owlready:python_name "class"^^xsd:string ;
    rdfs:comment """For Concept: The attribute or concept class of the
Concept. Examples are 'Clinical Drug',
'Ingredient', 'Clinical Finding' etc."""@en,
        """For Note: A Standard Concept Id representing the HL7 LOINC
Document Type Vocabulary classification of the note.
Map the note classification to a Standard Concept. For more information see the ETL Conventions in the description of the NOTE table. [AcceptedConcepts](https://athena.ohdsi.org/search-terms/terms?standardConcept=Standard&conceptClass=Doc+Kind&conceptClass=Doc+Role&conceptClass=Doc+Setting&conceptClass=Doc+Subject+Matter&conceptClass=Doc+Type+of+Service&domain=Meas+Value&page=1&pageSize=15&query=). This Concept can alternatively be represented by concepts with the relationship 'Kind of (LOINC)' to [706391](https://athena.ohdsi.org/search-terms/terms/706391) (Note)."""@en ;
    rdfs:domain [ a owl:Class ;
            owl:unionOf ( omop:Concept omop:Note ) ] ;
    omop:omop_cdm_name "concept.concept_class_id#366 AS ConceptClass"^^xsd:string,
        "note.note_class_concept_id#184 AS Concept"^^xsd:string .

omop:has_domain a owl:FunctionalProperty,
        owl:ObjectProperty ;
    rdfs:label "Has domain"^^xsd:string ;
    owlready:python_name "domain"^^xsd:string ;
    rdfs:comment "For Concept: A foreign key to the [DOMAIN](https://ohdsi.github.io/CommonDataModel/cdm531.html#domain) table the Concept belongs to."@en,
        "For Location History: The domain of the entity that is related to the location. Either PERSON, PROVIDER, or CARE_SITE."@en ;
    rdfs:domain [ a owl:Class ;
            owl:unionOf ( omop:LocationHistory omop:Concept ) ] ;
    rdfs:range omop:Domain ;
    omop:omop_cdm_name "concept.domain_id#364 AS Domain"^^xsd:string,
        "location_history.domain_id#263 AS Domain"^^xsd:string .

omop:has_event a owl:FunctionalProperty,
        owl:ObjectProperty ;
    rdfs:label "Has event"^^xsd:string ;
    owlready:python_name "event"^^xsd:string ;
    rdfs:comment """For Cost: If the Cost record is related to another record in the database, this field is the primary key of the linked record.
Put the primary key of the linked record, if applicable, here."""@en,
        """For Observation: If the Observation record is related to another record in the database, this field is the primary key of the linked record.
Put the primary key of the linked record, if applicable, here. See the [ETL Conventions for the OBSERVATION](https://ohdsi.github.io/CommonDataModel/cdm60.html#observation) table for more details."""@en ;
    rdfs:domain [ a owl:Class ;
            owl:unionOf ( omop:Cost omop:Observation omop:Note ) ] ;
    omop:omop_cdm_name "cost.cost_event_id#309 AS Thing"^^xsd:string,
        "note.note_event_id#179 AS Thing"^^xsd:string,
        "observation.observation_event_id#167 AS Thing"^^xsd:string .

omop:has_language a owl:FunctionalProperty,
        owl:ObjectProperty ;
    rdfs:label "Has language"^^xsd:string ;
    owlready:python_name "language"^^xsd:string ;
    rdfs:comment """For Note: The language of the note.
Use Concepts that are descendants of the concept [4182347](https://athena.ohdsi.org/search-terms/terms/4182347) (World Languages)."""@en ;
    rdfs:domain [ a owl:Class ;
            owl:unionOf ( omop:ConceptSynonym omop:Note ) ] ;
    rdfs:range omop:Concept ;
    omop:omop_cdm_name "concept_synonym.language_concept_id#397 AS Concept"^^xsd:string,
        "note.language_concept_id#188 AS Concept"^^xsd:string .

omop:has_location a owl:FunctionalProperty,
        owl:ObjectProperty ;
    rdfs:label "Has location"^^xsd:string ;
    owlready:python_name "location"^^xsd:string ;
    rdfs:comment "For Care Site: The location_id from the LOCATION table representing the physical location of the care_site."@en,
        "For Location History: This is the LOCATION_ID for the LOCATION_HISTORY record."@en,
        """For Person: The location refers to the physical address of the person. This field should capture the last known location of the person.  Any prior locations are captured in the [LOCATION_HISTORY](https://ohdsi.github.io/CommonDataModel/cdm60.html#location_history) table.
Put the location_id from the LOCATION table here that represents the most granular location information for the person. This could represent anything from postal code or parts thereof, state, or county for example. Since many databases contain deidentified data, it is common that the precision of the location is reduced to prevent re-identification. This field should capture the last known location. Any prior locations are captured in the [LOCATION_HISTORY](https://ohdsi.github.io/CommonDataModel/cdm60.html#location_history) table."""@en ;
    rdfs:domain [ a owl:Class ;
            owl:unionOf ( omop:LocationHistory omop:CareSite omop:Person ) ] ;
    rdfs:range omop:Location ;
    omop:omop_cdm_name "care_site.location_id#270 AS Location"^^xsd:string,
        "location_history.location_id#261 AS Location"^^xsd:string,
        "person.location_id#10 AS Location"^^xsd:string .

omop:has_relationship a owl:FunctionalProperty,
        owl:ObjectProperty ;
    rdfs:label "Has relationship"^^xsd:string ;
    owlready:python_name "relationship"^^xsd:string ;
    rdfs:comment "For Concept Relationship: The relationship between CONCEPT_ID_1 and CONCEPT_ID_2. Please see the [Vocabulary Conventions](https://ohdsi.github.io/CommonDataModel/dataModelConventions.html#concept_relationships). for more information."@en ;
    rdfs:domain [ a owl:Class ;
            owl:unionOf ( omop:FactRelationship omop:ConceptRelationship ) ] ;
    omop:omop_cdm_name "concept_relationship.relationship_id#385 AS Relationship"^^xsd:string,
        "fact_relationship.relationship_concept_id#226 AS Concept"^^xsd:string .

omop:has_subject a owl:FunctionalProperty,
        owl:ObjectProperty ;
    rdfs:label "Has subject"^^xsd:string ;
    owlready:python_name "subject"^^xsd:string ;
    rdfs:comment "For Cohort Definition: This field contains a Concept that represents the domain of the subjects that are members of the cohort (e.g., Person, Provider, Visit)."@en ;
    rdfs:domain [ a owl:Class ;
            owl:unionOf ( omop:CohortDefinition omop:Cohort ) ] ;
    omop:omop_cdm_name "cohort.subject_id#424 AS Thing"^^xsd:string,
        "cohort_definition.subject_concept_id#432 AS Concept"^^xsd:string .

omop:has_visit_detail a owl:ObjectProperty ;
    rdfs:label "Has visit detail"^^xsd:string ;
    owlready:python_name "visit_details"^^xsd:string ;
    rdfs:comment """reversed relation, For Visit Detail: Use this field to link the VISIT_DETAIL record to its VISIT_OCCURRENCE.
Put the VISIT_OCCURRENCE_ID that subsumes the VISIT_DETAIL record here."""@en ;
    rdfs:domain [ a owl:Class ;
            owl:unionOf ( omop:Person omop:VisitOccurrence ) ] ;
    rdfs:range omop:VisitDetail ;
    omop:omop_cdm_name "visit_detail.person_id#43 AS Person"^^xsd:string,
        "visit_detail.visit_occurrence_id#60 AS VisitOccurrence"^^xsd:string .

omop:invalid_reason a owl:DatatypeProperty,
        owl:FunctionalProperty ;
    rdfs:label "Invalid reason"^^xsd:string ;
    rdfs:comment "For Concept Relationship: Reason the relationship was invalidated. Possible values are 'D' (deleted), 'U' (updated) or NULL."@en,
        """For Concept: Reason the Concept was invalidated.
Possible values are D (deleted), U
(replaced with an update) or NULL when
valid_end_date has the default value."""@en,
        "For Drug Strength: Reason the concept was invalidated. Possible values are D (deleted), U (replaced with an update) or NULL when valid_end_date has the default value."@en,
        """For Source To Concept Map: Reason the mapping instance was
invalidated. Possible values are D
(deleted), U (replaced with an
update) or NULL when
valid_end_date has the default
value."""@en ;
    rdfs:domain [ a owl:Class ;
            owl:unionOf ( omop:SourceToConceptMap omop:DrugStrength omop:Concept omop:ConceptRelationship ) ] ;
    rdfs:range xsd:string ;
    omop:omop_cdm_name "concept.invalid_reason#371 AS str"^^xsd:string,
        "concept_relationship.invalid_reason#388 AS str"^^xsd:string,
        "drug_strength.invalid_reason#422 AS str"^^xsd:string,
        "source_to_concept_map.invalid_reason#410 AS str"^^xsd:string .

omop:quantity a owl:DatatypeProperty,
        owl:FunctionalProperty ;
    rdfs:label "Quantity"^^xsd:string ;
    rdfs:comment """For Drug Exposure: To find the dose form of a drug the RELATIONSHIP table can be used where the relationship_id is 'Has dose form'. If liquid, quantity stands for the total amount dispensed or ordered of ingredient in the units given by the drug_strength table. If the unit from the source data does not align with the unit in the DRUG_STRENGTH table the quantity should be converted to the correct unit given in DRUG_STRENGTH. For clinical drugs with fixed dose forms (tablets etc.) the quantity is the number of units/tablets/capsules prescribed or dispensed (can be partial, but then only 1/2 or 1/3, not 0.01). Clinical drugs with divisible dose forms (injections) the quantity is the amount of ingredient the patient got. For example, if the injection is 2mg/mL but the patient got 80mL then quantity is reported as 160.
Quantified clinical drugs with divisible dose forms (prefilled syringes), the quantity is the amount of ingredient similar to clinical drugs. Please see [how to calculate drug dose](https://ohdsi.github.io/CommonDataModel/drug_dose.html) for more information.
"""@en,
        """For Procedure Occurrence: If the quantity value is omitted, a single procedure is assumed.
If a Procedure has a quantity of '0' in the source, this should default to '1' in the ETL. If there is a record in the source it can be assumed the exposure occurred at least once"""@en,
        "For Specimen: The amount of specimen collected from the person."@en ;
    rdfs:domain [ a owl:Class ;
            owl:unionOf ( omop:DrugExposure omop:Specimen omop:DeviceExposure omop:ProcedureOccurrence ) ] ;
    omop:omop_cdm_name "device_exposure.quantity#123 AS int"^^xsd:string,
        "drug_exposure.quantity#88 AS float"^^xsd:string,
        "procedure_occurrence.quantity#107 AS int"^^xsd:string,
        "specimen.quantity#213 AS float"^^xsd:string .

omop:ClinicalElement a owl:Class ;
    rdfs:label "Clinical element"^^xsd:string ;
    rdfs:subClassOf omop:OmopCDMThing .

omop:DeviceExposure a owl:Class ;
    rdfs:label "Device exposure"^^xsd:string ;
    rdfs:comment "The Device domain captures information about a person's exposure to a foreign physical object or instrument which is used for diagnostic or therapeutic purposes through a mechanism beyond chemical action. Devices include implantable objects (e.g. pacemakers, stents, artificial joints), medical equipment and supplies (e.g. bandages, crutches, syringes), other instruments used in medical procedures (e.g. sutures, defibrillators) and material used in clinical care (e.g. adhesives, body material, dental material, surgical material)."@en ;
    rdfs:subClassOf [ a owl:Restriction ;
            owl:allValuesFrom xsd:integer ;
            owl:onProperty omop:quantity ],
        [ a owl:Restriction ;
            owl:onProperty [ owl:inverseOf omop:has_device_exposure ] ;
            owl:someValuesFrom omop:Person ],
        [ a owl:Restriction ;
            owl:allValuesFrom owl:Thing ;
            owl:onProperty omop:has_unique_device ],
        omop:Exposure ;
    omop:omop_cdm_name "device_exposure"^^xsd:string .

omop:FactRelationship a owl:Class ;
    rdfs:label "Fact relationship"^^xsd:string ;
    rdfs:comment "The FACT_RELATIONSHIP table contains records about the relationships between facts stored as records in any table of the CDM. Relationships can be defined between facts from the same domain, or different domains. Examples of Fact Relationships include: [Person relationships](https://athena.ohdsi.org/search-terms/terms?domain=Relationship&standardConcept=Standard&page=2&pageSize=15&query=) (parent-child), care site relationships (hierarchical organizational structure of facilities within a health system), indication relationship (between drug exposures and associated conditions), usage relationships (of devices during the course of an associated procedure), or facts derived from one another (measurements derived from an associated specimen)."@en ;
    rdfs:subClassOf [ a owl:Restriction ;
            owl:allValuesFrom xsd:integer ;
            owl:onProperty omop:domain_concept_id_1 ],
        [ a owl:Restriction ;
            owl:onProperty omop:domain_concept_id_1 ;
            owl:someValuesFrom xsd:integer ],
        [ a owl:Restriction ;
            owl:allValuesFrom xsd:integer ;
            owl:onProperty omop:fact_id_1 ],
        [ a owl:Restriction ;
            owl:onProperty omop:fact_id_1 ;
            owl:someValuesFrom xsd:integer ],
        [ a owl:Restriction ;
            owl:allValuesFrom xsd:integer ;
            owl:onProperty omop:domain_concept_id_2 ],
        [ a owl:Restriction ;
            owl:onProperty omop:domain_concept_id_2 ;
            owl:someValuesFrom xsd:integer ],
        [ a owl:Restriction ;
            owl:allValuesFrom xsd:integer ;
            owl:onProperty omop:fact_id_2 ],
        [ a owl:Restriction ;
            owl:onProperty omop:fact_id_2 ;
            owl:someValuesFrom xsd:integer ],
        [ a owl:Restriction ;
            owl:allValuesFrom omop:Concept ;
            owl:onProperty omop:has_relationship ],
        [ a owl:Restriction ;
            owl:onProperty omop:has_relationship ;
            owl:someValuesFrom omop:Concept ],
        omop:OmopCDMThing ;
    omop:omop_cdm_name "fact_relationship"^^xsd:string .

omop:Metadata a owl:Class ;
    rdfs:label "Metadata"^^xsd:string ;
    rdfs:comment "The METADATA table contains metadata information about a dataset that has been transformed to the OMOP Common Data Model."@en ;
    rdfs:subClassOf [ a owl:Restriction ;
            owl:allValuesFrom omop:Concept ;
            owl:onProperty omop:has_concept ],
        [ a owl:Restriction ;
            owl:onProperty omop:has_concept ;
            owl:someValuesFrom omop:Concept ],
        [ a owl:Restriction ;
            owl:allValuesFrom omop:Concept ;
            owl:onProperty omop:has_type ],
        [ a owl:Restriction ;
            owl:onProperty omop:has_type ;
            owl:someValuesFrom omop:Concept ],
        [ a owl:Restriction ;
            owl:allValuesFrom omop:Concept ;
            owl:onProperty omop:has_value_as_concept ],
        [ a owl:Restriction ;
            owl:allValuesFrom xsd:string ;
            owl:onProperty omop:value_as_string ],
        [ a owl:Restriction ;
            owl:allValuesFrom xsd:string ;
            owl:onProperty omop:name ],
        [ a owl:Restriction ;
            owl:onProperty omop:name ;
            owl:someValuesFrom xsd:string ],
        omop:Event ;
    omop:omop_cdm_name "metadata"^^xsd:string .

omop:has_unit a owl:FunctionalProperty,
        owl:ObjectProperty ;
    rdfs:label "Has unit"^^xsd:string ;
    owlready:python_name "unit"^^xsd:string ;
    rdfs:comment "For Dose Era: The Concept Id representing the unit of the specific drug ingredient."@en,
        """For Measurement: There is currently no recommended unit for individual measurements, i.e. it is not mandatory to represent Hemoglobin a1C measurements as a percentage. UNIT_SOURCE_VALUES should be mapped to a Standard Concept in the Unit domain that best represents the unit as given in the source data.
There is no standardization requirement for units associated with MEASUREMENT_CONCEPT_IDs, however, it is the responsibility of the ETL to choose the most plausible unit."""@en,
        """For Observation: There is currently no recommended unit for individual observation concepts. UNIT_SOURCE_VALUES should be mapped to a Standard Concept in the Unit domain that best represents the unit as given in the source data.
There is no standardization requirement for units associated with OBSERVATION_CONCEPT_IDs, however, it is the responsibility of the ETL to choose the most plausible unit."""@en,
        """For Specimen: The unit for the quantity of the specimen.
Map the UNIT_SOURCE_VALUE to a Standard Concept in the Unit domain. [Accepted Concepts](https://athena.ohdsi.org/search-terms/terms?domain=Unit&standardConcept=Standard&page=1&pageSize=15&query=)"""@en ;
    rdfs:domain [ a owl:Class ;
            owl:unionOf ( omop:Observation omop:Measurement omop:DoseEra omop:Specimen ) ] ;
    rdfs:range omop:Concept ;
    omop:omop_cdm_name "dose_era.unit_concept_id#335 AS Concept"^^xsd:string,
        "measurement.unit_concept_id#139 AS Concept"^^xsd:string,
        "observation.unit_concept_id#159 AS Concept"^^xsd:string,
        "specimen.unit_concept_id#214 AS Concept"^^xsd:string .

omop:ConceptRelationship a owl:Class ;
    rdfs:label "Concept relationship"^^xsd:string ;
    rdfs:comment "The CONCEPT_RELATIONSHIP table contains records that define direct relationships between any two Concepts and the nature or type of the relationship. Each type of a relationship is defined in the RELATIONSHIP table."@en ;
    rdfs:subClassOf [ a owl:Restriction ;
            owl:allValuesFrom omop:Relationship ;
            owl:onProperty omop:has_relationship ],
        [ a owl:Restriction ;
            owl:onProperty omop:has_relationship ;
            owl:someValuesFrom omop:Relationship ],
        [ a owl:Restriction ;
            owl:allValuesFrom xsd:date ;
            owl:onProperty omop:valid_start_date ],
        [ a owl:Restriction ;
            owl:onProperty omop:valid_start_date ;
            owl:someValuesFrom xsd:date ],
        [ a owl:Restriction ;
            owl:allValuesFrom xsd:date ;
            owl:onProperty omop:valid_end_date ],
        [ a owl:Restriction ;
            owl:onProperty omop:valid_end_date ;
            owl:someValuesFrom xsd:date ],
        [ a owl:Restriction ;
            owl:allValuesFrom xsd:string ;
            owl:onProperty omop:invalid_reason ],
        [ a owl:Restriction ;
            owl:allValuesFrom xsd:integer ;
            owl:onProperty omop:concept_id_1 ],
        [ a owl:Restriction ;
            owl:onProperty omop:concept_id_1 ;
            owl:someValuesFrom xsd:integer ],
        [ a owl:Restriction ;
            owl:allValuesFrom xsd:integer ;
            owl:onProperty omop:concept_id_2 ],
        [ a owl:Restriction ;
            owl:onProperty omop:concept_id_2 ;
            owl:someValuesFrom xsd:integer ],
        omop:OmopCDMThing ;
    omop:omop_cdm_name "concept_relationship"^^xsd:string .

omop:DatetimeDuration a owl:Class ;
    rdfs:label "Datetime duration"^^xsd:string ;
    rdfs:subClassOf [ a owl:Restriction ;
            owl:allValuesFrom xsd:dateTime ;
            owl:onProperty omop:start_datetime ],
        [ a owl:Restriction ;
            owl:allValuesFrom xsd:dateTime ;
            owl:onProperty omop:end_datetime ],
        omop:Duration .

omop:Death a owl:Class ;
    rdfs:label "Death"^^xsd:string ;
    rdfs:subClassOf [ a owl:Restriction ;
            owl:allValuesFrom omop:Concept ;
            owl:onProperty omop:has_type ],
        [ a owl:Restriction ;
            owl:allValuesFrom omop:Concept ;
            owl:onProperty omop:has_cause ],
        [ a owl:Restriction ;
            owl:allValuesFrom xsd:string ;
            owl:onProperty omop:cause_source_value ],
        [ a owl:Restriction ;
            owl:allValuesFrom omop:Concept ;
            owl:onProperty omop:has_cause_source ],
        omop:Event ;
    omop:omop_cdm_name "death"^^xsd:string .

omop:BasePerson a owl:Class ;
    rdfs:label "Base person"^^xsd:string ;
    rdfs:subClassOf [ a owl:Restriction ;
            owl:allValuesFrom omop:Concept ;
            owl:onProperty omop:has_gender ],
        [ a owl:Restriction ;
            owl:onProperty omop:has_gender ;
            owl:someValuesFrom omop:Concept ],
        [ a owl:Restriction ;
            owl:allValuesFrom omop:CareSite ;
            owl:onProperty omop:has_care_site ],
        [ a owl:Restriction ;
            owl:allValuesFrom xsd:string ;
            owl:onProperty omop:source_value ],
        [ a owl:Restriction ;
            owl:allValuesFrom xsd:string ;
            owl:onProperty omop:gender_source_value ],
        [ a owl:Restriction ;
            owl:allValuesFrom omop:Concept ;
            owl:onProperty omop:has_gender_source ],
        [ a owl:Restriction ;
            owl:onProperty omop:has_gender_source ;
            owl:someValuesFrom omop:Concept ],
        omop:OmopCDMThing .

omop:Domain a owl:Class ;
    rdfs:label "Domain"^^xsd:string ;
    rdfs:comment "The DOMAIN table includes a list of OMOP-defined Domains the Concepts of the Standardized Vocabularies can belong to. A Domain defines the set of allowable Concepts for the standardized fields in the CDM tables. For example, the \"Condition\" Domain contains Concepts that describe a condition of a patient, and these Concepts can only be stored in the condition_concept_id field of the CONDITION_OCCURRENCE and CONDITION_ERA tables. This reference table is populated with a single record for each Domain and includes a descriptive name for the Domain."@en ;
    rdfs:subClassOf [ a owl:Restriction ;
            owl:allValuesFrom omop:Concept ;
            owl:onProperty omop:has_concept ],
        [ a owl:Restriction ;
            owl:onProperty omop:has_concept ;
            owl:someValuesFrom omop:Concept ],
        [ a owl:Restriction ;
            owl:allValuesFrom xsd:string ;
            owl:onProperty omop:name ],
        [ a owl:Restriction ;
            owl:onProperty omop:name ;
            owl:someValuesFrom xsd:string ],
        omop:OmopCDMThing ;
    omop:omop_cdm_name "domain"^^xsd:string .

omop:Exposure a owl:Class ;
    rdfs:label "Exposure"^^xsd:string ;
    rdfs:subClassOf [ a owl:Restriction ;
            owl:allValuesFrom omop:Concept ;
            owl:onProperty omop:has_concept ],
        [ a owl:Restriction ;
            owl:onProperty omop:has_concept ;
            owl:someValuesFrom omop:Concept ],
        [ a owl:Restriction ;
            owl:allValuesFrom omop:Concept ;
            owl:onProperty omop:has_type ],
        [ a owl:Restriction ;
            owl:onProperty omop:has_type ;
            owl:someValuesFrom omop:Concept ],
        [ a owl:Restriction ;
            owl:allValuesFrom omop:Concept ;
            owl:onProperty omop:has_source ],
        [ a owl:Restriction ;
            owl:onProperty omop:has_source ;
            owl:someValuesFrom omop:Concept ],
        [ a owl:Restriction ;
            owl:allValuesFrom omop:Provider ;
            owl:onProperty omop:has_provider ],
        [ a owl:Restriction ;
            owl:allValuesFrom xsd:string ;
            owl:onProperty omop:source_value ],
        omop:ClinicalElement,
        omop:DateDuration,
        omop:DatetimeDuration .

omop:Relationship a owl:Class ;
    rdfs:label "Relationship"^^xsd:string ;
    rdfs:comment "The RELATIONSHIP table provides a reference list of all types of relationships that can be used to associate any two concepts in the CONCEPT_RELATIONSHP table."@en ;
    rdfs:subClassOf [ a owl:Restriction ;
            owl:allValuesFrom omop:Concept ;
            owl:onProperty omop:has_concept ],
        [ a owl:Restriction ;
            owl:onProperty omop:has_concept ;
            owl:someValuesFrom omop:Concept ],
        [ a owl:Restriction ;
            owl:allValuesFrom xsd:string ;
            owl:onProperty omop:name ],
        [ a owl:Restriction ;
            owl:onProperty omop:name ;
            owl:someValuesFrom xsd:string ],
        [ a owl:Restriction ;
            owl:allValuesFrom xsd:string ;
            owl:onProperty omop:is_hierarchical ],
        [ a owl:Restriction ;
            owl:onProperty omop:is_hierarchical ;
            owl:someValuesFrom xsd:string ],
        [ a owl:Restriction ;
            owl:allValuesFrom xsd:string ;
            owl:onProperty omop:defines_ancestry ],
        [ a owl:Restriction ;
            owl:onProperty omop:defines_ancestry ;
            owl:someValuesFrom xsd:string ],
        [ a owl:Restriction ;
            owl:allValuesFrom owl:Thing ;
            owl:onProperty omop:has_reverse_relationship ],
        [ a owl:Restriction ;
            owl:onProperty omop:has_reverse_relationship ;
            owl:someValuesFrom owl:Thing ],
        omop:OmopCDMThing ;
    omop:omop_cdm_name "relationship"^^xsd:string .

omop:CareSite a owl:Class ;
    rdfs:label "Care site"^^xsd:string ;
    rdfs:comment "The CARE_SITE table contains a list of uniquely identified institutional (physical or organizational) units where healthcare delivery is practiced (offices, wards, hospitals, clinics, etc.)."@en ;
    rdfs:subClassOf [ a owl:Restriction ;
            owl:allValuesFrom omop:Location ;
            owl:onProperty omop:has_location ],
        [ a owl:Restriction ;
            owl:allValuesFrom xsd:string ;
            owl:onProperty omop:name ],
        [ a owl:Restriction ;
            owl:allValuesFrom omop:Concept ;
            owl:onProperty omop:has_place_of_service ],
        [ a owl:Restriction ;
            owl:onProperty omop:has_place_of_service ;
            owl:someValuesFrom omop:Concept ],
        [ a owl:Restriction ;
            owl:allValuesFrom xsd:string ;
            owl:onProperty omop:place_of_service_source_value ],
        [ a owl:Restriction ;
            owl:allValuesFrom xsd:string ;
            owl:onProperty omop:source_value ],
        omop:OmopCDMThing ;
    omop:omop_cdm_name "care_site"^^xsd:string .

omop:valid_end_date a owl:DatatypeProperty,
        owl:FunctionalProperty ;
    rdfs:label "Valid end date"^^xsd:string ;
    rdfs:comment "For Concept Relationship: The date when the relationship is invalidated."@en,
        """For Concept: The date when the Concept became
invalid because it was deleted or
superseded (updated) by a new concept.
The default value is 31-Dec-2099,
meaning, the Concept is valid until it
becomes deprecated."""@en,
        "For Drug Strength: The date when then Concept became invalid."@en,
        """For Source To Concept Map: The date when the mapping
instance became invalid because it
was deleted or superseded
(updated) by a new relationship.
Default value is 31-Dec-2099."""@en ;
    rdfs:domain [ a owl:Class ;
            owl:unionOf ( omop:SourceToConceptMap omop:DrugStrength omop:Concept omop:ConceptRelationship ) ] ;
    rdfs:range xsd:date ;
    omop:omop_cdm_name "concept.valid_end_date#370 AS date"^^xsd:string,
        "concept_relationship.valid_end_date#387 AS date"^^xsd:string,
        "drug_strength.valid_end_date#421 AS date"^^xsd:string,
        "source_to_concept_map.valid_end_date#409 AS date"^^xsd:string .

omop:valid_start_date a owl:DatatypeProperty,
        owl:FunctionalProperty ;
    rdfs:label "Valid start date"^^xsd:string ;
    rdfs:comment "For Concept Relationship: The date when the relationship is first recorded."@en,
        """For Concept: The date when the Concept was first
recorded. The default value is
1-Jan-1970, meaning, the Concept has no
(known) date of inception."""@en,
        """For Drug Strength: The date when the Concept was first
recorded. The default value is
1-Jan-1970."""@en,
        """For Source To Concept Map: The date when the mapping
instance was first recorded."""@en ;
    rdfs:domain [ a owl:Class ;
            owl:unionOf ( omop:SourceToConceptMap omop:DrugStrength omop:Concept omop:ConceptRelationship ) ] ;
    rdfs:range xsd:date ;
    omop:omop_cdm_name "concept.valid_start_date#369 AS date"^^xsd:string,
        "concept_relationship.valid_start_date#386 AS date"^^xsd:string,
        "drug_strength.valid_start_date#420 AS date"^^xsd:string,
        "source_to_concept_map.valid_start_date#408 AS date"^^xsd:string .

omop:CohortDefinition a owl:Class ;
    rdfs:label "Cohort definition"^^xsd:string ;
    rdfs:comment "The COHORT_DEFINITION table contains records defining a Cohort derived from the data through the associated description and syntax and upon instantiation (execution of the algorithm) placed into the COHORT table. Cohorts are a set of subjects that satisfy a given combination of inclusion criteria for a duration of time. The COHORT_DEFINITION table provides a standardized structure for maintaining the rules governing the inclusion of a subject into a cohort, and can store operational programming code to instantiate the cohort within the OMOP Common Data Model."@en ;
    rdfs:subClassOf [ a owl:Restriction ;
            owl:allValuesFrom xsd:string ;
            owl:onProperty omop:name ],
        [ a owl:Restriction ;
            owl:onProperty omop:name ;
            owl:someValuesFrom xsd:string ],
        [ a owl:Restriction ;
            owl:allValuesFrom omop:Concept ;
            owl:onProperty omop:has_subject ],
        [ a owl:Restriction ;
            owl:onProperty omop:has_subject ;
            owl:someValuesFrom omop:Concept ],
        [ a owl:Restriction ;
            owl:allValuesFrom xsd:string ;
            owl:onProperty omop:description ],
        [ a owl:Restriction ;
            owl:allValuesFrom omop:Concept ;
            owl:onProperty omop:has_definition_type ],
        [ a owl:Restriction ;
            owl:onProperty omop:has_definition_type ;
            owl:someValuesFrom omop:Concept ],
        [ a owl:Restriction ;
            owl:allValuesFrom xsd:string ;
            owl:onProperty omop:syntax ],
        [ a owl:Restriction ;
            owl:allValuesFrom xsd:date ;
            owl:onProperty omop:cohort_initiation_date ],
        omop:OmopCDMThing ;
    omop:omop_cdm_name "cohort_definition"^^xsd:string .

omop:DateDuration a owl:Class ;
    rdfs:label "Date duration"^^xsd:string ;
    rdfs:subClassOf [ a owl:Restriction ;
            owl:allValuesFrom xsd:date ;
            owl:onProperty omop:start_date ],
        [ a owl:Restriction ;
            owl:allValuesFrom xsd:date ;
            owl:onProperty omop:end_date ],
        omop:Duration .

omop:SourceToConceptMap a owl:Class ;
    rdfs:label "Source to concept map"^^xsd:string ;
    rdfs:comment "The source to concept map table is a legacy data structure within the OMOP Common Data Model, recommended for use in ETL processes to maintain local source codes which are not available as Concepts in the Standardized Vocabularies, and to establish mappings for each source code into a Standard Concept as target_concept_ids that can be used to populate the Common Data Model tables. The SOURCE_TO_CONCEPT_MAP table is no longer populated with content within the Standardized Vocabularies published to the OMOP community."@en ;
    rdfs:subClassOf [ a owl:Restriction ;
            owl:allValuesFrom omop:Concept ;
            owl:onProperty omop:has_source ],
        [ a owl:Restriction ;
            owl:onProperty omop:has_source ;
            owl:someValuesFrom omop:Concept ],
        [ a owl:Restriction ;
            owl:allValuesFrom xsd:date ;
            owl:onProperty omop:valid_start_date ],
        [ a owl:Restriction ;
            owl:onProperty omop:valid_start_date ;
            owl:someValuesFrom xsd:date ],
        [ a owl:Restriction ;
            owl:allValuesFrom xsd:date ;
            owl:onProperty omop:valid_end_date ],
        [ a owl:Restriction ;
            owl:onProperty omop:valid_end_date ;
            owl:someValuesFrom xsd:date ],
        [ a owl:Restriction ;
            owl:allValuesFrom xsd:string ;
            owl:onProperty omop:invalid_reason ],
        [ a owl:Restriction ;
            owl:allValuesFrom xsd:string ;
            owl:onProperty omop:source_code ],
        [ a owl:Restriction ;
            owl:onProperty omop:source_code ;
            owl:someValuesFrom xsd:string ],
        [ a owl:Restriction ;
            owl:allValuesFrom omop:Vocabulary ;
            owl:onProperty omop:has_source_vocabulary ],
        [ a owl:Restriction ;
            owl:onProperty omop:has_source_vocabulary ;
            owl:someValuesFrom omop:Vocabulary ],
        [ a owl:Restriction ;
            owl:allValuesFrom xsd:string ;
            owl:onProperty omop:source_code_description ],
        [ a owl:Restriction ;
            owl:allValuesFrom omop:Concept ;
            owl:onProperty omop:has_target ],
        [ a owl:Restriction ;
            owl:onProperty omop:has_target ;
            owl:someValuesFrom omop:Concept ],
        [ a owl:Restriction ;
            owl:allValuesFrom omop:Vocabulary ;
            owl:onProperty omop:has_target_vocabulary ],
        [ a owl:Restriction ;
            owl:onProperty omop:has_target_vocabulary ;
            owl:someValuesFrom omop:Vocabulary ],
        omop:OmopCDMThing ;
    omop:omop_cdm_name "source_to_concept_map"^^xsd:string .

omop:has_provider a owl:FunctionalProperty,
        owl:ObjectProperty ;
    rdfs:label "Has provider"^^xsd:string ;
    owlready:python_name "provider"^^xsd:string ;
    rdfs:comment """For Condition Occurrence: The provider associated with condition record, e.g. the provider who made the diagnosis or the provider who recorded the symptom.
The ETL may need to make a choice as to which PROVIDER_ID to put here. Based on what is available this may or may not be different than the provider associated with the overall VISIT_OCCURRENCE record, for example the admitting vs attending physician on an EHR record."""@en,
        """For Device Exposure: The Provider associated with device record, e.g. the provider who wrote the prescription or the provider who implanted the device.
The ETL may need to make a choice as to which PROVIDER_ID to put here. Based on what is available this may or may not be different than the provider associated with the overall VISIT_OCCURRENCE record."""@en,
        """For Drug Exposure: The Provider associated with drug record, e.g. the provider who wrote the prescription or the provider who administered the drug.
The ETL may need to make a choice as to which PROVIDER_ID to put here. Based on what is available this may or may not be different than the provider associated with the overall VISIT_OCCURRENCE record, for example the ordering vs administering physician on an EHR record."""@en,
        """For Measurement: The provider associated with measurement record, e.g. the provider who ordered the test or the provider who recorded the result.
The ETL may need to make a choice as to which PROVIDER_ID to put here. Based on what is available this may or may not be different than the provider associated with the overall VISIT_OCCURRENCE record. For example the admitting vs attending physician on an EHR record."""@en,
        """For Note: The Provider who wrote the note.
The ETL may need to make a determination on which provider to put here."""@en,
        """For Observation: The provider associated with the observation record, e.g. the provider who ordered the test or the provider who recorded the result.
The ETL may need to make a choice as to which PROVIDER_ID to put here. Based on what is available this may or may not be different than the provider associated with the overall VISIT_OCCURRENCE record. For example the admitting vs attending physician on an EHR record."""@en,
        """For Person: The Provider refers to the last known primary care provider (General Practitioner).
Put the provider_id from the PROVIDER table of the last known general practitioner of the person. If there are multiple providers, it is up to the ETL to decide which to put here."""@en,
        """For Procedure Occurrence: The provider associated with the procedure record, e.g. the provider who performed the Procedure.
The ETL may need to make a choice as to which PROVIDER_ID to put here. Based on what is available this may or may not be different than the provider associated with the overall VISIT_OCCURRENCE record, for example the admitting vs attending physician on an EHR record."""@en,
        """For Survey Conduct: This is the Provider associated with the survey completion.
The ETL may need to make a choice as to which Provider to put here. This could either be the provider that ordered the survey or the provider who observed the completion of the survey."""@en,
        """For Visit Detail: There will only be one provider per  **visit** record and the ETL document should clearly state how they were chosen (attending, admitting, etc.). This is a typical reason for leveraging the VISIT_DETAIL table as even though each VISIT_DETAIL record can only have one provider, there is no limit to the number of VISIT_DETAIL records that can be associated to a VISIT_OCCURRENCE record.
The additional providers associated to a Visit can be stored in this table where each VISIT_DETAIL record represents a different provider."""@en,
        """For Visit Occurrence: There will only be one provider per visit record and the ETL document should clearly state how they were chosen (attending, admitting, etc.). If there are multiple providers associated with a visit in the source, this can be reflected in the event tables (CONDITION_OCCURRENCE, PROCEDURE_OCCURRENCE, etc.) or in the VISIT_DETAIL table.
If there are multiple providers associated with a visit, you will need to choose which one to put here. The additional providers can be stored in the visit_detail table."""@en ;
    rdfs:domain [ a owl:Class ;
            owl:unionOf ( omop:ProcedureOccurrence omop:BaseVisit omop:Person omop:ConditionOccurrence omop:Exposure omop:Measurement omop:Note omop:Observation omop:SurveyConduct ) ] ;
    rdfs:range omop:Provider ;
    omop:omop_cdm_name "condition_occurrence.provider_id#71 AS Provider"^^xsd:string,
        "device_exposure.provider_id#124 AS Provider"^^xsd:string,
        "drug_exposure.provider_id#93 AS Provider"^^xsd:string,
        "measurement.provider_id#142 AS Provider"^^xsd:string,
        "note.provider_id#189 AS Provider"^^xsd:string,
        "observation.provider_id#160 AS Provider"^^xsd:string,
        "person.provider_id#11 AS Provider"^^xsd:string,
        "procedure_occurrence.provider_id#108 AS Provider"^^xsd:string,
        "survey_conduct.provider_id#234 AS Provider"^^xsd:string,
        "visit_detail.provider_id#50 AS Provider"^^xsd:string,
        "visit_occurrence.provider_id#33 AS Provider"^^xsd:string .

omop:CdmSource a owl:Class ;
    rdfs:label "Cdm source"^^xsd:string ;
    rdfs:comment "The CDM_SOURCE table contains detail about the source database and the process used to transform the data into the OMOP Common Data Model."@en ;
    rdfs:subClassOf [ a owl:Restriction ;
            owl:allValuesFrom xsd:string ;
            owl:onProperty omop:name ],
        [ a owl:Restriction ;
            owl:onProperty omop:name ;
            owl:someValuesFrom xsd:string ],
        [ a owl:Restriction ;
            owl:allValuesFrom xsd:string ;
            owl:onProperty omop:abbreviation ],
        [ a owl:Restriction ;
            owl:allValuesFrom xsd:string ;
            owl:onProperty omop:cdm_holder ],
        [ a owl:Restriction ;
            owl:allValuesFrom xsd:string ;
            owl:onProperty omop:source_description ],
        [ a owl:Restriction ;
            owl:allValuesFrom xsd:string ;
            owl:onProperty omop:source_documentation_reference ],
        [ a owl:Restriction ;
            owl:allValuesFrom xsd:string ;
            owl:onProperty omop:cdm_etl_reference ],
        [ a owl:Restriction ;
            owl:allValuesFrom xsd:date ;
            owl:onProperty omop:source_release_date ],
        [ a owl:Restriction ;
            owl:allValuesFrom xsd:date ;
            owl:onProperty omop:cdm_release_date ],
        [ a owl:Restriction ;
            owl:allValuesFrom xsd:string ;
            owl:onProperty omop:cdm_version ],
        [ a owl:Restriction ;
            owl:allValuesFrom xsd:string ;
            owl:onProperty omop:vocabulary_version ],
        omop:OmopCDMThing ;
    omop:omop_cdm_name "cdm_source"^^xsd:string .

omop:Event a owl:Class ;
    rdfs:label "Event"^^xsd:string ;
    rdfs:subClassOf [ a owl:Restriction ;
            owl:allValuesFrom xsd:date ;
            owl:onProperty omop:date ],
        [ a owl:Restriction ;
            owl:allValuesFrom xsd:dateTime ;
            owl:onProperty omop:datetime ],
        omop:OmopCDMThing .

omop:ConditionOccurrence a owl:Class ;
    rdfs:label "Condition occurrence"^^xsd:string ;
    rdfs:comment "This table contains records of Events of a Person suggesting the presence of a disease or medical condition stated as a diagnosis, a sign, or a symptom, which is either observed by a Provider or reported by the patient."@en ;
    rdfs:subClassOf [ a owl:Restriction ;
            owl:allValuesFrom omop:Concept ;
            owl:onProperty omop:has_concept ],
        [ a owl:Restriction ;
            owl:onProperty omop:has_concept ;
            owl:someValuesFrom omop:Concept ],
        [ a owl:Restriction ;
            owl:allValuesFrom omop:Concept ;
            owl:onProperty omop:has_type ],
        [ a owl:Restriction ;
            owl:onProperty omop:has_type ;
            owl:someValuesFrom omop:Concept ],
        [ a owl:Restriction ;
            owl:allValuesFrom omop:Concept ;
            owl:onProperty omop:has_source ],
        [ a owl:Restriction ;
            owl:onProperty omop:has_source ;
            owl:someValuesFrom omop:Concept ],
        [ a owl:Restriction ;
            owl:onProperty [ owl:inverseOf omop:has_condition_occurrence ] ;
            owl:someValuesFrom omop:Person ],
        [ a owl:Restriction ;
            owl:allValuesFrom omop:Concept ;
            owl:onProperty omop:has_status ],
        [ a owl:Restriction ;
            owl:onProperty omop:has_status ;
            owl:someValuesFrom omop:Concept ],
        [ a owl:Restriction ;
            owl:allValuesFrom xsd:string ;
            owl:onProperty omop:stop_reason ],
        [ a owl:Restriction ;
            owl:allValuesFrom xsd:string ;
            owl:onProperty omop:status_source_value ],
        [ a owl:Restriction ;
            owl:allValuesFrom omop:Provider ;
            owl:onProperty omop:has_provider ],
        [ a owl:Restriction ;
            owl:allValuesFrom xsd:string ;
            owl:onProperty omop:source_value ],
        omop:DateDuration,
        omop:DatetimeDuration,
        omop:Occurrence ;
    omop:omop_cdm_name "condition_occurrence"^^xsd:string .

omop:ProcedureOccurrence a owl:Class ;
    rdfs:label "Procedure occurrence"^^xsd:string ;
    rdfs:comment "This table contains records of activities or processes ordered by, or carried out by, a healthcare provider on the patient with a diagnostic or therapeutic purpose."@en ;
    rdfs:subClassOf [ a owl:Restriction ;
            owl:allValuesFrom omop:Concept ;
            owl:onProperty omop:has_concept ],
        [ a owl:Restriction ;
            owl:onProperty omop:has_concept ;
            owl:someValuesFrom omop:Concept ],
        [ a owl:Restriction ;
            owl:allValuesFrom omop:Concept ;
            owl:onProperty omop:has_type ],
        [ a owl:Restriction ;
            owl:onProperty omop:has_type ;
            owl:someValuesFrom omop:Concept ],
        [ a owl:Restriction ;
            owl:allValuesFrom omop:Concept ;
            owl:onProperty omop:has_source ],
        [ a owl:Restriction ;
            owl:onProperty omop:has_source ;
            owl:someValuesFrom omop:Concept ],
        [ a owl:Restriction ;
            owl:allValuesFrom xsd:integer ;
            owl:onProperty omop:quantity ],
        [ a owl:Restriction ;
            owl:onProperty [ owl:inverseOf omop:has_procedure_occurrence ] ;
            owl:someValuesFrom omop:Person ],
        [ a owl:Restriction ;
            owl:allValuesFrom omop:Concept ;
            owl:onProperty omop:has_modifier ],
        [ a owl:Restriction ;
            owl:allValuesFrom xsd:string ;
            owl:onProperty omop:modifier_source_value ],
        [ a owl:Restriction ;
            owl:allValuesFrom omop:Provider ;
            owl:onProperty omop:has_provider ],
        [ a owl:Restriction ;
            owl:allValuesFrom xsd:string ;
            owl:onProperty omop:source_value ],
        omop:Event,
        omop:Occurrence ;
    omop:omop_cdm_name "procedure_occurrence"^^xsd:string .

omop:VisitDetail a owl:Class ;
    rdfs:label "Visit detail"^^xsd:string ;
    rdfs:comment "The VISIT_DETAIL table is an optional table used to represents details of each record in the parent VISIT_OCCURRENCE table. A good example of this would be the movement between units in a hospital during an inpatient stay or claim lines associated with a one insurance claim. For every record in the VISIT_OCCURRENCE table there may be 0 or more records in the VISIT_DETAIL table with a 1:n relationship where n may be 0. The VISIT_DETAIL table is structurally very similar to VISIT_OCCURRENCE table and belongs to the visit domain."@en ;
    rdfs:subClassOf [ a owl:Restriction ;
            owl:allValuesFrom omop:Concept ;
            owl:onProperty omop:has_admitted_from ],
        [ a owl:Restriction ;
            owl:allValuesFrom xsd:integer ;
            owl:onProperty omop:admitted_from_source_value ],
        [ a owl:Restriction ;
            owl:onProperty omop:admitted_from_source_value ;
            owl:someValuesFrom xsd:integer ],
        [ a owl:Restriction ;
            owl:onProperty [ owl:inverseOf omop:has_visit_detail ] ;
            owl:someValuesFrom omop:Person ],
        [ a owl:Restriction ;
            owl:onProperty [ owl:inverseOf omop:has_visit_detail ] ;
            owl:someValuesFrom omop:VisitOccurrence ],
        [ a owl:Restriction ;
            owl:allValuesFrom omop:VisitDetail ;
            owl:onProperty omop:has_preceding_visit_detail ],
        [ a owl:Restriction ;
            owl:allValuesFrom omop:VisitDetail ;
            owl:onProperty omop:has_parent ],
        omop:BaseVisit ;
    omop:omop_cdm_name "visit_detail"^^xsd:string .

omop:DrugStrength a owl:Class ;
    rdfs:label "Drug strength"^^xsd:string ;
    rdfs:comment "The DRUG_STRENGTH table contains structured content about the amount or concentration and associated units of a specific ingredient contained within a particular drug product. This table is supplemental information to support standardized analysis of drug utilization."@en ;
    rdfs:subClassOf [ a owl:Restriction ;
            owl:allValuesFrom omop:Concept ;
            owl:onProperty omop:has_concept ],
        [ a owl:Restriction ;
            owl:onProperty omop:has_concept ;
            owl:someValuesFrom omop:Concept ],
        [ a owl:Restriction ;
            owl:allValuesFrom xsd:date ;
            owl:onProperty omop:valid_start_date ],
        [ a owl:Restriction ;
            owl:onProperty omop:valid_start_date ;
            owl:someValuesFrom xsd:date ],
        [ a owl:Restriction ;
            owl:allValuesFrom xsd:date ;
            owl:onProperty omop:valid_end_date ],
        [ a owl:Restriction ;
            owl:onProperty omop:valid_end_date ;
            owl:someValuesFrom xsd:date ],
        [ a owl:Restriction ;
            owl:allValuesFrom xsd:string ;
            owl:onProperty omop:invalid_reason ],
        [ a owl:Restriction ;
            owl:allValuesFrom omop:Concept ;
            owl:onProperty omop:has_ingredient ],
        [ a owl:Restriction ;
            owl:onProperty omop:has_ingredient ;
            owl:someValuesFrom omop:Concept ],
        [ a owl:Restriction ;
            owl:allValuesFrom xsd:decimal ;
            owl:onProperty omop:amount_value ],
        [ a owl:Restriction ;
            owl:allValuesFrom omop:Concept ;
            owl:onProperty omop:has_amount_unit ],
        [ a owl:Restriction ;
            owl:allValuesFrom xsd:decimal ;
            owl:onProperty omop:numerator_value ],
        [ a owl:Restriction ;
            owl:allValuesFrom omop:Concept ;
            owl:onProperty omop:has_numerator_unit ],
        [ a owl:Restriction ;
            owl:allValuesFrom xsd:decimal ;
            owl:onProperty omop:denominator_value ],
        [ a owl:Restriction ;
            owl:allValuesFrom omop:Concept ;
            owl:onProperty omop:has_denominator_unit ],
        [ a owl:Restriction ;
            owl:allValuesFrom xsd:integer ;
            owl:onProperty omop:box_size ],
        omop:OmopCDMThing ;
    omop:omop_cdm_name "drug_strength"^^xsd:string .

omop:NoteNlp a owl:Class ;
    rdfs:label "Note nlp"^^xsd:string ;
    rdfs:comment "The NOTE_NLP table encodes all output of NLP on clinical notes. Each row represents a single extracted term from a note."@en ;
    rdfs:subClassOf [ a owl:Restriction ;
            owl:allValuesFrom omop:Concept ;
            owl:onProperty omop:has_concept ],
        [ a owl:Restriction ;
            owl:allValuesFrom omop:Concept ;
            owl:onProperty omop:has_source ],
        [ a owl:Restriction ;
            owl:onProperty [ owl:inverseOf omop:has_note_nlp ] ;
            owl:someValuesFrom omop:Note ],
        [ a owl:Restriction ;
            owl:allValuesFrom omop:Concept ;
            owl:onProperty omop:has_section ],
        [ a owl:Restriction ;
            owl:allValuesFrom xsd:string ;
            owl:onProperty omop:snippet ],
        [ a owl:Restriction ;
            owl:allValuesFrom xsd:string ;
            owl:onProperty omop:offset ],
        [ a owl:Restriction ;
            owl:allValuesFrom xsd:string ;
            owl:onProperty omop:lexical_variant ],
        [ a owl:Restriction ;
            owl:onProperty omop:lexical_variant ;
            owl:someValuesFrom xsd:string ],
        [ a owl:Restriction ;
            owl:allValuesFrom xsd:string ;
            owl:onProperty omop:system ],
        [ a owl:Restriction ;
            owl:allValuesFrom xsd:string ;
            owl:onProperty omop:term_exists ],
        [ a owl:Restriction ;
            owl:allValuesFrom xsd:string ;
            owl:onProperty omop:term_temporal ],
        [ a owl:Restriction ;
            owl:allValuesFrom xsd:string ;
            owl:onProperty omop:term_modifiers ],
        omop:Event ;
    omop:omop_cdm_name "note_nlp"^^xsd:string .

omop:VisitOccurrence a owl:Class ;
    rdfs:label "Visit occurrence"^^xsd:string ;
    rdfs:comment "This table contains Events where Persons engage with the healthcare system for a duration of time. They are often also called \"Encounters\". Visits are defined by a configuration of circumstances under which they occur, such as (i) whether the patient comes to a healthcare institution, the other way around, or the interaction is remote, (ii) whether and what kind of trained medical staff is delivering the service during the Visit, and (iii) whether the Visit is transient or for a longer period involving a stay in bed."@en ;
    rdfs:subClassOf [ a owl:Restriction ;
            owl:onProperty [ owl:inverseOf omop:has_visit_occurrence ] ;
            owl:someValuesFrom omop:Person ],
        [ a owl:Restriction ;
            owl:allValuesFrom omop:Concept ;
            owl:onProperty omop:has_admitted_from ],
        [ a owl:Restriction ;
            owl:onProperty omop:has_admitted_from ;
            owl:someValuesFrom omop:Concept ],
        [ a owl:Restriction ;
            owl:allValuesFrom xsd:string ;
            owl:onProperty omop:admitted_from_source_value ],
        [ a owl:Restriction ;
            owl:allValuesFrom omop:VisitOccurrence ;
            owl:onProperty omop:has_preceding_visit_occurrence ],
        [ a owl:Restriction ;
            owl:allValuesFrom omop:VisitDetail ;
            owl:onProperty omop:has_visit_detail ],
        [ a owl:Restriction ;
            owl:allValuesFrom omop:SurveyConduct ;
            owl:onProperty omop:has_survey_conduct ],
        omop:BaseVisit ;
    omop:omop_cdm_name "visit_occurrence"^^xsd:string .

omop:source_value a owl:DatatypeProperty,
        owl:FunctionalProperty ;
    rdfs:label "Source value"^^xsd:string ;
    rdfs:comment "For Care Site: The identifier of the care_site as it appears in the source data. This could be an identifier separate from the name of the care_site."@en,
        """For Condition Occurrence: This field houses the verbatim value from the source data representing the condition that occurred. For example, this could be an ICD10 or Read code.
This code is mapped to a Standard Condition Concept in the Standardized Vocabularies and the original code is stored here for reference."""@en,
        "For Cost: The source value for the cost as it appears in the source data"@en,
        """For Device Exposure: This field houses the verbatim value from the source data representing the device exposure that occurred. For example, this could be an NDC or Gemscript code.
This code is mapped to a Standard Device Concept in the Standardized Vocabularies and the original code is stored here for reference."""@en,
        """For Drug Exposure: This field houses the verbatim value from the source data representing the drug exposure that occurred. For example, this could be an NDC or Gemscript code.
This code is mapped to a Standard Drug Concept in the Standardized Vocabularies and the original code is stored here for reference."""@en,
        "For Location: Put the verbatim value for the location here, as it shows up in the source."@en,
        """For Measurement: This field houses the verbatim value from the source data representing the Measurement that occurred. For example, this could be an ICD10 or Read code.
This code is mapped to a Standard Measurement Concept in the Standardized Vocabularies and the original code is stored here for reference."""@en,
        "For Note: The source value mapped to the NOTE_CLASS_CONCEPT_ID."@en,
        """For Observation: This field houses the verbatim value from the source data representing the Observation that occurred. For example, this could be an ICD10 or Read code.
This code is mapped to a Standard Concept in the Standardized Vocabularies and the original code is stored here for reference."""@en,
        """For Person: Use this field to link back to persons in the source data. This is typically used for error checking of ETL logic.
Some use cases require the ability to link back to persons in the source data. This field allows for the storing of the person value as it appears in the source. This field is not required but strongly recommended."""@en,
        """For Procedure Occurrence: This field houses the verbatim value from the source data representing the procedure that occurred. For example, this could be an CPT4 or OPCS4 code.
Use this value to look up the source concept id and then map the source concept id to a standard concept id."""@en,
        """For Provider: Use this field to link back to providers in the source data. This is typically used for error checking of ETL logic.
Some use cases require the ability to link back to providers in the source data. This field allows for the storing of the provider identifier as it appears in the source."""@en,
        """For Visit Detail: This field houses the verbatim value from the source data representing the kind of visit detail that took place (inpatient, outpatient, emergency, etc.)
If there is information about the kind of visit detail in the source data that value should be stored here. If a visit is an amalgamation of visits from the source then use a hierarchy to choose the VISIT_DETAIL_SOURCE_VALUE, such as IP -> ER-> OP. This should line up with the logic chosen to determine how visits are created."""@en,
        """For Visit Occurrence: This field houses the verbatim value from the source data representing the kind of visit that took place (inpatient, outpatient, emergency, etc.)
If there is information about the kind of visit in the source data that value should be stored here. If a visit is an amalgamation of visits from the source then use a hierarchy to choose the visit source value, such as IP -> ER-> OP. This should line up with the logic chosen to determine how visits are created."""@en ;
    rdfs:domain [ a owl:Class ;
            owl:unionOf ( omop:CareSite omop:ProcedureOccurrence omop:BaseVisit omop:BasePerson omop:Specimen omop:ConditionOccurrence omop:Cost omop:Location omop:Exposure omop:Measurement omop:Note omop:Observation ) ] ;
    rdfs:range xsd:string ;
    omop:omop_cdm_name "care_site.care_site_source_value#271 AS str"^^xsd:string,
        "condition_occurrence.condition_source_value#74 AS str"^^xsd:string,
        "cost.cost_source_value#314 AS str"^^xsd:string,
        "device_exposure.device_source_value#127 AS str"^^xsd:string,
        "drug_exposure.drug_source_value#96 AS str"^^xsd:string,
        "location.location_source_value#258 AS str"^^xsd:string,
        "measurement.measurement_source_value#145 AS str"^^xsd:string,
        "note.note_source_value#192 AS str"^^xsd:string,
        "observation.observation_source_value#163 AS str"^^xsd:string,
        "person.person_source_value#13 AS str"^^xsd:string,
        "procedure_occurrence.procedure_source_value#111 AS str"^^xsd:string,
        "provider.provider_source_value#281 AS str"^^xsd:string,
        "specimen.specimen_source_value#218 AS str"^^xsd:string,
        "visit_detail.visit_detail_source_value#52 AS str"^^xsd:string,
        "visit_occurrence.visit_source_value#35 AS str"^^xsd:string .

omop:DrugExposure a owl:Class ;
    rdfs:label "Drug exposure"^^xsd:string ;
    rdfs:comment "This table captures records about the exposure to a Drug ingested or otherwise introduced into the body. A Drug is a biochemical substance formulated in such a way that when administered to a Person it will exert a certain biochemical effect on the metabolism. Drugs include prescription and over-the-counter medicines, vaccines, and large-molecule biologic therapies. Radiological devices ingested or applied locally do not count as Drugs."@en ;
    rdfs:subClassOf [ a owl:Restriction ;
            owl:allValuesFrom xsd:string ;
            owl:onProperty omop:stop_reason ],
        [ a owl:Restriction ;
            owl:onProperty [ owl:inverseOf omop:has_drug_exposure ] ;
            owl:someValuesFrom omop:Person ],
        [ a owl:Restriction ;
            owl:allValuesFrom xsd:date ;
            owl:onProperty omop:verbatim_end_date ],
        [ a owl:Restriction ;
            owl:allValuesFrom xsd:integer ;
            owl:onProperty omop:refills ],
        [ a owl:Restriction ;
            owl:allValuesFrom xsd:decimal ;
            owl:onProperty omop:quantity ],
        [ a owl:Restriction ;
            owl:allValuesFrom xsd:integer ;
            owl:onProperty omop:days_supply ],
        [ a owl:Restriction ;
            owl:allValuesFrom xsd:string ;
            owl:onProperty omop:sig ],
        [ a owl:Restriction ;
            owl:allValuesFrom omop:Concept ;
            owl:onProperty omop:has_route ],
        [ a owl:Restriction ;
            owl:allValuesFrom xsd:string ;
            owl:onProperty omop:lot_number ],
        [ a owl:Restriction ;
            owl:allValuesFrom xsd:string ;
            owl:onProperty omop:route_source_value ],
        [ a owl:Restriction ;
            owl:allValuesFrom xsd:string ;
            owl:onProperty omop:dose_unit_source_value ],
        omop:Exposure ;
    omop:omop_cdm_name "drug_exposure"^^xsd:string .

omop:Specimen a owl:Class ;
    rdfs:label "Specimen"^^xsd:string ;
    rdfs:comment "The specimen domain contains the records identifying biological samples from a person."@en ;
    rdfs:subClassOf [ a owl:Restriction ;
            owl:allValuesFrom omop:Concept ;
            owl:onProperty omop:has_concept ],
        [ a owl:Restriction ;
            owl:onProperty omop:has_concept ;
            owl:someValuesFrom omop:Concept ],
        [ a owl:Restriction ;
            owl:allValuesFrom omop:Concept ;
            owl:onProperty omop:has_type ],
        [ a owl:Restriction ;
            owl:onProperty omop:has_type ;
            owl:someValuesFrom omop:Concept ],
        [ a owl:Restriction ;
            owl:allValuesFrom owl:Thing ;
            owl:onProperty omop:has_source ],
        [ a owl:Restriction ;
            owl:allValuesFrom xsd:decimal ;
            owl:onProperty omop:quantity ],
        [ a owl:Restriction ;
            owl:allValuesFrom omop:Concept ;
            owl:onProperty omop:has_unit ],
        [ a owl:Restriction ;
            owl:allValuesFrom xsd:string ;
            owl:onProperty omop:unit_source_value ],
        [ a owl:Restriction ;
            owl:onProperty [ owl:inverseOf omop:has_specimen ] ;
            owl:someValuesFrom omop:Person ],
        [ a owl:Restriction ;
            owl:allValuesFrom omop:Concept ;
            owl:onProperty omop:has_anatomic_site ],
        [ a owl:Restriction ;
            owl:allValuesFrom omop:Concept ;
            owl:onProperty omop:has_disease_status ],
        [ a owl:Restriction ;
            owl:allValuesFrom xsd:string ;
            owl:onProperty omop:anatomic_site_source_value ],
        [ a owl:Restriction ;
            owl:allValuesFrom xsd:string ;
            owl:onProperty omop:disease_status_source_value ],
        [ a owl:Restriction ;
            owl:allValuesFrom xsd:string ;
            owl:onProperty omop:source_value ],
        omop:Event ;
    omop:omop_cdm_name "specimen"^^xsd:string .

omop:Vocabulary a owl:Class ;
    rdfs:label "Vocabulary"^^xsd:string ;
    rdfs:comment "The VOCABULARY table includes a list of the Vocabularies collected from various sources or created de novo by the OMOP community. This reference table is populated with a single record for each Vocabulary source and includes a descriptive name and other associated attributes for the Vocabulary."@en ;
    rdfs:subClassOf [ a owl:Restriction ;
            owl:allValuesFrom omop:Concept ;
            owl:onProperty omop:has_concept ],
        [ a owl:Restriction ;
            owl:onProperty omop:has_concept ;
            owl:someValuesFrom omop:Concept ],
        [ a owl:Restriction ;
            owl:allValuesFrom xsd:string ;
            owl:onProperty omop:name ],
        [ a owl:Restriction ;
            owl:onProperty omop:name ;
            owl:someValuesFrom xsd:string ],
        [ a owl:Restriction ;
            owl:allValuesFrom xsd:string ;
            owl:onProperty omop:reference ],
        [ a owl:Restriction ;
            owl:onProperty omop:reference ;
            owl:someValuesFrom xsd:string ],
        [ a owl:Restriction ;
            owl:allValuesFrom xsd:string ;
            owl:onProperty omop:version ],
        omop:OmopCDMThing ;
    omop:omop_cdm_name "vocabulary"^^xsd:string .

omop:Location a owl:Class ;
    rdfs:label "Location"^^xsd:string ;
    rdfs:comment "The LOCATION table represents a generic way to capture physical location or address information of Persons and Care Sites. **New to CDM v6.0** The LOCATION table now includes latitude and longitude."@en ;
    rdfs:subClassOf [ a owl:Restriction ;
            owl:allValuesFrom xsd:string ;
            owl:onProperty omop:address_1 ],
        [ a owl:Restriction ;
            owl:allValuesFrom xsd:string ;
            owl:onProperty omop:address_2 ],
        [ a owl:Restriction ;
            owl:allValuesFrom xsd:string ;
            owl:onProperty omop:city ],
        [ a owl:Restriction ;
            owl:allValuesFrom xsd:string ;
            owl:onProperty omop:state ],
        [ a owl:Restriction ;
            owl:allValuesFrom xsd:string ;
            owl:onProperty omop:zip ],
        [ a owl:Restriction ;
            owl:allValuesFrom xsd:string ;
            owl:onProperty omop:county ],
        [ a owl:Restriction ;
            owl:allValuesFrom xsd:decimal ;
            owl:onProperty omop:latitude ],
        [ a owl:Restriction ;
            owl:allValuesFrom xsd:decimal ;
            owl:onProperty omop:longitude ],
        [ a owl:Restriction ;
            owl:allValuesFrom xsd:string ;
            owl:onProperty omop:source_value ],
        omop:OmopCDMThing ;
    omop:omop_cdm_name "location"^^xsd:string .

omop:Note a owl:Class ;
    rdfs:label "Note"^^xsd:string ;
    rdfs:comment "The NOTE table captures unstructured information that was recorded by a provider about a patient in free text (in ASCII, or preferably in UTF8 format) notes on a given date. The type of note_text is CLOB or varchar(MAX) depending on RDBMS."@en ;
    rdfs:subClassOf [ a owl:Restriction ;
            owl:allValuesFrom omop:Concept ;
            owl:onProperty omop:has_type ],
        [ a owl:Restriction ;
            owl:onProperty omop:has_type ;
            owl:someValuesFrom omop:Concept ],
        [ a owl:Restriction ;
            owl:allValuesFrom owl:Thing ;
            owl:onProperty omop:has_event ],
        [ a owl:Restriction ;
            owl:onProperty [ owl:inverseOf omop:has_note ] ;
            owl:someValuesFrom omop:Person ],
        [ a owl:Restriction ;
            owl:allValuesFrom omop:Concept ;
            owl:onProperty omop:has_event_field ],
        [ a owl:Restriction ;
            owl:allValuesFrom omop:Concept ;
            owl:onProperty omop:has_class ],
        [ a owl:Restriction ;
            owl:onProperty omop:has_class ;
            owl:someValuesFrom omop:Concept ],
        [ a owl:Restriction ;
            owl:allValuesFrom xsd:string ;
            owl:onProperty omop:title ],
        [ a owl:Restriction ;
            owl:allValuesFrom xsd:string ;
            owl:onProperty omop:text ],
        [ a owl:Restriction ;
            owl:onProperty omop:text ;
            owl:someValuesFrom xsd:string ],
        [ a owl:Restriction ;
            owl:allValuesFrom omop:Concept ;
            owl:onProperty omop:has_encoding ],
        [ a owl:Restriction ;
            owl:onProperty omop:has_encoding ;
            owl:someValuesFrom omop:Concept ],
        [ a owl:Restriction ;
            owl:allValuesFrom omop:Concept ;
            owl:onProperty omop:has_language ],
        [ a owl:Restriction ;
            owl:onProperty omop:has_language ;
            owl:someValuesFrom omop:Concept ],
        [ a owl:Restriction ;
            owl:allValuesFrom omop:NoteNlp ;
            owl:onProperty omop:has_note_nlp ],
        [ a owl:Restriction ;
            owl:allValuesFrom omop:Provider ;
            owl:onProperty omop:has_provider ],
        [ a owl:Restriction ;
            owl:allValuesFrom xsd:string ;
            owl:onProperty omop:source_value ],
        omop:ClinicalElement,
        omop:Event ;
    omop:omop_cdm_name "note"^^xsd:string .

omop:BaseVisit a owl:Class ;
    rdfs:label "Base visit"^^xsd:string ;
    rdfs:subClassOf [ a owl:Restriction ;
            owl:allValuesFrom omop:Concept ;
            owl:onProperty omop:has_concept ],
        [ a owl:Restriction ;
            owl:onProperty omop:has_concept ;
            owl:someValuesFrom omop:Concept ],
        [ a owl:Restriction ;
            owl:allValuesFrom omop:Concept ;
            owl:onProperty omop:has_type ],
        [ a owl:Restriction ;
            owl:onProperty omop:has_type ;
            owl:someValuesFrom omop:Concept ],
        [ a owl:Restriction ;
            owl:allValuesFrom omop:Concept ;
            owl:onProperty omop:has_source ],
        [ a owl:Restriction ;
            owl:onProperty omop:has_source ;
            owl:someValuesFrom omop:Concept ],
        [ a owl:Restriction ;
            owl:allValuesFrom omop:Concept ;
            owl:onProperty omop:has_discharge_to ],
        [ a owl:Restriction ;
            owl:onProperty omop:has_discharge_to ;
            owl:someValuesFrom omop:Concept ],
        [ a owl:Restriction ;
            owl:allValuesFrom xsd:string ;
            owl:onProperty omop:discharge_to_source_value ],
        [ a owl:Restriction ;
            owl:allValuesFrom omop:ConditionOccurrence ;
            owl:onProperty omop:has_condition_occurrence ],
        [ a owl:Restriction ;
            owl:allValuesFrom omop:DrugExposure ;
            owl:onProperty omop:has_drug_exposure ],
        [ a owl:Restriction ;
            owl:allValuesFrom omop:ProcedureOccurrence ;
            owl:onProperty omop:has_procedure_occurrence ],
        [ a owl:Restriction ;
            owl:allValuesFrom omop:DeviceExposure ;
            owl:onProperty omop:has_device_exposure ],
        [ a owl:Restriction ;
            owl:allValuesFrom omop:Measurement ;
            owl:onProperty omop:has_measurement ],
        [ a owl:Restriction ;
            owl:allValuesFrom omop:Observation ;
            owl:onProperty omop:has_observation ],
        [ a owl:Restriction ;
            owl:allValuesFrom omop:Note ;
            owl:onProperty omop:has_note ],
        [ a owl:Restriction ;
            owl:allValuesFrom omop:Provider ;
            owl:onProperty omop:has_provider ],
        [ a owl:Restriction ;
            owl:allValuesFrom omop:CareSite ;
            owl:onProperty omop:has_care_site ],
        [ a owl:Restriction ;
            owl:allValuesFrom xsd:string ;
            owl:onProperty omop:source_value ],
        omop:DateDuration,
        omop:DatetimeDuration,
        omop:Occurrence .

omop:Measurement a owl:Class ;
    rdfs:label "Measurement"^^xsd:string ;
    rdfs:comment "The MEASUREMENT table contains records of Measurements, i.e. structured values (numerical or categorical) obtained through systematic and standardized examination or testing of a Person or Person's sample. The MEASUREMENT table contains both orders and results of such Measurements as laboratory tests, vital signs, quantitative findings from pathology reports, etc. Measurements are stored as attribute value pairs, with the attribute as the Measurement Concept and the value representing the result. The value can be a Concept (stored in VALUE_AS_CONCEPT), or a numerical value (VALUE_AS_NUMBER) with a Unit (UNIT_CONCEPT_ID). The Procedure for obtaining the sample is housed in the PROCEDURE_OCCURRENCE table, though it is unnecessary to create a PROCEDURE_OCCURRENCE record for each measurement if one does not exist in the source data. Measurements differ from Observations in that they require a standardized test or some other activity to generate a quantitative or qualitative result. If there is no result, it is assumed that the lab test was conducted but the result was not captured."@en ;
    rdfs:subClassOf [ a owl:Restriction ;
            owl:allValuesFrom omop:Concept ;
            owl:onProperty omop:has_concept ],
        [ a owl:Restriction ;
            owl:onProperty omop:has_concept ;
            owl:someValuesFrom omop:Concept ],
        [ a owl:Restriction ;
            owl:allValuesFrom omop:Concept ;
            owl:onProperty omop:has_type ],
        [ a owl:Restriction ;
            owl:onProperty omop:has_type ;
            owl:someValuesFrom omop:Concept ],
        [ a owl:Restriction ;
            owl:allValuesFrom omop:Concept ;
            owl:onProperty omop:has_source ],
        [ a owl:Restriction ;
            owl:onProperty omop:has_source ;
            owl:someValuesFrom omop:Concept ],
        [ a owl:Restriction ;
            owl:onProperty [ owl:inverseOf omop:has_measurement ] ;
            owl:someValuesFrom omop:Person ],
        [ a owl:Restriction ;
            owl:allValuesFrom xsd:string ;
            owl:onProperty omop:time ],
        [ a owl:Restriction ;
            owl:allValuesFrom omop:Concept ;
            owl:onProperty omop:has_operator ],
        [ a owl:Restriction ;
            owl:allValuesFrom xsd:decimal ;
            owl:onProperty omop:value_as_number ],
        [ a owl:Restriction ;
            owl:allValuesFrom omop:Concept ;
            owl:onProperty omop:has_value_as_concept ],
        [ a owl:Restriction ;
            owl:allValuesFrom omop:Concept ;
            owl:onProperty omop:has_unit ],
        [ a owl:Restriction ;
            owl:allValuesFrom xsd:decimal ;
            owl:onProperty omop:range_low ],
        [ a owl:Restriction ;
            owl:allValuesFrom xsd:decimal ;
            owl:onProperty omop:range_high ],
        [ a owl:Restriction ;
            owl:allValuesFrom xsd:string ;
            owl:onProperty omop:unit_source_value ],
        [ a owl:Restriction ;
            owl:allValuesFrom xsd:string ;
            owl:onProperty omop:value_source_value ],
        [ a owl:Restriction ;
            owl:allValuesFrom omop:Provider ;
            owl:onProperty omop:has_provider ],
        [ a owl:Restriction ;
            owl:allValuesFrom xsd:string ;
            owl:onProperty omop:source_value ],
        omop:Event,
        omop:Occurrence ;
    omop:omop_cdm_name "measurement"^^xsd:string .

omop:Provider a owl:Class ;
    rdfs:label "Provider"^^xsd:string ;
    rdfs:comment "The PROVIDER table contains a list of uniquely identified healthcare providers. These are individuals providing hands-on healthcare to patients, such as physicians, nurses, midwives, physical therapists etc."@en ;
    rdfs:subClassOf [ a owl:Restriction ;
            owl:allValuesFrom xsd:integer ;
            owl:onProperty omop:year_of_birth ],
        [ a owl:Restriction ;
            owl:allValuesFrom xsd:string ;
            owl:onProperty omop:name ],
        [ a owl:Restriction ;
            owl:allValuesFrom xsd:string ;
            owl:onProperty omop:npi ],
        [ a owl:Restriction ;
            owl:allValuesFrom xsd:string ;
            owl:onProperty omop:dea ],
        [ a owl:Restriction ;
            owl:allValuesFrom omop:Concept ;
            owl:onProperty omop:has_specialty ],
        [ a owl:Restriction ;
            owl:onProperty omop:has_specialty ;
            owl:someValuesFrom omop:Concept ],
        [ a owl:Restriction ;
            owl:allValuesFrom xsd:string ;
            owl:onProperty omop:specialty_source_value ],
        [ a owl:Restriction ;
            owl:allValuesFrom omop:Concept ;
            owl:onProperty omop:has_specialty_source ],
        [ a owl:Restriction ;
            owl:onProperty omop:has_specialty_source ;
            owl:someValuesFrom omop:Concept ],
        omop:BasePerson ;
    omop:omop_cdm_name "provider"^^xsd:string .

omop:has_source a owl:FunctionalProperty,
        owl:ObjectProperty ;
    rdfs:label "Has source"^^xsd:string ;
    owlready:python_name "source"^^xsd:string ;
    rdfs:comment """For Condition Occurrence: This is the concept representing the condition source value and may not necessarily be standard. This field is discouraged from use in analysis because it is not required to contain Standard Concepts that are used across the OHDSI community, and should only be used when Standard Concepts do not adequately represent the source detail for the Condition necessary for a given analytic use case. Consider using CONDITION_CONCEPT_ID instead to enable standardized analytics that can be consistent across the network.
If the CONDITION_SOURCE_VALUE is coded in the source data using an OMOP supported vocabulary put the concept id representing the source value here. If not available, set to 0."""@en,
        "For Cost: A foreign key to a Cost Concept that refers to the code used in the source."@en,
        """For Device Exposure: This is the concept representing the device source value and may not necessarily be standard. This field is discouraged from use in analysis because it is not required to contain Standard Concepts that are used across the OHDSI community, and should only be used when Standard Concepts do not adequately represent the source detail for the Device necessary for a given analytic use case. Consider using DEVICE_CONCEPT_ID instead to enable standardized analytics that can be consistent across the network.
If the DEVICE_SOURCE_VALUE is coded in the source data using an OMOP supported vocabulary put the concept id representing the source value here. If unavailable, set to 0."""@en,
        """For Drug Exposure: This is the concept representing the drug source value and may not necessarily be standard. This field is discouraged from use in analysis because it is not required to contain Standard Concepts that are used across the OHDSI community, and should only be used when Standard Concepts do not adequately represent the source detail for the Drug necessary for a given analytic use case. Consider using DRUG_CONCEPT_ID instead to enable standardized analytics that can be consistent across the network.
If the DRUG_SOURCE_VALUE is coded in the source data using an OMOP supported vocabulary put the concept id representing the source value here. If unavailable, set to 0."""@en,
        """For Measurement: This is the concept representing the MEASUREMENT_SOURCE_VALUE and may not necessarily be standard. This field is discouraged from use in analysis because it is not required to contain Standard Concepts that are used across the OHDSI community, and should only be used when Standard Concepts do not adequately represent the source detail for the Measurement necessary for a given analytic use case. Consider using MEASUREMENT_CONCEPT_ID instead to enable standardized analytics that can be consistent across the network.
If the MEASUREMENT_SOURCE_VALUE is coded in the source data using an OMOP supported vocabulary put the concept id representing the source value here. If not available, set to 0."""@en,
        """For Observation: This is the concept representing the OBSERVATION_SOURCE_VALUE and may not necessarily be standard. This field is discouraged from use in analysis because it is not required to contain Standard Concepts that are used across the OHDSI community, and should only be used when Standard Concepts do not adequately represent the source detail for the Observation necessary for a given analytic use case. Consider using OBSERVATION_CONCEPT_ID instead to enable standardized analytics that can be consistent across the network.
If the OBSERVATION_SOURCE_VALUE is coded in the source data using an OMOP supported vocabulary put the concept id representing the source value here. If not available, set to 0."""@en,
        """For Procedure Occurrence: This is the concept representing the procedure source value and may not necessarily be standard. This field is discouraged from use in analysis because it is not required to contain Standard Concepts that are used across the OHDSI community, and should only be used when Standard Concepts do not adequately represent the source detail for the Procedure necessary for a given analytic use case. Consider using PROCEDURE_CONCEPT_ID instead to enable standardized analytics that can be consistent across the network.
If the PROCEDURE_SOURCE_VALUE is coded in the source data using an OMOP supported vocabulary put the concept id representing the source value here. If not available, set to 0."""@en,
        """For Source To Concept Map: A foreign key to the Source
Concept that is being translated
into a Standard Concept.
This is either 0 or should be a number above 2 billion, which are the Concepts reserved for site-specific codes and mappings."""@en,
        "For Specimen: This is the identifier for the specimen from the source system."@en,
        "For Visit Detail: If the VISIT_DETAIL_SOURCE_VALUE is coded in the source data using an OMOP supported vocabulary put the concept id representing the source value here. If not available, map to 0."@en,
        "For Visit Occurrence: If the visit source value is coded in the source data using an OMOP supported vocabulary put the concept id representing the source value here. If not available set to 0."@en ;
    rdfs:domain [ a owl:Class ;
            owl:unionOf ( omop:SourceToConceptMap omop:ProcedureOccurrence omop:BaseVisit omop:Specimen omop:ConditionOccurrence omop:Cost omop:Exposure omop:Measurement omop:Observation omop:NoteNlp ) ] ;
    omop:omop_cdm_name "condition_occurrence.condition_source_concept_id#75 AS Concept"^^xsd:string,
        "cost.cost_source_concept_id#313 AS Concept"^^xsd:string,
        "device_exposure.device_source_concept_id#128 AS Concept"^^xsd:string,
        "drug_exposure.drug_source_concept_id#97 AS Concept"^^xsd:string,
        "measurement.measurement_source_concept_id#146 AS Concept"^^xsd:string,
        "note_nlp.note_nlp_source_concept_id#200 AS Concept"^^xsd:string,
        "observation.observation_source_concept_id#164 AS Concept"^^xsd:string,
        "procedure_occurrence.procedure_source_concept_id#112 AS Concept"^^xsd:string,
        "source_to_concept_map.source_concept_id#403 AS Concept"^^xsd:string,
        "specimen.specimen_source_id#217 AS Thing"^^xsd:string,
        "visit_detail.visit_detail_source_concept_id#53 AS Concept"^^xsd:string,
        "visit_occurrence.visit_source_concept_id#36 AS Concept"^^xsd:string .

omop:Cost a owl:Class ;
    rdfs:label "Cost"^^xsd:string ;
    rdfs:comment """The COST table captures records containing the cost of any medical event recorded in one of the OMOP clinical event tables such as DRUG_EXPOSURE, PROCEDURE_OCCURRENCE, VISIT_OCCURRENCE, VISIT_DETAIL, DEVICE_OCCURRENCE, OBSERVATION or MEASUREMENT.

Each record in the cost table account for the amount of money transacted for the clinical event. So, the COST table may be used to represent both receivables (charges) and payments (paid), each transaction type represented by its COST_CONCEPT_ID. The COST_TYPE_CONCEPT_ID field will use concepts in the Standardized Vocabularies to designate the source (provenance) of the cost data. A reference to the health plan information in the PAYER_PLAN_PERIOD table is stored in the record for information used for the adjudication system to determine the persons benefit for the clinical event."""@en ;
    rdfs:subClassOf [ a owl:Restriction ;
            owl:allValuesFrom omop:Concept ;
            owl:onProperty omop:has_concept ],
        [ a owl:Restriction ;
            owl:allValuesFrom omop:Concept ;
            owl:onProperty omop:has_type ],
        [ a owl:Restriction ;
            owl:allValuesFrom omop:Concept ;
            owl:onProperty omop:has_source ],
        [ a owl:Restriction ;
            owl:allValuesFrom owl:Thing ;
            owl:onProperty omop:has_event ],
        [ a owl:Restriction ;
            owl:onProperty omop:has_event ;
            owl:someValuesFrom owl:Thing ],
        [ a owl:Restriction ;
            owl:allValuesFrom omop:Concept ;
            owl:onProperty omop:has_event_field ],
        [ a owl:Restriction ;
            owl:onProperty omop:has_event_field ;
            owl:someValuesFrom omop:Concept ],
        [ a owl:Restriction ;
            owl:allValuesFrom omop:PayerPlanPeriod ;
            owl:onProperty omop:has_payer_plan_period ],
        [ a owl:Restriction ;
            owl:onProperty [ owl:inverseOf omop:has_cost ] ;
            owl:someValuesFrom omop:Person ],
        [ a owl:Restriction ;
            owl:allValuesFrom omop:Concept ;
            owl:onProperty omop:has_currency ],
        [ a owl:Restriction ;
            owl:allValuesFrom xsd:decimal ;
            owl:onProperty omop:cost ],
        [ a owl:Restriction ;
            owl:allValuesFrom xsd:date ;
            owl:onProperty omop:incurred_date ],
        [ a owl:Restriction ;
            owl:allValuesFrom xsd:date ;
            owl:onProperty omop:billed_date ],
        [ a owl:Restriction ;
            owl:allValuesFrom xsd:date ;
            owl:onProperty omop:paid_date ],
        [ a owl:Restriction ;
            owl:allValuesFrom omop:Concept ;
            owl:onProperty omop:has_revenue_code ],
        [ a owl:Restriction ;
            owl:allValuesFrom omop:Concept ;
            owl:onProperty omop:has_drg ],
        [ a owl:Restriction ;
            owl:allValuesFrom xsd:string ;
            owl:onProperty omop:revenue_code_source_value ],
        [ a owl:Restriction ;
            owl:allValuesFrom xsd:string ;
            owl:onProperty omop:drg_source_value ],
        [ a owl:Restriction ;
            owl:allValuesFrom xsd:string ;
            owl:onProperty omop:source_value ],
        omop:OmopCDMThing ;
    omop:omop_cdm_name "cost"^^xsd:string .

omop:Observation a owl:Class ;
    rdfs:label "Observation"^^xsd:string ;
    rdfs:comment "The OBSERVATION table captures clinical facts about a Person obtained in the context of examination, questioning or a procedure. Any data that cannot be represented by any other domains, such as social and lifestyle facts, medical history, family history, etc. are recorded here. **New to CDM v6.0** An Observation can now be linked to other records in the CDM instance using the fields OBSERVATION_EVENT_ID and OBS_EVENT_FIELD_CONCEPT_ID. To link another record to an Observation, the primary key goes in OBSERVATION_EVENT_ID (CONDITION_OCCURRENCE_ID, DRUG_EXPOSURE_ID, etc.) and the Concept representing the field where the OBSERVATION_EVENT_ID was taken from go in the OBS_EVENT_FIELD_CONCEPT_ID. For example, a CONDITION_OCCURRENCE of Asthma might be linked to an Observation of a family history of Asthma. In this case the CONDITION_OCCURRENCE_ID of the Asthma record would go in OBSERVATION_EVENT_ID of the family history record and the CONCEPT_ID [1147127](https://athena.ohdsi.org/search-terms/terms/1147127) would go in OBS_EVENT_FIELD_CONCEPT_ID to denote that the OBSERVATION_EVENT_ID represents a CONDITION_OCCURRENCE_ID."@en ;
    rdfs:subClassOf [ a owl:Restriction ;
            owl:allValuesFrom omop:Concept ;
            owl:onProperty omop:has_concept ],
        [ a owl:Restriction ;
            owl:onProperty omop:has_concept ;
            owl:someValuesFrom omop:Concept ],
        [ a owl:Restriction ;
            owl:allValuesFrom omop:Concept ;
            owl:onProperty omop:has_type ],
        [ a owl:Restriction ;
            owl:onProperty omop:has_type ;
            owl:someValuesFrom omop:Concept ],
        [ a owl:Restriction ;
            owl:allValuesFrom omop:Concept ;
            owl:onProperty omop:has_source ],
        [ a owl:Restriction ;
            owl:onProperty omop:has_source ;
            owl:someValuesFrom omop:Concept ],
        [ a owl:Restriction ;
            owl:allValuesFrom xsd:decimal ;
            owl:onProperty omop:value_as_number ],
        [ a owl:Restriction ;
            owl:allValuesFrom omop:Concept ;
            owl:onProperty omop:has_value_as_concept ],
        [ a owl:Restriction ;
            owl:allValuesFrom omop:Concept ;
            owl:onProperty omop:has_unit ],
        [ a owl:Restriction ;
            owl:allValuesFrom xsd:string ;
            owl:onProperty omop:unit_source_value ],
        [ a owl:Restriction ;
            owl:onProperty [ owl:inverseOf omop:has_observation ] ;
            owl:someValuesFrom omop:Person ],
        [ a owl:Restriction ;
            owl:allValuesFrom xsd:string ;
            owl:onProperty omop:value_as_string ],
        [ a owl:Restriction ;
            owl:allValuesFrom omop:Concept ;
            owl:onProperty omop:has_qualifier ],
        [ a owl:Restriction ;
            owl:allValuesFrom xsd:string ;
            owl:onProperty omop:qualifier_source_value ],
        [ a owl:Restriction ;
            owl:allValuesFrom owl:Thing ;
            owl:onProperty omop:has_event ],
        [ a owl:Restriction ;
            owl:allValuesFrom omop:Concept ;
            owl:onProperty omop:has_obs_event_field ],
        [ a owl:Restriction ;
            owl:allValuesFrom xsd:dateTime ;
            owl:onProperty omop:value_as_datetime ],
        [ a owl:Restriction ;
            owl:allValuesFrom omop:Provider ;
            owl:onProperty omop:has_provider ],
        [ a owl:Restriction ;
            owl:allValuesFrom xsd:string ;
            owl:onProperty omop:source_value ],
        omop:Event ;
    omop:omop_cdm_name "observation"^^xsd:string .

omop:PayerPlanPeriod a owl:Class ;
    rdfs:label "Payer plan period"^^xsd:string ;
    rdfs:comment "The PAYER_PLAN_PERIOD table captures details of the period of time that a Person is continuously enrolled under a specific health Plan benefit structure from a given Payer. Each Person receiving healthcare is typically covered by a health benefit plan, which pays for (fully or partially), or directly provides, the care. These benefit plans are provided by payers, such as health insurances or state or government agencies. In each plan the details of the health benefits are defined for the Person or her family, and the health benefit Plan might change over time typically with increasing utilization (reaching certain cost thresholds such as deductibles), plan availability and purchasing choices of the Person. The unique combinations of Payer organizations, health benefit Plans and time periods in which they are valid for a Person are recorded in this table."@en ;
    rdfs:subClassOf [ a owl:Restriction ;
            owl:onProperty [ owl:inverseOf omop:has_payer_plan_period ] ;
            owl:someValuesFrom omop:Person ],
        [ a owl:Restriction ;
            owl:allValuesFrom omop:Person ;
            owl:onProperty omop:has_contract_person ],
        [ a owl:Restriction ;
            owl:allValuesFrom omop:Concept ;
            owl:onProperty omop:has_payer ],
        [ a owl:Restriction ;
            owl:onProperty omop:has_payer ;
            owl:someValuesFrom omop:Concept ],
        [ a owl:Restriction ;
            owl:allValuesFrom xsd:string ;
            owl:onProperty omop:payer_source_value ],
        [ a owl:Restriction ;
            owl:allValuesFrom omop:Concept ;
            owl:onProperty omop:has_payer_source ],
        [ a owl:Restriction ;
            owl:onProperty omop:has_payer_source ;
            owl:someValuesFrom omop:Concept ],
        [ a owl:Restriction ;
            owl:allValuesFrom omop:Concept ;
            owl:onProperty omop:has_plan ],
        [ a owl:Restriction ;
            owl:onProperty omop:has_plan ;
            owl:someValuesFrom omop:Concept ],
        [ a owl:Restriction ;
            owl:allValuesFrom xsd:string ;
            owl:onProperty omop:plan_source_value ],
        [ a owl:Restriction ;
            owl:allValuesFrom omop:Concept ;
            owl:onProperty omop:has_plan_source ],
        [ a owl:Restriction ;
            owl:onProperty omop:has_plan_source ;
            owl:someValuesFrom omop:Concept ],
        [ a owl:Restriction ;
            owl:allValuesFrom omop:Concept ;
            owl:onProperty omop:has_contract ],
        [ a owl:Restriction ;
            owl:onProperty omop:has_contract ;
            owl:someValuesFrom omop:Concept ],
        [ a owl:Restriction ;
            owl:allValuesFrom xsd:string ;
            owl:onProperty omop:contract_source_value ],
        [ a owl:Restriction ;
            owl:onProperty omop:contract_source_value ;
            owl:someValuesFrom xsd:string ],
        [ a owl:Restriction ;
            owl:allValuesFrom omop:Concept ;
            owl:onProperty omop:has_contract_source ],
        [ a owl:Restriction ;
            owl:onProperty omop:has_contract_source ;
            owl:someValuesFrom omop:Concept ],
        [ a owl:Restriction ;
            owl:allValuesFrom omop:Concept ;
            owl:onProperty omop:has_sponsor ],
        [ a owl:Restriction ;
            owl:onProperty omop:has_sponsor ;
            owl:someValuesFrom omop:Concept ],
        [ a owl:Restriction ;
            owl:allValuesFrom xsd:string ;
            owl:onProperty omop:sponsor_source_value ],
        [ a owl:Restriction ;
            owl:allValuesFrom omop:Concept ;
            owl:onProperty omop:has_sponsor_source ],
        [ a owl:Restriction ;
            owl:allValuesFrom xsd:string ;
            owl:onProperty omop:family_source_value ],
        [ a owl:Restriction ;
            owl:allValuesFrom omop:Concept ;
            owl:onProperty omop:has_stop_reason_concept ],
        [ a owl:Restriction ;
            owl:allValuesFrom xsd:string ;
            owl:onProperty omop:stop_reason_source_value ],
        [ a owl:Restriction ;
            owl:allValuesFrom omop:Concept ;
            owl:onProperty omop:has_stop_reason_source ],
        omop:DateDuration ;
    omop:omop_cdm_name "payer_plan_period"^^xsd:string .

omop:has_type a owl:FunctionalProperty,
        owl:ObjectProperty ;
    rdfs:label "Has type"^^xsd:string ;
    owlready:python_name "type"^^xsd:string ;
    rdfs:comment """For Condition Occurrence: This field can be used to determine the provenance of the Condition record, as in whether the condition was from an EHR system, insurance claim, registry, or other sources.
Choose the condition_type_concept_id that best represents the provenance of the record. [Accepted Concepts](https://athena.ohdsi.org/search-terms/terms?domain=Type+Concept&standardConcept=Standard&page=1&pageSize=15&query=)."""@en,
        "For Cost: A foreign key identifier to a concept in the CONCEPT table for the provenance or the source of the COST data and belonging to the 'Type Concept' vocabulary"@en,
        """For Device Exposure: You can use the TYPE_CONCEPT_ID to denote the provenance of the record, as in whether the record is from administrative claims or EHR. [Accepted Concepts](https://athena.ohdsi.org/search-terms/terms?domain=Type+Concept&standardConcept=Standard&page=1&pageSize=15&query=).
Choose the drug_type_concept_id that best represents the provenance of the record, for example whether it came from a record of a prescription written or physician administered drug."""@en,
        """For Drug Exposure: You can use the TYPE_CONCEPT_ID to delineate between prescriptions written vs. prescriptions dispensed vs. medication history vs. patient-reported exposure, etc.
Choose the drug_type_concept_id that best represents the provenance of the record, for example whether it came from a record of a prescription written or physician administered drug. [Accepted Concepts](https://athena.ohdsi.org/search-terms/terms?domain=Type+Concept&standardConcept=Standard&page=1&pageSize=15&query=)."""@en,
        """For Measurement: This field can be used to determine the provenance of the Measurement record, as in whether the measurement was from an EHR system, insurance claim, registry, or other sources.
Choose the MEASUREMENT_TYPE_CONCEPT_ID that best represents the provenance of the record, for example whether it came from an EHR record or billing claim. [Accepted Concepts](https://athena.ohdsi.org/search-terms/terms?domain=Type+Concept&standardConcept=Standard&page=1&pageSize=15&query=)."""@en,
        """For Note: The provenance of the note. Most likely this will be EHR.
Put the source system of the note, as in EHR record. [Accepted Concepts](https://athena.ohdsi.org/search-terms/terms?standardConcept=Standard&domain=Type+Concept&page=1&pageSize=15&query=)."""@en,
        """For Observation: This field can be used to determine the provenance of the Observation record, as in whether the measurement was from an EHR system, insurance claim, registry, or other sources.
Choose the OBSERVATION_TYPE_CONCEPT_ID that best represents the provenance of the record, for example whether it came from an EHR record or billing claim. [Accepted Concepts](https://athena.ohdsi.org/search-terms/terms?domain=Type+Concept&standardConcept=Standard&page=1&pageSize=15&query=)."""@en,
        """For Procedure Occurrence: This field can be used to determine the provenance of the Procedure record, as in whether the procedure was from an EHR system, insurance claim, registry, or other sources.
Choose the PROCEDURE_TYPE_CONCEPT_ID that best represents the provenance of the record, for example whether it came from an EHR record or billing claim. If a procedure is recorded as an EHR encounter, the PROCEDURE_TYPE_CONCEPT would be 'EHR encounter record'. [Accepted Concepts](https://athena.ohdsi.org/search-terms/terms?domain=Type+Concept&standardConcept=Standard&page=1&pageSize=15&query=)."""@en,
        "For Specimen: Put the source of the specimen record, as in an EHR system. [Accepted Concepts](https://athena.ohdsi.org/search-terms/terms?standardConcept=Standard&domain=Type+Concept&page=1&pageSize=15&query=)."@en,
        """For Visit Detail: Use this field to understand the provenance of the visit detail record, or where the record comes from.
Populate this field based on the provenance of the visit detail record, as in whether it came from an EHR record or billing claim. [Accepted Concepts](https://athena.ohdsi.org/search-terms/terms?domain=Type+Concept&standardConcept=Standard&page=1&pageSize=15&query=)."""@en,
        """For Visit Occurrence: Use this field to understand the provenance of the visit record, or where the record comes from.
Populate this field based on the provenance of the visit record, as in whether it came from an EHR record or billing claim."""@en ;
    rdfs:domain [ a owl:Class ;
            owl:unionOf ( omop:Death omop:ProcedureOccurrence omop:BaseVisit omop:Specimen omop:Metadata omop:ConditionOccurrence omop:Cost omop:Exposure omop:Measurement omop:Note omop:Observation ) ] ;
    rdfs:range omop:Concept ;
    omop:omop_cdm_name "condition_occurrence.condition_type_concept_id#68 AS Concept"^^xsd:string,
        "cost.cost_type_concept_id#312 AS Concept"^^xsd:string,
        "death.death_type_concept_id#173 AS Concept"^^xsd:string,
        "device_exposure.device_type_concept_id#121 AS Concept"^^xsd:string,
        "drug_exposure.drug_type_concept_id#85 AS Concept"^^xsd:string,
        "measurement.measurement_type_concept_id#135 AS Concept"^^xsd:string,
        "metadata.metadata_type_concept_id#346 AS Concept"^^xsd:string,
        "note.note_type_concept_id#183 AS Concept"^^xsd:string,
        "observation.observation_type_concept_id#154 AS Concept"^^xsd:string,
        "procedure_occurrence.procedure_type_concept_id#105 AS Concept"^^xsd:string,
        "specimen.specimen_type_concept_id#210 AS Concept"^^xsd:string,
        "visit_detail.visit_detail_type_concept_id#49 AS Concept"^^xsd:string,
        "visit_occurrence.visit_type_concept_id#32 AS Concept"^^xsd:string .

omop:name a owl:DatatypeProperty,
        owl:FunctionalProperty ;
    rdfs:label "Name"^^xsd:string ;
    rdfs:comment "For Care Site: The name of the care_site as it appears in the source data"@en,
        "For Cdm Source: The name of the CDM instance."@en,
        "For Cohort Definition: A short description of the cohort"@en,
        """For Concept Class: The name describing the Concept Class, e.g.
Clinical Finding, Ingredient, etc."""@en,
        "For Concept: An unambiguous, meaningful and descriptive name for the Concept."@en,
        """For Domain: The name describing the Domain, e.g.
Condition, Procedure, Measurement
etc."""@en,
        "For Provider: This field is not necessary as it is not necessary to have the actual identity of the Provider. Rather, the idea is to uniquely and anonymously identify providers of care across the database."@en,
        """For Vocabulary: The name describing the vocabulary, for
example International Classification of
Diseases, Ninth Revision, Clinical
Modification, Volume 1 and 2 (NCHS) etc."""@en ;
    rdfs:domain [ a owl:Class ;
            owl:unionOf ( omop:CareSite omop:ConceptSynonym omop:Domain omop:CdmSource omop:Provider omop:Metadata omop:CohortDefinition omop:Vocabulary omop:Concept omop:Relationship omop:ConceptClass ) ] ;
    rdfs:range xsd:string ;
    omop:omop_cdm_name "care_site.care_site_name#268 AS str"^^xsd:string,
        "cdm_source.cdm_source_name#352 AS str"^^xsd:string,
        "cohort_definition.cohort_definition_name#428 AS str"^^xsd:string,
        "concept.concept_name#363 AS str"^^xsd:string,
        "concept_class.concept_class_name#381 AS str"^^xsd:string,
        "concept_synonym.concept_synonym_name#396 AS str"^^xsd:string,
        "domain.domain_name#378 AS str"^^xsd:string,
        "metadata.name#347 AS str"^^xsd:string,
        "provider.provider_name#274 AS str"^^xsd:string,
        "relationship.relationship_name#390 AS str"^^xsd:string,
        "vocabulary.vocabulary_name#373 AS str"^^xsd:string .

omop:OmopCDMThing a owl:Class ;
    rdfs:label "OMOP CDM thing"^^xsd:string ;
    rdfs:subClassOf [ a owl:Restriction ;
            owl:allValuesFrom [ a rdfs:Datatype ;
                    owl:unionOf ( xsd:integer xsd:string ) ] ;
            owl:onProperty omop:id ],
        [ a owl:Restriction ;
            owl:onProperty omop:id ;
            owl:someValuesFrom [ a rdfs:Datatype ;
                    owl:unionOf ( xsd:integer xsd:string ) ] ],
        owl:Thing .

omop:SurveyConduct a owl:Class ;
    rdfs:label "Survey conduct"^^xsd:string ;
    rdfs:comment "The SURVEY_CONDUCT table is used to store an instance of a completed survey or questionnaire."@en ;
    rdfs:subClassOf [ a owl:Restriction ;
            owl:onProperty [ owl:inverseOf omop:has_survey_conduct ] ;
            owl:someValuesFrom omop:Person ],
        [ a owl:Restriction ;
            owl:allValuesFrom omop:Concept ;
            owl:onProperty omop:has_survey ],
        [ a owl:Restriction ;
            owl:onProperty omop:has_survey ;
            owl:someValuesFrom omop:Concept ],
        [ a owl:Restriction ;
            owl:allValuesFrom xsd:date ;
            owl:onProperty omop:survey_start_date ],
        [ a owl:Restriction ;
            owl:allValuesFrom xsd:dateTime ;
            owl:onProperty omop:survey_start_datetime ],
        [ a owl:Restriction ;
            owl:allValuesFrom xsd:date ;
            owl:onProperty omop:survey_end_date ],
        [ a owl:Restriction ;
            owl:allValuesFrom xsd:dateTime ;
            owl:onProperty omop:survey_end_datetime ],
        [ a owl:Restriction ;
            owl:onProperty omop:survey_end_datetime ;
            owl:someValuesFrom xsd:dateTime ],
        [ a owl:Restriction ;
            owl:allValuesFrom omop:Concept ;
            owl:onProperty omop:has_assisted ],
        [ a owl:Restriction ;
            owl:onProperty omop:has_assisted ;
            owl:someValuesFrom omop:Concept ],
        [ a owl:Restriction ;
            owl:allValuesFrom omop:Concept ;
            owl:onProperty omop:has_respondent_type ],
        [ a owl:Restriction ;
            owl:onProperty omop:has_respondent_type ;
            owl:someValuesFrom omop:Concept ],
        [ a owl:Restriction ;
            owl:allValuesFrom omop:Concept ;
            owl:onProperty omop:has_timing ],
        [ a owl:Restriction ;
            owl:onProperty omop:has_timing ;
            owl:someValuesFrom omop:Concept ],
        [ a owl:Restriction ;
            owl:allValuesFrom omop:Concept ;
            owl:onProperty omop:has_collection_method ],
        [ a owl:Restriction ;
            owl:onProperty omop:has_collection_method ;
            owl:someValuesFrom omop:Concept ],
        [ a owl:Restriction ;
            owl:allValuesFrom xsd:string ;
            owl:onProperty omop:assisted_source_value ],
        [ a owl:Restriction ;
            owl:allValuesFrom xsd:string ;
            owl:onProperty omop:respondent_type_source_value ],
        [ a owl:Restriction ;
            owl:allValuesFrom xsd:string ;
            owl:onProperty omop:timing_source_value ],
        [ a owl:Restriction ;
            owl:allValuesFrom xsd:string ;
            owl:onProperty omop:collection_method_source_value ],
        [ a owl:Restriction ;
            owl:allValuesFrom xsd:string ;
            owl:onProperty omop:survey_source_value ],
        [ a owl:Restriction ;
            owl:allValuesFrom omop:Concept ;
            owl:onProperty omop:has_survey_source ],
        [ a owl:Restriction ;
            owl:onProperty omop:has_survey_source ;
            owl:someValuesFrom omop:Concept ],
        [ a owl:Restriction ;
            owl:allValuesFrom xsd:string ;
            owl:onProperty omop:survey_source_identifier ],
        [ a owl:Restriction ;
            owl:allValuesFrom omop:Concept ;
            owl:onProperty omop:has_validated_survey ],
        [ a owl:Restriction ;
            owl:onProperty omop:has_validated_survey ;
            owl:someValuesFrom omop:Concept ],
        [ a owl:Restriction ;
            owl:allValuesFrom xsd:integer ;
            owl:onProperty omop:validated_survey_source_value ],
        [ a owl:Restriction ;
            owl:allValuesFrom xsd:string ;
            owl:onProperty omop:survey_version_number ],
        [ a owl:Restriction ;
            owl:allValuesFrom omop:VisitOccurrence ;
            owl:onProperty omop:has_response_visit_occurrence ],
        [ a owl:Restriction ;
            owl:allValuesFrom omop:Provider ;
            owl:onProperty omop:has_provider ],
        omop:OmopCDMThing ;
    omop:omop_cdm_name "survey_conduct"^^xsd:string .

omop:has_concept a owl:FunctionalProperty,
        owl:ObjectProperty ;
    rdfs:label "Has concept"^^xsd:string ;
    owlready:python_name "concept"^^xsd:string ;
    rdfs:comment "For Concept Class: A Concept that represents the Concept Class."@en,
        "For Condition Era: The Concept Id representing the Condition."@en,
        """For Condition Occurrence: The CONDITION_CONCEPT_ID field is recommended for primary use in analyses, and must be used for network studies. This is the standard concept mapped from the source value which represents a condition
The CONCEPT_ID that the CONDITION_SOURCE_VALUE maps to. Only records whose source values map to concepts with a domain of "Condition" should go in this table. [Accepted Concepts](https://athena.ohdsi.org/search-terms/terms?domain=Condition&standardConcept=Standard&page=1&pageSize=15&query=)."""@en,
        "For Cost: A foreign key that refers to a Standard Cost Concept identifier in the Standardized Vocabularies belonging to the 'Cost' vocabulary."@en,
        """For Device Exposure: The DEVICE_CONCEPT_ID field is recommended for primary use in analyses, and must be used for network studies. This is the standard concept mapped from the source concept id which represents a foreign object or instrument the person was exposed to.
The CONCEPT_ID that the DEVICE_SOURCE_VALUE maps to."""@en,
        "For Domain: A Concept representing the Domain Concept the DOMAIN record belongs to."@en,
        "For Dose Era: The Concept Id representing the specific drug ingredient."@en,
        "For Drug Era: The Concept Id representing the specific drug ingredient."@en,
        """For Drug Exposure: The DRUG_CONCEPT_ID field is recommended for primary use in analyses, and must be used for network studies. This is the standard concept mapped from the source concept id which represents a drug product or molecule otherwise introduced to the body. The drug concepts can have a varying degree of information about drug strength and dose. This information is relevant in the context of quantity and administration information in the subsequent fields plus strength information from the DRUG_STRENGTH table, provided as part of the standard vocabulary download.
The CONCEPT_ID that the DRUG_SOURCE_VALUE maps to. The concept id should be derived either from mapping from the source concept id or by picking the drug concept representing the most amount of detail you have. Records whose source values map to standard concepts with a domain of Drug should go in this table. When the Drug Source Value of the code cannot be translated into Standard Drug Concept IDs, a Drug exposure entry is stored with only the corresponding SOURCE_CONCEPT_ID and DRUG_SOURCE_VALUE and a DRUG_CONCEPT_ID of 0. The Drug Concept with the most detailed content of information is preferred during the mapping process. These are indicated in the CONCEPT_CLASS_ID field of the Concept and are recorded in the following order of precedence: 'Branded Pack', 'Clinical Pack', 'Branded Drug', 'Clinical Drug', 'Branded Drug Component', 'Clinical Drug Component', 'Branded Drug Form', 'Clinical Drug Form', and only if no other information is available 'Ingredient'. Note: If only the drug class is known, the DRUG_CONCEPT_ID field should contain 0. [Accepted Concepts](https://athena.ohdsi.org/search-terms/terms?domain=Drug&standardConcept=Standard&page=1&pageSize=15&query=)."""@en,
        "For Drug Strength: The Concept representing the Branded Drug or Clinical Drug Product."@en,
        """For Measurement: The MEASUREMENT_CONCEPT_ID field is recommended for primary use in analyses, and must be used for network studies.
The CONCEPT_ID that the MEASUREMENT_SOURCE_CONCEPT_ID maps to. Only records whose SOURCE_CONCEPT_IDs map to Standard Concepts with a domain of "Measurement" should go in this table."""@en,
        """For Observation: The OBSERVATION_CONCEPT_ID field is recommended for primary use in analyses, and must be used for network studies.
The CONCEPT_ID that the OBSERVATION_SOURCE_CONCEPT_ID maps to. There is no specified domain that the Concepts in this table must adhere to. The only rule is that records with Concepts in the Condition, Procedure, Drug, Measurement, or Device domains MUST go to the corresponding table."""@en,
        """For Procedure Occurrence: The PROCEDURE_CONCEPT_ID field is recommended for primary use in analyses, and must be used for network studies. This is the standard concept mapped from the source value which represents a procedure
The CONCEPT_ID that the PROCEDURE_SOURCE_VALUE maps to. Only records whose source values map to standard concepts with a domain of "Procedure" should go in this table. [Accepted Concepts](https://athena.ohdsi.org/search-terms/terms?domain=Procedure&standardConcept=Standard&page=1&pageSize=15&query=)."""@en,
        "For Specimen: The standard CONCEPT_ID that the SPECIMEN_SOURCE_VALUE maps to in the specimen domain. [Accepted Concepts](https://athena.ohdsi.org/search-terms/terms?domain=Specimen&standardConcept=Standard&page=1&pageSize=15&query=)"@en,
        """For Visit Detail: This field contains a concept id representing the kind of visit detail, like inpatient or outpatient. All concepts in this field should be standard and belong to the Visit domain.
Populate this field based on the kind of visit that took place for the person. For example this could be "Inpatient Visit", "Outpatient Visit", "Ambulatory Visit", etc. This table will contain standard concepts in the Visit domain. These concepts are arranged in a hierarchical structure to facilitate cohort definitions by rolling up to generally familiar Visits adopted in most healthcare systems worldwide. [Accepted Concepts](https://athena.ohdsi.org/search-terms/terms?domain=Visit&standardConcept=Standard&page=1&pageSize=15&query=)."""@en,
        """For Visit Occurrence: This field contains a concept id representing the kind of visit, like inpatient or outpatient. All concepts in this field should be standard and belong to the Visit domain.
Populate this field based on the kind of visit that took place for the person. For example this could be "Inpatient Visit", "Outpatient Visit", "Ambulatory Visit", etc. This table will contain standard concepts in the Visit domain. These concepts are arranged in a hierarchical structure to facilitate cohort definitions by rolling up to generally familiar Visits adopted in most healthcare systems worldwide."""@en,
        "For Vocabulary: A Concept that represents the Vocabulary the VOCABULARY record belongs to."@en ;
    rdfs:domain [ a owl:Class ;
            owl:unionOf ( omop:BaseVisit omop:ConditionOccurrence omop:Measurement omop:DrugStrength omop:Vocabulary omop:Domain omop:Metadata omop:Exposure omop:Era omop:ProcedureOccurrence omop:Cost omop:Specimen omop:Relationship omop:ConceptClass omop:Observation omop:ConceptSynonym omop:NoteNlp ) ] ;
    rdfs:range omop:Concept ;
    omop:omop_cdm_name "concept_class.concept_class_concept_id#382 AS Concept"^^xsd:string,
        "concept_synonym.concept_id#395 AS Concept"^^xsd:string,
        "condition_era.condition_concept_id#341 AS Concept"^^xsd:string,
        "condition_occurrence.condition_concept_id#63 AS Concept"^^xsd:string,
        "cost.cost_concept_id#311 AS Concept"^^xsd:string,
        "device_exposure.device_concept_id#116 AS Concept"^^xsd:string,
        "domain.domain_concept_id#379 AS Concept"^^xsd:string,
        "dose_era.drug_concept_id#334 AS Concept"^^xsd:string,
        "drug_era.drug_concept_id#327 AS Concept"^^xsd:string,
        "drug_exposure.drug_concept_id#79 AS Concept"^^xsd:string,
        "drug_strength.drug_concept_id#411 AS Concept"^^xsd:string,
        "measurement.measurement_concept_id#131 AS Concept"^^xsd:string,
        "metadata.metadata_concept_id#345 AS Concept"^^xsd:string,
        "note_nlp.note_nlp_concept_id#199 AS Concept"^^xsd:string,
        "observation.observation_concept_id#151 AS Concept"^^xsd:string,
        "procedure_occurrence.procedure_concept_id#102 AS Concept"^^xsd:string,
        "relationship.relationship_concept_id#394 AS Concept"^^xsd:string,
        "specimen.specimen_concept_id#209 AS Concept"^^xsd:string,
        "visit_detail.visit_detail_concept_id#44 AS Concept"^^xsd:string,
        "visit_occurrence.visit_concept_id#27 AS Concept"^^xsd:string,
        "vocabulary.vocabulary_concept_id#376 AS Concept"^^xsd:string .

omop:Person a owl:Class ;
    rdfs:label "Person"^^xsd:string ;
    rdfs:comment "This table serves as the central identity management for all Persons in the database. It contains records that uniquely identify each person or patient, and some demographic information."@en ;
    rdfs:subClassOf [ a owl:Restriction ;
            owl:allValuesFrom omop:VisitOccurrence ;
            owl:onProperty omop:has_visit_occurrence ],
        [ a owl:Restriction ;
            owl:allValuesFrom xsd:integer ;
            owl:onProperty omop:year_of_birth ],
        [ a owl:Restriction ;
            owl:onProperty omop:year_of_birth ;
            owl:someValuesFrom xsd:integer ],
        [ a owl:Restriction ;
            owl:allValuesFrom xsd:integer ;
            owl:onProperty omop:month_of_birth ],
        [ a owl:Restriction ;
            owl:allValuesFrom xsd:integer ;
            owl:onProperty omop:day_of_birth ],
        [ a owl:Restriction ;
            owl:allValuesFrom xsd:dateTime ;
            owl:onProperty omop:birth_datetime ],
        [ a owl:Restriction ;
            owl:allValuesFrom xsd:dateTime ;
            owl:onProperty omop:death_datetime ],
        [ a owl:Restriction ;
            owl:allValuesFrom omop:VisitDetail ;
            owl:onProperty omop:has_visit_detail ],
        [ a owl:Restriction ;
            owl:allValuesFrom omop:Concept ;
            owl:onProperty omop:has_race ],
        [ a owl:Restriction ;
            owl:allValuesFrom omop:ConditionOccurrence ;
            owl:onProperty omop:has_condition_occurrence ],
        [ a owl:Restriction ;
            owl:onProperty omop:has_race ;
            owl:someValuesFrom omop:Concept ],
        [ a owl:Restriction ;
            owl:allValuesFrom omop:Concept ;
            owl:onProperty omop:has_ethnicity ],
        [ a owl:Restriction ;
            owl:allValuesFrom omop:DrugExposure ;
            owl:onProperty omop:has_drug_exposure ],
        [ a owl:Restriction ;
            owl:onProperty omop:has_ethnicity ;
            owl:someValuesFrom omop:Concept ],
        [ a owl:Restriction ;
            owl:allValuesFrom omop:ProcedureOccurrence ;
            owl:onProperty omop:has_procedure_occurrence ],
        [ a owl:Restriction ;
            owl:allValuesFrom omop:DeviceExposure ;
            owl:onProperty omop:has_device_exposure ],
        [ a owl:Restriction ;
            owl:allValuesFrom omop:Measurement ;
            owl:onProperty omop:has_measurement ],
        [ a owl:Restriction ;
            owl:allValuesFrom omop:Location ;
            owl:onProperty omop:has_location ],
        [ a owl:Restriction ;
            owl:allValuesFrom omop:Observation ;
            owl:onProperty omop:has_observation ],
        [ a owl:Restriction ;
            owl:allValuesFrom omop:Death ;
            owl:onProperty omop:has_death ],
        [ a owl:Restriction ;
            owl:allValuesFrom omop:Note ;
            owl:onProperty omop:has_note ],
        [ a owl:Restriction ;
            owl:allValuesFrom omop:Specimen ;
            owl:onProperty omop:has_specimen ],
        [ a owl:Restriction ;
            owl:allValuesFrom omop:SurveyConduct ;
            owl:onProperty omop:has_survey_conduct ],
        [ a owl:Restriction ;
            owl:allValuesFrom omop:Provider ;
            owl:onProperty omop:has_provider ],
        [ a owl:Restriction ;
            owl:allValuesFrom omop:PayerPlanPeriod ;
            owl:onProperty omop:has_payer_plan_period ],
        [ a owl:Restriction ;
            owl:allValuesFrom omop:Cost ;
            owl:onProperty omop:has_cost ],
        [ a owl:Restriction ;
            owl:allValuesFrom omop:DrugEra ;
            owl:onProperty omop:has_drug_era ],
        [ a owl:Restriction ;
            owl:allValuesFrom omop:DoseEra ;
            owl:onProperty omop:has_dose_era ],
        [ a owl:Restriction ;
            owl:allValuesFrom omop:ConditionEra ;
            owl:onProperty omop:has_condition_era ],
        [ a owl:Restriction ;
            owl:allValuesFrom xsd:string ;
            owl:onProperty omop:race_source_value ],
        [ a owl:Restriction ;
            owl:allValuesFrom omop:Concept ;
            owl:onProperty omop:has_race_source ],
        [ a owl:Restriction ;
            owl:onProperty omop:has_race_source ;
            owl:someValuesFrom omop:Concept ],
        [ a owl:Restriction ;
            owl:allValuesFrom xsd:string ;
            owl:onProperty omop:ethnicity_source_value ],
        [ a owl:Restriction ;
            owl:allValuesFrom omop:Concept ;
            owl:onProperty omop:has_ethnicity_source ],
        [ a owl:Restriction ;
            owl:onProperty omop:has_ethnicity_source ;
            owl:someValuesFrom omop:Concept ],
        [ a owl:Restriction ;
            owl:allValuesFrom omop:ObservationPeriod ;
            owl:onProperty omop:has_observation_period ],
        omop:BasePerson ;
    omop:omop_cdm_name "person"^^xsd:string .

omop:Concept a owl:Class ;
    rdfs:label "Concept"^^xsd:string ;
    rdfs:comment """The Standardized Vocabularies contains records, or Concepts, that uniquely identify each fundamental unit of meaning used to express clinical information in all domain tables of the CDM. Concepts are derived from vocabularies, which represent clinical information across a domain (e.g. conditions, drugs, procedures) through the use of codes and associated descriptions. Some Concepts are designated Standard Concepts, meaning these Concepts can be used as normative expressions of a clinical entity within the OMOP Common Data Model and within standardized analytics. Each Standard Concept belongs to one domain, which defines the location where the Concept would be expected to occur within data tables of the CDM.

Concepts can represent broad categories (like 'Cardiovascular disease'), detailed clinical elements ('Myocardial infarction of the anterolateral wall') or modifying characteristics and attributes that define Concepts at various levels of detail (severity of a disease, associated morphology, etc.).

Records in the Standardized Vocabularies tables are derived from national or international vocabularies such as SNOMED-CT, RxNorm, and LOINC, or custom Concepts defined to cover various aspects of observational data analysis."""@en ;
    rdfs:subClassOf [ a owl:Restriction ;
            owl:allValuesFrom omop:ConceptClass ;
            owl:onProperty omop:has_class ],
        [ a owl:Restriction ;
            owl:onProperty omop:has_class ;
            owl:someValuesFrom omop:ConceptClass ],
        [ a owl:Restriction ;
            owl:allValuesFrom omop:Domain ;
            owl:onProperty omop:has_domain ],
        [ a owl:Restriction ;
            owl:onProperty omop:has_domain ;
            owl:someValuesFrom omop:Domain ],
        [ a owl:Restriction ;
            owl:allValuesFrom xsd:string ;
            owl:onProperty omop:name ],
        [ a owl:Restriction ;
            owl:onProperty omop:name ;
            owl:someValuesFrom xsd:string ],
        [ a owl:Restriction ;
            owl:allValuesFrom omop:Vocabulary ;
            owl:onProperty omop:has_vocabulary ],
        [ a owl:Restriction ;
            owl:onProperty omop:has_vocabulary ;
            owl:someValuesFrom omop:Vocabulary ],
        [ a owl:Restriction ;
            owl:allValuesFrom xsd:string ;
            owl:onProperty omop:standard ],
        [ a owl:Restriction ;
            owl:allValuesFrom xsd:string ;
            owl:onProperty omop:code ],
        [ a owl:Restriction ;
            owl:onProperty omop:code ;
            owl:someValuesFrom xsd:string ],
        [ a owl:Restriction ;
            owl:allValuesFrom xsd:date ;
            owl:onProperty omop:valid_start_date ],
        [ a owl:Restriction ;
            owl:onProperty omop:valid_start_date ;
            owl:someValuesFrom xsd:date ],
        [ a owl:Restriction ;
            owl:allValuesFrom xsd:date ;
            owl:onProperty omop:valid_end_date ],
        [ a owl:Restriction ;
            owl:onProperty omop:valid_end_date ;
            owl:someValuesFrom xsd:date ],
        [ a owl:Restriction ;
            owl:allValuesFrom xsd:string ;
            owl:onProperty omop:invalid_reason ],
        omop:OmopCDMThing ;
    omop:omop_cdm_name "concept"^^xsd:string .

